Semantics fixes and half of associativity
Bug fixes in the semantics:
- Minor: The do bind rule had a bug where v >>= e would reduce to e' v
for some e', which obviously does not work
- Major: the move rules in for would only fire if both of the edges were
expressions, however this was breaking associativity

Overhaul in the way the fork commutativity is proved:
- Because of the above change many of the underlying lemmas had to be
changed, so I have changed the structure to be a little bit more
intuitive. Now there is some dead proof code, but I don't have a good
automatic way of identifying it.

Half of the associativity: I have essentially proven that fork a (fork b
c) simulates fork (fork a b) c. It is fairly involved so the other edge
will take time as well.

Adding LibTactics, the library used throughout the proofs.

forkProofs.v
@@ -618,6 +618,22 @@ Proof.
  assumption.
 Qed.
 
+Lemma bind_tau_behave_front_boxed : forall ( e e' x : expr), tauRed e x -> tauRed ((E_live_expr (LM_expr e)) >>= e') ((E_live_expr (LM_expr x)) >>= e').
+Proof.
+ intros.
+ apply star_ind with (R:=tauStep)(X:=expr)(P:= (fun y z => tauRed ((E_live_expr (LM_expr y)) >>= e') ((E_live_expr (LM_expr z)) >>= e'))).
+ intros.
+ apply star_refl.
+ intros.
+ apply S_star with (y:=((E_live_expr (LM_expr y))>>=e')).
+ inversion H0.
+ apply tStep with (s:= s).
+ apply JO_red_movebind.
+ assumption.
+ assumption.
+ assumption.
+Qed.
+
 Lemma bind_lab_behave_front : forall ( e e' x : expr) (l : label), labRed l e x -> labRed l (e >>= e') (x >>= e').
 Proof.
  intros.
@@ -643,6 +659,28 @@ Proof.
  assumption.
 Qed.
 
+Lemma fork_tau_push_ee_1 : forall  (e e' x : expr), tauRed e x -> tauRed (E_apply (E_apply (E_constant CONST_fork) (E_live_expr (LM_expr e))) (E_live_expr (LM_expr e'))) (E_apply (E_apply (E_constant CONST_fork) (E_live_expr (LM_expr x))) (E_live_expr (LM_expr e'))).
+Proof. 
+ intros.
+ apply star_ind with (R:=tauStep)(X:=expr)(P:= (fun y z => tauRed (E_apply (E_apply (E_constant CONST_fork) (E_live_expr (LM_expr y))) (E_live_expr (LM_expr e'))) (E_apply (E_apply (E_constant CONST_fork) (E_live_expr (LM_expr z))) (E_live_expr (LM_expr e'))))).
+ intros; apply star_refl.
+ intros.
+ apply S_star with (y:=(E_apply (E_apply (E_constant CONST_fork) (E_live_expr (LM_expr y))) (E_live_expr (LM_expr e')))).
+ apply tStep with (s:=S_First).
+ inversion H1.
+ substs.
+ inversion H0.
+ substs.
+ apply  JO_red_forkmove1 with (s:=s).
+ assumption.
+ substs.
+ inversion H0.
+ apply  JO_red_forkmove1 with (s:=s).
+ assumption.
+ assumption.
+ assumption.
+Qed.
+
 Lemma fork_tau_behave_edge2 : forall  (e e' x : expr), tauRed e' x -> ~ (is_value_of_expr e) -> tauRed (E_apply (E_apply (E_constant CONST_fork) (E_live_expr (LM_expr e))) (E_live_expr (LM_expr e'))) (E_apply (E_apply (E_constant CONST_fork) (E_live_expr (LM_expr e))) (E_live_expr (LM_expr x))).
 Proof. 
  intros.
@@ -653,6 +691,100 @@ Proof.
  apply tStep with (s:=S_Second).
  inversion H1.
  apply  JO_red_forkmove2 with (s:=s).
+ assumption.
+ assumption.
+ assumption.
+Qed.
+
+Lemma fork_tau_push_ee_2 : forall  (e e' x : expr), tauRed e' x ->  tauRed (E_apply (E_apply (E_constant CONST_fork) (E_live_expr (LM_expr e))) (E_live_expr (LM_expr e'))) (E_apply (E_apply (E_constant CONST_fork) (E_live_expr (LM_expr e))) (E_live_expr (LM_expr x))).
+Proof. 
+ intros.
+ apply star_ind with (R:=tauStep)(X:=expr)(P:= (fun y z => tauRed (E_apply (E_apply (E_constant CONST_fork) (E_live_expr (LM_expr e))) (E_live_expr (LM_expr y))) (E_apply (E_apply (E_constant CONST_fork) (E_live_expr (LM_expr e))) (E_live_expr (LM_expr z))))).
+ intros; apply star_refl.
+ intros.
+ apply S_star with (y:=(E_apply (E_apply (E_constant CONST_fork) (E_live_expr (LM_expr e))) (E_live_expr (LM_expr y)))).
+ apply tStep with (s:=S_Second).
+ inversion H0.
+ apply  JO_red_forkmove2 with (s:=s).
+ assumption.
+ assumption.
+ assumption.
+Qed.
+
+Lemma fork_tau_push_ee_12 : forall  (e e' x y : expr), tauRed e' x -> tauRed e y -> tauRed (E_apply (E_apply (E_constant CONST_fork) (E_live_expr (LM_expr e))) (E_live_expr (LM_expr e'))) (E_apply (E_apply (E_constant CONST_fork) (E_live_expr (LM_expr y))) (E_live_expr (LM_expr x))).
+Proof. 
+ intros.
+ assert (He:=H0).
+ apply fork_tau_push_ee_1 with (e':=e') in He.
+ assert (He':=H).
+ apply fork_tau_push_ee_2 with (e:=y) in He'.
+ apply star_trans with (y:=(E_apply (E_apply (E_constant CONST_fork) (E_live_expr (LM_expr y)))
+          (E_live_expr (LM_expr e')))).
+ assumption.
+ assumption.
+Qed.
+
+Lemma fork_lab_push_ee_1 : forall  (e e' x : expr) (l:label), labRed l e x ->  labRed l (E_apply (E_apply (E_constant CONST_fork) (E_live_expr (LM_expr e))) (E_live_expr (LM_expr e'))) (E_apply (E_apply (E_constant CONST_fork) (E_live_expr (LM_expr x))) (E_live_expr (LM_expr e'))).
+Proof.
+ intros.
+ inversion H.
+ intuition.
+ substs.
+ apply lab_r with (e1:= (E_apply (E_apply (E_constant CONST_fork) (E_live_expr (LM_expr e1)))
+     (E_live_expr (LM_expr e'))))(e2:= (E_apply (E_apply (E_constant CONST_fork) (E_live_expr (LM_expr e2)))
+     (E_live_expr (LM_expr e'))))(s:=S_First).
+ splits.
+ apply fork_tau_push_ee_1;[ assumption ].
+ apply JO_red_forkmove1 with (s:=s);  assumption .
+ apply fork_tau_push_ee_1; [ assumption ].
+Qed.
+
+Lemma fork_lab_push_ee_2 : forall  (e e' x : expr) (l:label), labRed l e' x -> labRed l (E_apply (E_apply (E_constant CONST_fork) (E_live_expr (LM_expr e))) (E_live_expr (LM_expr e'))) (E_apply (E_apply (E_constant CONST_fork) (E_live_expr (LM_expr e))) (E_live_expr (LM_expr x))).
+Proof.
+ intros.
+ inversion H.
+ intuition.
+ substs.
+ apply lab_r with (e1:= (E_apply (E_apply (E_constant CONST_fork) (E_live_expr (LM_expr e)))
+     (E_live_expr (LM_expr e1))))(e2:= (E_apply (E_apply (E_constant CONST_fork) (E_live_expr (LM_expr e)))
+     (E_live_expr (LM_expr e2))))(s:=S_Second).
+ splits.
+ apply fork_tau_push_ee_2;[ assumption ].
+ apply JO_red_forkmove2 with (s:=s); assumption.
+ apply fork_tau_push_ee_2; [ assumption ].
+Qed.
+
+Lemma fork_lab_push_ee_full1 : forall  (e e' x e'' : expr) (l:label), labRed l e x -> tauRed e' e'' -> labRed l (E_apply (E_apply (E_constant CONST_fork) (E_live_expr (LM_expr e))) (E_live_expr (LM_expr e'))) (E_apply (E_apply (E_constant CONST_fork) (E_live_expr (LM_expr x))) (E_live_expr (LM_expr e''))).
+Proof.
+ intros.
+ apply fork_tau_push_ee_2 with (e:=e) in H0.
+ apply fork_lab_push_ee_1 with (e':=e'') in H.
+ inversion H.
+ intuition.
+ substs.
+ apply lab_r with (e1:=e1)(e2:=e2)(s:=s).
+ splits.
+ apply star_trans with (y:=(E_apply (E_apply (E_constant CONST_fork) (E_live_expr (LM_expr e)))
+          (E_live_expr (LM_expr e'')))).
+ assumption.
+ assumption.
+ assumption.
+ assumption.
+Qed.
+
+Lemma fork_lab_push_ee_full2 : forall  (e e' x e'' : expr) (l:label), labRed l e' x -> tauRed e e'' -> labRed l (E_apply (E_apply (E_constant CONST_fork) (E_live_expr (LM_expr e))) (E_live_expr (LM_expr e'))) (E_apply (E_apply (E_constant CONST_fork) (E_live_expr (LM_expr e''))) (E_live_expr (LM_expr x))).
+Proof.
+ intros.
+ apply fork_tau_push_ee_1 with (e':=e') in H0.
+ apply fork_lab_push_ee_2 with (e:=e'') in H.
+ inversion H.
+ intuition.
+ substs.
+ apply lab_r with (e1:=e1)(e2:=e2)(s:=s).
+ splits.
+ apply star_trans with (y:=(E_apply (E_apply (E_constant CONST_fork) (E_live_expr (LM_expr e'')))
+          (E_live_expr (LM_expr e')))).
+ assumption.
  assumption.
  assumption.
  assumption.
@@ -717,84 +849,707 @@ Inductive fork_tau_ce_ext_s : relation expr :=
           (E_live_expr (LM_expr e))) e'.
 
 
+Lemma fork_tau_behave_ce_h : forall (x y : expr), tauRed x y ->
+       ((fun a b => 
 
-Lemma fork_tau_behave_ce: forall (expr5 e : expr) (lab : label), tauRed (E_apply (E_apply (E_constant CONST_fork) (E_live_expr (LM_comp lab)))
-          (E_live_expr (LM_expr expr5))) e -> ((e = (E_apply (E_apply (E_constant CONST_fork) (E_live_expr (LM_comp lab)))
-          (E_live_expr (LM_expr expr5))))\/(e = E_live_expr
-       (LM_expr (E_taggingright (E_pair (E_live_expr (LM_comp lab)) expr5))) /\ is_value_of_expr expr5)) .
+    ((exists (expr5 : expr) (lab : label), 
+         a= (E_apply (E_apply (E_constant CONST_fork) (E_live_expr (LM_comp lab))) (E_live_expr (LM_expr expr5))) ) 
+          -> 
+        (exists (expr5 : expr) (lab : label), 
+           a=(E_apply (E_apply (E_constant CONST_fork) (E_live_expr (LM_comp lab))) (E_live_expr (LM_expr expr5))) 
+           /\ (exists ( e' : expr),tauRed expr5 e' /\
+                 (
+                  (
+                   (b = (E_apply (E_apply (E_constant CONST_fork) (E_live_expr (LM_comp lab))) (E_live_expr (LM_expr e'))))
+                    \/
+                   (b = E_live_expr (LM_expr (E_taggingright (E_pair (E_live_expr (LM_comp lab)) e'))) /\ is_value_of_expr e')
+                  )       
+                 )
+               )
+        )
+    )) x y).
 Proof.
+ apply star_ind.
  intros.
- inversion H.
+ destruct H.
+ destruct H.
  substs.
- auto.
- substs.
- inversion H0.
- substs.
- inversion H2.
- right.
- substs.
- apply taured_val_id in H1.
- substs.
+ exists x0 x1.
  splits.
  reflexivity.
+ exists x0.
+ splits.
+ apply star_refl.
+ left.
+ reflexivity.
+ intros.
+ destruct H2.
+ destruct H2.
+ substs.
+ exists x0 x1.
+ splits.
+ reflexivity.
+ inversion H.
+ substs.
+ inversion H2.
+ substs.
+ destruct H1.
+ exists e'' x1.
+ reflexivity.
+ destruct H1.
+ intuition.
+ destruct H4.
+ intuition.
+ substs.
+ simplify_eq H3; clear H3; intros; substs.
+ exists x3.
+ splits.
+ apply S_star with (y:=x).
+ apply tStep with (s:=s0).
  assumption.
+ assumption.
+ left.
+ reflexivity.
+ substs.
+ simplify_eq H3; clear H3; intros; substs.
+ exists x3.
+ splits.
+ apply S_star with (y:=x).
+ apply tStep with (s:=s0).
+ assumption.
+ assumption.
+ right.
+ splits; [reflexivity | assumption].
+ substs.
+ apply taured_val_id in H0.
+ substs.
+ exists x0. 
+ splits; [apply star_refl | right; splits; [ reflexivity | assumption ] ].
  simpl; auto.
  apply red_not_value in H8; simpl in H8; intuition.
  apply red_not_value in H9; simpl in H9; intuition.
 Qed.
 
+
+Lemma fork_tau_behave_ce: forall (expr5 e  : expr) (lab : label), tauRed (E_apply (E_apply (E_constant CONST_fork) (E_live_expr (LM_comp lab)))
+          (E_live_expr (LM_expr expr5))) e -> (exists ( e' : expr),tauRed expr5 e' /\ ((  e = (E_apply (E_apply (E_constant CONST_fork) (E_live_expr (LM_comp lab)))
+          (E_live_expr (LM_expr e'))))\/(e = E_live_expr
+       (LM_expr (E_taggingright (E_pair (E_live_expr (LM_comp lab)) e'))) /\ is_value_of_expr e'))) .
+Proof.
+  intros.
+  assert (
+   (fun a b => 
+
+    ((exists (expr5 : expr) (lab : label), 
+         a= (E_apply (E_apply (E_constant CONST_fork) (E_live_expr (LM_comp lab))) (E_live_expr (LM_expr expr5))) ) 
+          -> 
+        (exists (expr5 : expr) (lab : label), 
+           a=(E_apply (E_apply (E_constant CONST_fork) (E_live_expr (LM_comp lab))) (E_live_expr (LM_expr expr5))) 
+           /\ (exists ( e' : expr),tauRed expr5 e' /\
+                 (
+                  (
+                   (b = (E_apply (E_apply (E_constant CONST_fork) (E_live_expr (LM_comp lab))) (E_live_expr (LM_expr e'))))
+                    \/
+                   (b = E_live_expr (LM_expr (E_taggingright (E_pair (E_live_expr (LM_comp lab)) e'))) /\ is_value_of_expr e')
+                  )       
+                 )
+               )
+        )
+    )) (E_apply (E_apply (E_constant CONST_fork) (E_live_expr (LM_comp lab)))
+         (E_live_expr (LM_expr expr5))) e
+  ).
+  apply fork_tau_behave_ce_h.
+  assumption.
+  simpl in H0.
+  destruct H0.
+  exists expr5 lab; reflexivity.
+  destruct H0.
+  intuition.
+  simplify_eq H1; clear H1; intros; substs.
+  assumption.
+Qed.
+
+
+Lemma fork_tau_ec_push_h : forall (x y : expr), tauRed x y ->
+       ((fun a b => 
+
+    ((forall (lab : label), 
+         tauRed (E_apply (E_apply (E_constant CONST_fork) (E_live_expr (LM_expr a))) (E_live_expr  (LM_comp lab)))  (E_apply (E_apply (E_constant CONST_fork) (E_live_expr (LM_expr b))) (E_live_expr  (LM_comp lab))) ) 
+          
+    )) x y).
+Proof.
+ apply star_ind.
+ intros; apply star_refl.
+ intros.
+ apply S_star with (y:=(E_apply (E_apply (E_constant CONST_fork) (E_live_expr (LM_expr y)))
+     (E_live_expr (LM_comp lab)))).
+ apply tStep with (s:=S_First).
+ inversion H.
+ 
+ apply JO_red_forkmove1 with (s:=s).
+ assumption.
+ apply H1.
+Qed.
+
+Lemma fork_tau_ce_push_h : forall (x y : expr), tauRed x y ->
+       ((fun a b => 
+
+    ((forall (lab : label), 
+         tauRed (E_apply (E_apply (E_constant CONST_fork) (E_live_expr (LM_comp lab))) (E_live_expr   (LM_expr a)))  (E_apply (E_apply (E_constant CONST_fork) (E_live_expr (LM_comp lab))) (E_live_expr   (LM_expr b))) ) 
+          
+    )) x y).
+Proof.
+ apply star_ind.
+ intros; apply star_refl.
+ intros.
+ apply S_star with (y:=(E_apply (E_apply (E_constant CONST_fork) (E_live_expr (LM_comp lab)))
+     (E_live_expr  (LM_expr y)))).
+ apply tStep with (s:=S_Second).
+ inversion H.
+ 
+ apply JO_red_forkmove2 with (s:=s).
+ assumption.
+ apply H1.
+Qed.
+
+Lemma fork_tau_swap_ce: forall (expr5 e  : expr) (lab : label), tauRed (E_apply (E_apply (E_constant CONST_fork) (E_live_expr (LM_comp lab)  ))
+          (E_live_expr  (LM_expr expr5))) e -> (exists ( e' : expr),tauRed expr5 e' /\ ((  e = (E_apply (E_apply (E_constant CONST_fork) (E_live_expr (LM_comp lab)))
+          (E_live_expr   (LM_expr e'))) /\ tauRed (E_apply (E_apply (E_constant CONST_fork) (E_live_expr  (LM_expr expr5) ))
+          (E_live_expr   (LM_comp lab))) (E_apply (E_apply (E_constant CONST_fork) (E_live_expr   (LM_expr e')))
+          (E_live_expr  (LM_comp lab)))  )\/(e = E_live_expr
+       (LM_expr (E_taggingright (E_pair (E_live_expr (LM_comp lab)) e'))) /\ is_value_of_expr e' /\ tauRed (E_apply (E_apply (E_constant CONST_fork) (E_live_expr  (LM_expr expr5) ))
+          (E_live_expr   (LM_comp lab))) (E_live_expr
+       (LM_expr (E_taggingleft (E_pair e' (E_live_expr  (LM_comp lab)))))) ))) .
+Proof.
+intros.
+ apply fork_tau_behave_ce in H.
+ intuition.
+ destruct H.
+ intuition.
+ substs.
+ exists x.
+ intuition.
+ left.
+ intuition.
+ apply fork_tau_ec_push_h.
+ assumption.
+ substs.
+ exists x.
+ intuition.
+ right.
+ intuition. 
+ assert (tauRed
+  (E_apply (E_apply (E_constant CONST_fork) (E_live_expr (LM_expr expr5)  ))
+     (E_live_expr (LM_comp lab)))  (E_apply (E_apply (E_constant CONST_fork) (E_live_expr (LM_expr x)  ))
+     (E_live_expr (LM_comp lab)))).
+ apply fork_tau_ec_push_h.
+ assumption.
+ apply star_S with (y:=(E_apply (E_apply (E_constant CONST_fork) (E_live_expr (LM_expr x)))
+         (E_live_expr (LM_comp lab)  ))).
+ assumption.
+ apply tStep with (s:=S_First).
+ apply JO_red_forkdeath1.
+ assumption.
+Qed.
+
+Lemma fork_tau_behave_ec_h : forall (x y : expr), tauRed x y ->
+       ((fun a b => 
+
+    ((exists (expr5 : expr) (lab : label), 
+         a= (E_apply (E_apply (E_constant CONST_fork) (E_live_expr (LM_expr expr5))) (E_live_expr  (LM_comp lab))) ) 
+          -> 
+        (exists (expr5 : expr) (lab : label), 
+           a=(E_apply (E_apply (E_constant CONST_fork) (E_live_expr (LM_expr expr5) )) (E_live_expr  (LM_comp lab))) 
+           /\ (exists ( e' : expr),tauRed expr5 e' /\
+                 (
+                  (
+                   (b = (E_apply (E_apply (E_constant CONST_fork) (E_live_expr (LM_expr e') )) (E_live_expr  (LM_comp lab))))
+                    \/
+                   (b = E_live_expr (LM_expr (E_taggingleft (E_pair e' (E_live_expr (LM_comp lab))))) /\ is_value_of_expr e')
+                  )       
+                 )
+               )
+        )
+    )) x y).
+Proof.
+ apply star_ind.
+ intros.
+ destruct H.
+ destruct H.
+ substs.
+ exists x0 x1.
+ splits.
+ reflexivity.
+ exists x0.
+ splits.
+ apply star_refl.
+ left.
+ reflexivity.
+ intros.
+ destruct H2.
+ destruct H2.
+ substs.
+ exists x0 x1.
+ splits.
+ reflexivity.
+ inversion H.
+ substs.
+ inversion H2.
+ substs.
+ destruct H1.
+ exists e'' x1.
+ reflexivity.
+ destruct H1.
+ intuition.
+ destruct H4.
+ intuition.
+ substs.
+ simplify_eq H3; clear H3; intros; substs.
+ exists x3.
+ splits.
+ apply S_star with (y:=x).
+ apply tStep with (s:=s0).
+ assumption.
+ assumption.
+ left.
+ reflexivity.
+ substs.
+ simplify_eq H3; clear H3; intros; substs.
+ exists x3.
+ splits.
+ apply S_star with (y:=x).
+ apply tStep with (s:=s0).
+ assumption.
+ assumption.
+ right.
+ splits; [reflexivity | assumption].
+ substs.
+ apply taured_val_id in H0.
+ substs.
+ exists x0. 
+ splits; [apply star_refl | right; splits; [ reflexivity | assumption ] ].
+ simpl; auto.
+ apply red_not_value in H8; simpl in H8; intuition.
+ apply red_not_value in H9; simpl in H9; intuition.
+Qed.
+
+
+Lemma fork_tau_behave_ec: forall (expr5 e  : expr) (lab : label), tauRed (E_apply (E_apply (E_constant CONST_fork) (E_live_expr  (LM_expr expr5) ))
+          (E_live_expr (LM_comp lab))) e -> (exists ( e' : expr),tauRed expr5 e' /\ ((  e = (E_apply (E_apply (E_constant CONST_fork) (E_live_expr (LM_expr e')))
+          (E_live_expr  (LM_comp lab))))\/(e = E_live_expr
+       (LM_expr (E_taggingleft (E_pair e' (E_live_expr (LM_comp lab))))) /\ is_value_of_expr e'))) .
+Proof.
+  intros.
+  assert (
+   (fun a b => 
+
+    ((exists (expr5 : expr) (lab : label), 
+         a= (E_apply (E_apply (E_constant CONST_fork) (E_live_expr (LM_expr expr5))) (E_live_expr  (LM_comp lab))) ) 
+          -> 
+        (exists (expr5 : expr) (lab : label), 
+           a=(E_apply (E_apply (E_constant CONST_fork) (E_live_expr (LM_expr expr5))) (E_live_expr  (LM_comp lab))) 
+           /\ (exists ( e' : expr),tauRed expr5 e' /\
+                 (
+                  (
+                   (b = (E_apply (E_apply (E_constant CONST_fork) (E_live_expr (LM_expr e'))) (E_live_expr (LM_comp lab))))
+                    \/
+                   (b = E_live_expr (LM_expr (E_taggingleft (E_pair e' (E_live_expr (LM_comp lab))))) /\ is_value_of_expr e')
+                  )       
+                 )
+               )
+        )
+    )) (E_apply (E_apply (E_constant CONST_fork) (E_live_expr (LM_expr expr5) ))
+         (E_live_expr  (LM_comp lab))) e
+  ).
+  apply fork_tau_behave_ec_h.
+  assumption.
+  simpl in H0.
+  destruct H0.
+  exists expr5 lab; reflexivity.
+  destruct H0.
+  intuition.
+  simplify_eq H1; clear H1; intros; substs.
+  assumption.
+Qed.
+
+Lemma fork_tau_swap_ec: forall (expr5 e  : expr) (lab : label), tauRed (E_apply (E_apply (E_constant CONST_fork) (E_live_expr  (LM_expr expr5) ))
+          (E_live_expr (LM_comp lab))) e -> (exists ( e' : expr),tauRed expr5 e' /\ ((  e = (E_apply (E_apply (E_constant CONST_fork) (E_live_expr (LM_expr e')))
+          (E_live_expr  (LM_comp lab))) /\ tauRed (E_apply (E_apply (E_constant CONST_fork) (E_live_expr   (LM_comp lab)))
+          (E_live_expr  (LM_expr expr5))) (E_apply (E_apply (E_constant CONST_fork) (E_live_expr   (LM_comp lab)))
+          (E_live_expr  (LM_expr e')))  )\/(e = E_live_expr
+       (LM_expr (E_taggingleft (E_pair e' (E_live_expr (LM_comp lab))))) /\ is_value_of_expr e' /\ tauRed (E_apply (E_apply (E_constant CONST_fork) (E_live_expr   (LM_comp lab)))
+          (E_live_expr  (LM_expr expr5))) (E_live_expr
+       (LM_expr (E_taggingright (E_pair (E_live_expr (LM_comp lab)) e')))) ))) .
+Proof.
+intros.
+ apply fork_tau_behave_ec in H.
+ intuition.
+ destruct H.
+ intuition.
+ substs.
+ exists x.
+ intuition.
+ left.
+ intuition.
+ apply fork_tau_ce_push_h.
+ assumption.
+ substs.
+ exists x.
+ intuition.
+ right.
+ intuition. 
+ assert (tauRed
+  (E_apply (E_apply (E_constant CONST_fork) (E_live_expr (LM_comp lab)))
+     (E_live_expr (LM_expr expr5)))  (E_apply (E_apply (E_constant CONST_fork) (E_live_expr (LM_comp lab)))
+     (E_live_expr (LM_expr x)))).
+ apply fork_tau_ce_push_h.
+ assumption.
+ apply star_S with (y:=(E_apply (E_apply (E_constant CONST_fork) (E_live_expr (LM_comp lab)))
+         (E_live_expr (LM_expr x)))).
+ assumption.
+ apply tStep with (s:=S_Second).
+ apply JO_red_forkdeath2.
+ assumption.
+Qed.
+
+
 Lemma fork_label_origin_ce: forall (expr5 e : expr) (lab l : label), labRed l (E_apply (E_apply (E_constant CONST_fork) (E_live_expr (LM_comp lab)))
-          (E_live_expr (LM_expr expr5))) e -> (l=lab).
+          (E_live_expr (LM_expr expr5))) e -> ((l=lab) \/ (exists (e' : expr), labRed l expr5 e')).
 Proof.
  intros.
  inversion H; intuition; substs.
  apply fork_tau_behave_ce in H4.
  substs.
- intuition; substs.
- inversion H0; intuition; substs.
- apply red_not_value in H7; simpl in H7; intuition.
- apply red_not_value in H8; simpl in H8; intuition.
- apply red_not_value in H0; simpl in H0; intuition.
-Qed.
-
-Lemma fork_tau_behave_ec: forall (expr5 e : expr) (lab : label), tauRed (E_apply (E_apply (E_constant CONST_fork) (E_live_expr (LM_expr expr5)) ) (E_live_expr (LM_comp lab))) e -> 
- ((e = (E_apply (E_apply (E_constant CONST_fork) (E_live_expr (LM_expr expr5))) (E_live_expr (LM_comp lab))))\/(e=E_live_expr
-       (LM_expr (E_taggingleft (E_pair expr5 (E_live_expr (LM_comp lab))))) /\ is_value_of_expr expr5)) .
-Proof.
- intros.
- inversion H.
- left.
- reflexivity.
+ destruct H4.
+ intuition.
  substs.
  inversion H0.
  substs.
- inversion H2.
+ right.
+ exists e''.
+ apply lab_r with (e1:=x)(e2:=e'')(s:=s0).
+ splits; [assumption | assumption | apply star_refl ].
  substs.
- apply taured_val_id in H1.
+ left; reflexivity.
+ apply red_not_value in H8; simpl in H8; intuition.
+ apply red_not_value in H9; simpl in H9; intuition.
+ substs.
+ apply red_not_value in H0; simpl in H0; intuition.
+Qed.
+
+Lemma fork_label_behave_ce: forall (expr5 e : expr) (lab l : label), labRed l (E_apply (E_apply (E_constant CONST_fork) (E_live_expr (LM_comp lab)))
+          (E_live_expr (LM_expr expr5))) e -> (
+           ((l=lab) /\ (exists (e' : expr), tauRed expr5 e' /\ e=(E_live_expr (LM_expr (E_taggingleft (E_pair (E_constant (CONST_unit)) (E_live_expr (LM_expr e'))))))))
+           \/
+           ( (exists (e' : expr), labRed l expr5 e' /\ e=((E_apply (E_apply (E_constant CONST_fork) (E_live_expr (LM_comp lab)))
+          (E_live_expr (LM_expr e'))))))
+           \/
+           ( (exists (e' : expr), labRed l expr5 e' /\ e=(E_live_expr (LM_expr (E_taggingright (E_pair (E_live_expr (LM_comp lab)) e')))) /\ is_value_of_expr e'))
+          ).
+Proof.
+ intros.
+ inversion H; intuition; substs.
+ apply fork_tau_behave_ce in H4.
+ substs.
+ destruct H4.
+ intuition.
+ substs.
+ inversion H0.
  substs.
  right.
+ apply fork_tau_behave_ce in H6.
+ substs.
+ destruct H6.
+ intuition.
+ substs.
+ left.
+ exists x0.
  splits.
+ apply lab_r with (e1:=x)(e2:=e'')(s:=s0).
+ splits; [assumption | assumption | assumption ]. 
+ reflexivity.
+ substs.
+ right.
+ exists x0.
+ splits.
+ apply lab_r with (e1:=x)(e2:=e'')(s:=s0).
+ splits; [assumption | assumption | assumption ]. 
  reflexivity.
  assumption.
+ substs.
+ left.
+ splits.
+ reflexivity.
+ apply taured_val_id in H6; substs.
+ exists x.
+ splits; [assumption | reflexivity ].
  simpl; auto.
  apply red_not_value in H8; simpl in H8; intuition.
  apply red_not_value in H9; simpl in H9; intuition.
+ substs.
+ apply red_not_value in H0; simpl in H0; intuition.
 Qed.
 
-Lemma fork_label_origin_ec: forall (expr5 e : expr) (lab l : label), labRed l (E_apply (E_apply (E_constant CONST_fork) (E_live_expr (LM_expr expr5))) (E_live_expr (LM_comp lab))) e -> (l=lab (* \/ (exists (e' : expr), labRed l expr5 e' /\ e = (E_apply (E_apply (E_constant CONST_fork) (E_live_expr (LM_expr e'))) (E_live_expr (LM_comp lab))))*)).
+Lemma fork_label_swap_ec_ce: forall (expr5 e : expr) (lab l : label), labRed l (E_apply (E_apply (E_constant CONST_fork) (E_live_expr (LM_comp lab)))
+          (E_live_expr (LM_expr expr5))) e -> (
+           ((l=lab) /\ (exists (e' : expr), tauRed expr5 e' /\ e=(E_live_expr (LM_expr (E_taggingleft (E_pair (E_constant (CONST_unit)) (E_live_expr (LM_expr e')))))) /\
+               labRed l (E_apply (E_apply (E_constant CONST_fork) (E_live_expr (LM_expr expr5)))
+          (E_live_expr (LM_comp lab))) (E_live_expr (LM_expr (E_taggingright (E_pair  (E_live_expr (LM_expr e')) (E_constant (CONST_unit))))))
+                ))
+           \/
+           ( (exists (e' : expr), labRed l expr5 e' /\ e=((E_apply (E_apply (E_constant CONST_fork) (E_live_expr (LM_comp lab)))
+          (E_live_expr (LM_expr e')))) /\ labRed l (E_apply (E_apply (E_constant CONST_fork) (E_live_expr (LM_expr expr5)))
+          (E_live_expr (LM_comp lab))) (E_apply (E_apply (E_constant CONST_fork) (E_live_expr (LM_expr e')))
+          (E_live_expr (LM_comp lab)))))
+           \/
+           ( (exists (e' : expr), labRed l expr5 e' /\ e=(E_live_expr (LM_expr (E_taggingright (E_pair (E_live_expr (LM_comp lab)) e')))) /\ is_value_of_expr e' /\
+             labRed l (E_apply (E_apply (E_constant CONST_fork) (E_live_expr (LM_expr expr5)))
+          (E_live_expr (LM_comp lab))) (E_live_expr (LM_expr (E_taggingleft (E_pair  e' (E_live_expr (LM_comp lab))))))
+           ))
+          ).
+Proof.
+ intros.
+ apply  fork_label_behave_ce in H.
+ intuition.
+ left.
+ substs.
+ destruct H1.
+ intuition.
+ substs.
+ exists x.
+ splits. assumption. reflexivity.
+ apply lab_r with (e1:=(E_apply (E_apply (E_constant CONST_fork) (E_live_expr (LM_expr x)))
+     (E_live_expr (LM_comp lab))))(e2:=(E_live_expr
+     (LM_expr
+        (E_taggingright
+           (E_pair (E_live_expr (LM_expr x)) (E_constant CONST_unit))))))(s:=S_Second).
+ splits.
+ apply fork_tau_ec_push_h.
+ assumption.
+ apply JO_red_forkdocomp2.
+ apply star_refl.
+ right.
+ left.
+ destruct H.
+ intuition; substs.
+ exists x.
+ splits.
+ assumption.
+ reflexivity.
+ destruct H0.
+ intuition.
+ apply lab_r with (e1:=(E_apply (E_apply (E_constant CONST_fork) (E_live_expr (LM_expr e1)))
+     (E_live_expr (LM_comp lab))))(e2:=(E_apply (E_apply (E_constant CONST_fork) (E_live_expr (LM_expr e2)))
+     (E_live_expr (LM_comp lab))))(s:=S_First).
+ splits.
+ apply fork_tau_ec_push_h.
+ assumption.
+ apply JO_red_forkmove1 with (s:=s).
+ assumption.
+ apply fork_tau_ec_push_h.
+ assumption.
+ right.
+ right.
+ destruct H.
+ intuition.
+ exists x.
+ substs.
+ splits.
+ assumption.
+ reflexivity.
+ assumption.
+ destruct H0.
+ intuition.
+ apply lab_r with (e1:=(E_apply (E_apply (E_constant CONST_fork) (E_live_expr (LM_expr e1)))
+     (E_live_expr (LM_comp lab))))(e2:=(E_apply (E_apply (E_constant CONST_fork) (E_live_expr (LM_expr e2)))
+     (E_live_expr (LM_comp lab))))(s:=S_First).
+ splits.
+ apply fork_tau_ec_push_h.
+ assumption.
+ apply JO_red_forkmove1 with (s:=s).
+ assumption.
+ apply star_trans with (y:=(E_apply (E_apply (E_constant CONST_fork) (E_live_expr (LM_expr e3)))
+     (E_live_expr (LM_comp lab)))).
+ apply fork_tau_ec_push_h.
+ assumption.
+ apply S_star with (y:=(E_live_expr
+     (LM_expr (E_taggingleft (E_pair e3 (E_live_expr (LM_comp lab))))))).
+ apply tStep with (s:=S_First).
+ apply JO_red_forkdeath1.
+ assumption.
+ apply star_refl.
+Qed.
+
+Lemma fork_label_origin_ec: forall (expr5 e : expr) (lab l : label), labRed l (E_apply (E_apply (E_constant CONST_fork) (E_live_expr (LM_expr expr5)))
+          (E_live_expr  (LM_comp lab))) e -> ((l=lab) \/ (exists (e' : expr), labRed l expr5 e')).
 Proof.
  intros.
  inversion H; intuition; substs.
  apply fork_tau_behave_ec in H4.
  substs.
+ destruct H4.
  intuition.
  substs.
- inversion H0; intuition; substs.
- apply red_not_value in H7; simpl in H7; intuition.
+ inversion H0.
+ substs.
+ right.
+ exists e''.
+ apply lab_r with (e1:=x)(e2:=e'')(s:=s0).
+ splits; [assumption | assumption | apply star_refl ].
+ substs.
+ left; reflexivity.
  apply red_not_value in H8; simpl in H8; intuition.
+ apply red_not_value in H9; simpl in H9; intuition.
  substs.
  apply red_not_value in H0; simpl in H0; intuition.
 Qed.
+
+
+Lemma fork_label_behave_ec: forall (expr5 e : expr) (lab l : label), labRed l (E_apply (E_apply (E_constant CONST_fork) (E_live_expr (LM_expr expr5)))
+          (E_live_expr  (LM_comp lab))) e -> (
+           ((l=lab) /\ (exists (e' : expr), tauRed expr5 e' /\ e=(E_live_expr (LM_expr (E_taggingright (E_pair  (E_live_expr (LM_expr e')) (E_constant (CONST_unit))))))))
+           \/
+           ( (exists (e' : expr), labRed l expr5 e' /\ e=((E_apply (E_apply (E_constant CONST_fork) (E_live_expr (LM_expr e')))
+          (E_live_expr  (LM_comp lab))))))
+           \/
+           ( (exists (e' : expr), labRed l expr5 e' /\ e=(E_live_expr (LM_expr (E_taggingleft (E_pair  e' (E_live_expr (LM_comp lab)))))) /\ is_value_of_expr e'))
+          ).
+Proof.
+ intros.
+ inversion H; intuition; substs.
+ apply fork_tau_behave_ec in H4.
+ substs.
+ destruct H4.
+ intuition.
+ substs.
+ inversion H0.
+ substs.
+ right.
+ apply fork_tau_behave_ec in H6.
+ substs.
+ destruct H6.
+ intuition.
+ substs.
+ left.
+ exists x0.
+ splits.
+ apply lab_r with (e1:=x)(e2:=e'')(s:=s0).
+ splits; [assumption | assumption | assumption ]. 
+ reflexivity.
+ substs.
+ right.
+ exists x0.
+ splits.
+ apply lab_r with (e1:=x)(e2:=e'')(s:=s0).
+ splits; [assumption | assumption | assumption ]. 
+ reflexivity.
+ assumption.
+ substs.
+ left.
+ splits.
+ reflexivity.
+ apply taured_val_id in H6; substs.
+ exists x.
+ splits; [assumption | reflexivity ].
+ simpl; auto.
+ apply red_not_value in H8; simpl in H8; intuition.
+ apply red_not_value in H9; simpl in H9; intuition.
+ substs.
+ apply red_not_value in H0; simpl in H0; intuition.
+Qed.
+
+Lemma fork_label_swap_ce_ec: forall (expr5 e : expr) (lab l : label), labRed l (E_apply (E_apply (E_constant CONST_fork) (E_live_expr (LM_expr expr5)))
+          (E_live_expr (LM_comp lab)))  e -> (
+           ((l=lab) /\ (exists (e' : expr), tauRed expr5 e' /\ e= (E_live_expr (LM_expr (E_taggingright (E_pair  (E_live_expr (LM_expr e')) (E_constant (CONST_unit)))))) /\
+               labRed l (E_apply (E_apply (E_constant CONST_fork) (E_live_expr (LM_comp lab)))
+          (E_live_expr (LM_expr expr5))) (E_live_expr (LM_expr (E_taggingleft (E_pair (E_constant (CONST_unit)) (E_live_expr (LM_expr e'))))))
+ 
+                ))
+           \/
+           ( (exists (e' : expr), labRed l expr5 e' /\ e= (E_apply (E_apply (E_constant CONST_fork) (E_live_expr (LM_expr e'))) (E_live_expr (LM_comp lab))) /\ labRed l 
+(E_apply (E_apply (E_constant CONST_fork) (E_live_expr (LM_comp lab)))
+          (E_live_expr (LM_expr expr5))) ((E_apply (E_apply (E_constant CONST_fork) (E_live_expr (LM_comp lab)))
+          (E_live_expr (LM_expr e'))))  ))
+           \/
+           ( (exists (e' : expr), labRed l expr5 e' /\ e= (E_live_expr (LM_expr (E_taggingleft (E_pair  e' (E_live_expr (LM_comp lab)))))) /\ is_value_of_expr e' /\
+             labRed l (E_apply (E_apply (E_constant CONST_fork) (E_live_expr (LM_comp lab)))
+          (E_live_expr (LM_expr expr5)))  (E_live_expr (LM_expr (E_taggingright (E_pair (E_live_expr (LM_comp lab)) e'))))
+           ))
+          ).
+Proof.
+ intros.
+ apply  fork_label_behave_ec in H.
+ intuition.
+ left.
+ substs.
+ destruct H1.
+ intuition.
+ substs.
+ exists x.
+ splits. assumption. reflexivity.
+ apply lab_r with (e1:=(E_apply (E_apply (E_constant CONST_fork) (E_live_expr (LM_comp lab)))
+     (E_live_expr (LM_expr x))))(e2:=(E_live_expr
+     (LM_expr
+        (E_taggingleft
+           (E_pair  (E_constant CONST_unit) (E_live_expr (LM_expr x)))))))(s:=S_First).
+ splits.
+ apply fork_tau_ce_push_h.
+ assumption.
+ apply JO_red_forkdocomp1.
+ apply star_refl.
+ right.
+ left.
+ destruct H.
+ intuition; substs.
+ exists x.
+ splits.
+ assumption.
+ reflexivity.
+ destruct H0.
+ intuition.
+ apply lab_r with (e1:=(E_apply (E_apply (E_constant CONST_fork) (E_live_expr (LM_comp lab)))
+     (E_live_expr  (LM_expr e1))))(e2:=(E_apply (E_apply (E_constant CONST_fork) (E_live_expr (LM_comp lab)))
+     (E_live_expr  (LM_expr e2))))(s:=S_Second).
+ splits.
+ apply fork_tau_ce_push_h.
+ assumption.
+ apply JO_red_forkmove2 with (s:=s).
+ assumption.
+ apply fork_tau_ce_push_h.
+ assumption.
+ right.
+ right.
+ destruct H.
+ intuition.
+ exists x.
+ substs.
+ splits.
+ assumption.
+ reflexivity.
+ assumption.
+ destruct H0.
+ intuition.
+ apply lab_r with (e1:=(E_apply (E_apply (E_constant CONST_fork) (E_live_expr (LM_comp lab)))
+     (E_live_expr  (LM_expr e1))))(e2:=(E_apply (E_apply (E_constant CONST_fork) (E_live_expr (LM_comp lab)))
+     (E_live_expr  (LM_expr e2))))(s:=S_Second).
+ splits.
+ apply fork_tau_ce_push_h.
+ assumption.
+ apply JO_red_forkmove2 with (s:=s).
+ assumption.
+ apply star_trans with (y:=(E_apply (E_apply (E_constant CONST_fork) (E_live_expr (LM_comp lab)))
+     (E_live_expr  (LM_expr e3)))).
+ apply fork_tau_ce_push_h.
+ assumption.
+ apply S_star with (y:=(E_live_expr
+     (LM_expr (E_taggingright (E_pair (E_live_expr (LM_comp lab)) e3))))).
+ apply tStep with (s:=S_Second).
+ apply JO_red_forkdeath2.
+ assumption.
+ apply star_refl.
+Qed.
+
+
 
 Lemma fork_tau_behave_cc : forall (e : expr) (lab1 lab2 : label), tauRed (E_apply (E_apply (E_constant CONST_fork) (E_live_expr (LM_comp lab1))) (E_live_expr (LM_comp lab2))) e -> e= (E_apply (E_apply (E_constant CONST_fork) (E_live_expr (LM_comp lab1))) (E_live_expr (LM_comp lab2))).
 Proof.
@@ -808,6 +1563,17 @@ Proof.
  substs.
   apply red_not_value in H8; simpl in H8; intuition.
  apply red_not_value in H9; simpl in H9; intuition.
+Qed.
+
+Lemma fork_tau_swap_cc : forall (e : expr) (lab1 lab2 : label), tauRed (E_apply (E_apply (E_constant CONST_fork) (E_live_expr (LM_comp lab1))) (E_live_expr (LM_comp lab2))) e -> (e= (E_apply (E_apply (E_constant CONST_fork) (E_live_expr (LM_comp lab1))) (E_live_expr (LM_comp lab2)))
+ /\ tauRed (E_apply (E_apply (E_constant CONST_fork) (E_live_expr (LM_comp lab2))) (E_live_expr (LM_comp lab1))) (E_apply (E_apply (E_constant CONST_fork) (E_live_expr (LM_comp lab2))) (E_live_expr (LM_comp lab1)))
+).
+Proof.
+ intros.
+ apply fork_tau_behave_cc in H.
+ substs.
+ intuition.
+ apply star_refl.
 Qed.
 
 Lemma fork_label_origin_cc: forall (e : expr) (lab1 lab2 l : label), labRed l (E_apply (E_apply (E_constant CONST_fork) (E_live_expr (LM_comp lab1))) (E_live_expr (LM_comp lab2))) e -> 
@@ -839,6 +1605,64 @@ Proof.
  apply red_not_value in H11; simpl in H11; intuition.
  apply red_not_value in H12; simpl in H12; intuition.
 Qed.
+
+Lemma fork_label_swap_cc: forall (e : expr) (lab1 lab2 l : label), labRed l (E_apply (E_apply (E_constant CONST_fork) (E_live_expr (LM_comp lab1))) (E_live_expr (LM_comp lab2))) e -> 
+((l=lab1 /\ e = (E_live_expr
+       (LM_expr
+          (E_taggingleft
+             (E_pair (E_constant CONST_unit) (E_live_expr (LM_comp lab2)))))) /\  
+          labRed l (E_apply (E_apply (E_constant CONST_fork) (E_live_expr (LM_comp lab2))) (E_live_expr (LM_comp lab1))) 
+                ((E_live_expr
+          (LM_expr
+             (E_taggingright
+                (E_pair (E_live_expr (LM_comp lab2)) (E_constant CONST_unit))))))
+               ) 
+ \/ (l=lab2 /\ e =((E_live_expr
+          (LM_expr
+             (E_taggingright
+                (E_pair (E_live_expr (LM_comp lab1)) (E_constant CONST_unit)))))) /\
+                labRed l (E_apply (E_apply (E_constant CONST_fork) (E_live_expr (LM_comp lab2))) (E_live_expr (LM_comp lab1))) 
+                    (E_live_expr
+       (LM_expr
+          (E_taggingleft
+             (E_pair (E_constant CONST_unit) (E_live_expr (LM_comp lab1))))))
+                )).
+Proof.
+ intros.
+ inversion H; intuition; substs.
+ inversion H4; intuition; substs.
+ inversion H0; intuition; substs.
+ left. splits. reflexivity.
+ inversion H6. reflexivity. substs. inversion H1. substs.
+ inversion H3.
+ apply taured_val_id in H6; substs.
+ apply lab_r with (e1:=(E_apply (E_apply (E_constant CONST_fork) (E_live_expr (LM_comp lab2)))
+     (E_live_expr (LM_comp l))))(e2:=(E_live_expr
+     (LM_expr
+        (E_taggingright
+           (E_pair (E_live_expr (LM_comp lab2)) (E_constant CONST_unit))))))(s:=S_Second).
+ splits; [apply star_refl | apply JO_red_forkdocomp2 | apply star_refl].
+ simpl; auto.
+ right.
+ splits. reflexivity.
+ apply taured_val_id in H6.
+ substs.
+ reflexivity.
+ simpl; auto.
+ apply lab_r with (e1:=(E_apply (E_apply (E_constant CONST_fork) (E_live_expr (LM_comp l)))
+     (E_live_expr (LM_comp lab1))))(e2:=(E_live_expr
+     (LM_expr
+        (E_taggingleft
+           (E_pair (E_constant CONST_unit) (E_live_expr (LM_comp lab1)))))))(s:=S_First).
+ splits; [apply star_refl | apply JO_red_forkdocomp1 | apply star_refl].
+ apply red_not_value in H8; simpl in H8; intuition.
+ apply red_not_value in H9; simpl in H9; intuition.
+ inversion H1; intuition; substs.
+ inversion H3; intuition; substs.
+ apply red_not_value in H11; simpl in H11; intuition.
+ apply red_not_value in H12; simpl in H12; intuition.
+Qed.
+
 
 
 Lemma fork_tau_step_behave_ee: forall (p q e : expr), tauStep (E_apply (E_apply (E_constant CONST_fork) (E_live_expr (LM_expr p)) ) (E_live_expr (LM_expr q))) e -> 
@@ -949,6 +1773,74 @@ Proof.
  specialize (H p q).
  apply H.
  reflexivity.
+Qed.
+
+Lemma fork_tau_swap_ee : forall (p q e : expr), tauRed (E_apply (E_apply (E_constant CONST_fork) (E_live_expr (LM_expr p)) ) (E_live_expr (LM_expr q))) e -> 
+((exists (p' q' : expr), tauRed p p' /\ tauRed q q' /\ e = (E_apply (E_apply (E_constant CONST_fork) (E_live_expr (LM_expr p')) ) (E_live_expr (LM_expr q')))
+   /\ tauRed (E_apply (E_apply (E_constant CONST_fork) (E_live_expr (LM_expr q)) ) (E_live_expr (LM_expr p))) (E_apply (E_apply (E_constant CONST_fork) (E_live_expr (LM_expr q')) ) (E_live_expr (LM_expr p')))
+  ) \/ 
+  ((exists (p' vq : expr), is_value_of_expr vq /\ tauRed p p' /\ tauRed q vq /\ e = ((E_live_expr (LM_expr  (  (E_taggingright  (E_pair  (E_live_expr (LM_expr p')) vq ) ) ) )))
+   /\ tauRed (E_apply (E_apply (E_constant CONST_fork) (E_live_expr (LM_expr q)) ) (E_live_expr (LM_expr p))) ((E_live_expr (LM_expr  (E_taggingleft  (  (E_pair vq (E_live_expr (LM_expr p'))  ) ) ) )))
+  ) \/ 
+  (
+   (exists (vp q' : expr), is_value_of_expr vp /\ tauRed p vp /\ tauRed q q' /\ e=((E_live_expr (LM_expr  (E_taggingleft  (  (E_pair vp (E_live_expr (LM_expr q'))  ) ) ) ))) /\ 
+      tauRed (E_apply (E_apply (E_constant CONST_fork) (E_live_expr (LM_expr q)) ) (E_live_expr (LM_expr p))) ((E_live_expr (LM_expr  (  (E_taggingright  (E_pair  (E_live_expr (LM_expr q')) vp ) ) ) )))
+  )))) .
+Proof.
+ intros.
+ 
+ apply fork_tau_behave_ee in H.
+ intuition.
+ left.
+ destruct H0; destruct H.
+ intuition.
+ substs.
+ exists x x0.
+ splits.
+ assumption.
+ assumption.
+ reflexivity.
+ apply fork_tau_push_ee_12.
+ assumption.
+ assumption.
+ destruct H; destruct H.
+ intuition.
+ substs.
+ right.
+ left.
+ exists x x0.
+ splits.
+ assumption.
+ assumption.
+ assumption.
+ reflexivity.
+ apply star_S with (y:=(E_apply (E_apply (E_constant CONST_fork) (E_live_expr (LM_expr x0)))
+     (E_live_expr (LM_expr x)))).
+ apply fork_tau_push_ee_12.
+ assumption.
+ assumption.
+ apply tStep with (s:=S_First).
+ apply JO_red_forkdeath1.
+ assumption.
+ destruct H; destruct H.
+ intuition.
+ substs.
+ right.
+ right.
+ exists x x0.
+ splits.
+ assumption.
+ assumption.
+ assumption.
+ reflexivity.
+ apply star_S with (y:=(E_apply (E_apply (E_constant CONST_fork) (E_live_expr (LM_expr x0)))
+     (E_live_expr (LM_expr x)))).
+ apply fork_tau_push_ee_12.
+ assumption.
+ assumption.
+ apply tStep with (s:=S_Second).
+ apply JO_red_forkdeath2.
+ assumption.
 Qed.
 (*
 
@@ -1142,33 +2034,941 @@ Proof.
  destruct H0; destruct H0; intuition; substs; simpl in H1; intuition.
 Qed.
 
+Lemma fork_label_swap_ee : forall (e' e e'' : expr) (l : label), labRed l (E_apply (E_apply (E_constant CONST_fork) (E_live_expr (LM_expr e)) ) (E_live_expr (LM_expr e'))) e'' -> 
+ ((exists (f : expr), labRed l e f /\ (
+((exists ( q' : expr), tauRed e' q' /\ e'' = (E_apply (E_apply (E_constant CONST_fork) (E_live_expr (LM_expr f)) ) (E_live_expr (LM_expr q'))) /\
+   labRed l (E_apply (E_apply (E_constant CONST_fork) (E_live_expr (LM_expr e')) ) (E_live_expr (LM_expr e)))  (E_apply (E_apply (E_constant CONST_fork) (E_live_expr (LM_expr q')) ) (E_live_expr (LM_expr f)))
+   ) \/ 
+  ((exists ( vq : expr), is_value_of_expr vq /\ tauRed e' vq /\ e'' = ((E_live_expr (LM_expr  (  (E_taggingright  (E_pair  (E_live_expr (LM_expr f)) vq ) ) ) ))) /\
+    labRed l (E_apply (E_apply (E_constant CONST_fork) (E_live_expr (LM_expr e')) ) (E_live_expr (LM_expr e))) ((E_live_expr (LM_expr  (E_taggingleft  (  (E_pair vq (E_live_expr (LM_expr f))  ) ) ) )))
+  ) \/ 
+  (
+   (exists ( q' : expr), is_value_of_expr f /\  tauRed e' q' /\ e''=((E_live_expr (LM_expr  (E_taggingleft  (  (E_pair f (E_live_expr (LM_expr q'))  ) ) ) ))) /\
+     labRed l (E_apply (E_apply (E_constant CONST_fork) (E_live_expr (LM_expr e')) ) (E_live_expr (LM_expr e))) ((E_live_expr (LM_expr  (  (E_taggingright  (E_pair  (E_live_expr (LM_expr q')) f ) ) ) )))
+   ))))
+
+)) 
 
 
-Lemma fork_tau_swap_ee_non_val : forall (p q p' q': expr), (~ (is_value_of_expr p)) -> (~(is_value_of_expr q)) ->  (~ (is_value_of_expr p')) -> (~(is_value_of_expr q')) ->  tauRed
-       (E_apply (E_apply (E_constant CONST_fork) (E_live_expr (LM_expr p)))
-          (E_live_expr (LM_expr q)))
-       (E_apply (E_apply (E_constant CONST_fork) (E_live_expr (LM_expr p')))
-          (E_live_expr (LM_expr q'))) -> tauRed
-       (E_apply (E_apply (E_constant CONST_fork) (E_live_expr (LM_expr q)))
-          (E_live_expr (LM_expr p)))
-       (E_apply (E_apply (E_constant CONST_fork) (E_live_expr (LM_expr q')))
-          (E_live_expr (LM_expr p'))).
+\/ 
+  (exists (f : expr), labRed l e' f /\ (
+((exists (p'  : expr), tauRed e p' /\ e'' = (E_apply (E_apply (E_constant CONST_fork) (E_live_expr (LM_expr p')) ) (E_live_expr (LM_expr f)))  /\
+ labRed l (E_apply (E_apply (E_constant CONST_fork) (E_live_expr (LM_expr e')) ) (E_live_expr (LM_expr e))) (E_apply (E_apply (E_constant CONST_fork) (E_live_expr (LM_expr f)) ) (E_live_expr (LM_expr p')))
+ ) \/ 
+  ((exists (p'  : expr), is_value_of_expr f /\ tauRed e p'  /\ e'' = ((E_live_expr (LM_expr  (  (E_taggingright  (E_pair  (E_live_expr (LM_expr p')) f ) ) ) )))  /\
+   labRed l (E_apply (E_apply (E_constant CONST_fork) (E_live_expr (LM_expr e')) ) (E_live_expr (LM_expr e))) ((E_live_expr (LM_expr  (E_taggingleft  (  (E_pair f (E_live_expr (LM_expr p'))  ) ) ) )))
+  ) \/ 
+  (
+   (exists (vp : expr), is_value_of_expr vp /\ tauRed e vp  /\ e''=((E_live_expr (LM_expr  (E_taggingleft  (  (E_pair vp (E_live_expr (LM_expr f))  ) ) ) ))) /\
+    labRed l (E_apply (E_apply (E_constant CONST_fork) (E_live_expr (LM_expr e')) ) (E_live_expr (LM_expr e)))  ((E_live_expr (LM_expr  (  (E_taggingright  (E_pair  (E_live_expr (LM_expr f)) vp ) ) ) )))
+   )))) 
+
+))).
 Proof.
  intros.
- apply fork_tau_behave_ee in H3.
+ apply fork_label_origin_ee in H.
  intuition.
- destruct H4; destruct H3; intuition.
- simplify_eq H6; intros; substs.
- apply fork_tau_behave_edge12.
- assumption. assumption. assumption. assumption. assumption. assumption.
- destruct H3; destruct H3; intuition.
- simplify_eq H7; intros; substs.
- destruct H3; destruct H3; intuition.
- simplify_eq H7; intros; substs; assumption.
+ destruct H0.
+ left.
+ exists x.
+ intuition.
+ destruct H.
+ left. 
+ exists x0.
+ intuition.
+ substs.
+ apply fork_lab_push_ee_full2.
+ assumption.
+ assumption.
+ right.
+ left.
+ destruct H1.
+ exists x0.
+ intuition.
+ substs.
+ assert (labRed l
+  (E_apply (E_apply (E_constant CONST_fork) (E_live_expr (LM_expr e')))
+     (E_live_expr (LM_expr e))) (E_apply (E_apply (E_constant CONST_fork) (E_live_expr (LM_expr x0)))
+     (E_live_expr (LM_expr x)))).
+ apply fork_lab_push_ee_full2.
+ assumption.
+ assumption.
+ inversion H2.
+ intuition.
+ substs.
+ apply lab_r with (e1:=e1)(e2:=e2)(s:=s).
+ intuition.
+ apply star_S with (y:=(E_apply (E_apply (E_constant CONST_fork) (E_live_expr (LM_expr x0)))
+          (E_live_expr (LM_expr x)))).
+ assumption.
+ apply tStep with (s:=S_First).
+ apply JO_red_forkdeath1.
+ assumption.
+ right.
+ right.
+ destruct H1.
+ exists x0.
+ intuition.
+ substs.
+ assert (labRed l
+  (E_apply (E_apply (E_constant CONST_fork) (E_live_expr (LM_expr e')))
+     (E_live_expr (LM_expr e))) (E_apply (E_apply (E_constant CONST_fork) (E_live_expr (LM_expr x0)))
+     (E_live_expr (LM_expr x)))).
+ apply fork_lab_push_ee_full2.
+ assumption.
+ assumption.
+ inversion H2.
+ intuition.
+ substs.
+ apply lab_r with (e1:=e1)(e2:=e2)(s:=s).
+ intuition.
+ apply star_S with (y:=(E_apply (E_apply (E_constant CONST_fork) (E_live_expr (LM_expr x0)))
+          (E_live_expr (LM_expr x)))).
+ assumption.
+ apply tStep with (s:=S_Second).
+ apply JO_red_forkdeath2.
+ assumption.
+
+
+ right.
+ destruct H0.
+ exists x.
+ intuition.
+ destruct H.
+ left. 
+ exists x0.
+ intuition.
+ substs.
+ apply fork_lab_push_ee_full1.
+ assumption.
+ assumption.
+ right.
+ left.
+ destruct H1.
+ exists x0.
+ intuition.
+ substs.
+ assert (labRed l
+  (E_apply (E_apply (E_constant CONST_fork) (E_live_expr (LM_expr e')))
+     (E_live_expr (LM_expr e))) (E_apply (E_apply (E_constant CONST_fork) (E_live_expr (LM_expr x)))
+     (E_live_expr (LM_expr x0)))).
+ apply fork_lab_push_ee_full1.
+ assumption.
+ assumption.
+ inversion H2.
+ intuition.
+ substs.
+ apply lab_r with (e1:=e1)(e2:=e2)(s:=s).
+ intuition.
+ apply star_S with (y:=(E_apply (E_apply (E_constant CONST_fork) (E_live_expr (LM_expr x)))
+          (E_live_expr (LM_expr x0)))).
+ assumption.
+ apply tStep with (s:=S_First).
+ apply JO_red_forkdeath1.
+ assumption.
+ right.
+ right.
+ destruct H1.
+ exists x0.
+ intuition.
+ substs.
+ assert (labRed l
+  (E_apply (E_apply (E_constant CONST_fork) (E_live_expr (LM_expr e')))
+     (E_live_expr (LM_expr e))) (E_apply (E_apply (E_constant CONST_fork) (E_live_expr (LM_expr x)))
+     (E_live_expr (LM_expr x0)))).
+ apply fork_lab_push_ee_full1.
+ assumption.
+ assumption.
+ inversion H2.
+ intuition.
+ substs.
+ apply lab_r with (e1:=e1)(e2:=e2)(s:=s).
+ intuition.
+ apply star_S with (y:=(E_apply (E_apply (E_constant CONST_fork) (E_live_expr (LM_expr x)))
+          (E_live_expr (LM_expr x0)))).
+ assumption.
+ apply tStep with (s:=S_Second).
+ apply JO_red_forkdeath2.
+ assumption.
+Qed. 
+
+Lemma fork_tau_swap_total : forall (p q : livemodes) (e : expr) , tauRed (E_apply (E_apply (E_constant CONST_fork) (E_live_expr (p))) (E_live_expr ( q))) e ->
+        (
+         ((exists (p' q' : livemodes), e = (E_apply (E_apply (E_constant CONST_fork) (E_live_expr (p'))) (E_live_expr ( q'))) /\
+              tauRed (E_apply (E_apply (E_constant CONST_fork) (E_live_expr (q)))(E_live_expr ( p))) (E_apply (E_apply (E_constant CONST_fork) (E_live_expr (q'))) (E_live_expr ( p')))
+          )
+          )
+             
+          \/
+         (
+            (exists (p' : expr) (q': livemodes),is_value_of_expr p' /\ e= ((E_live_expr (LM_expr  (E_taggingleft  (  (E_pair p' (E_live_expr (q'))  ) ) ) ))) /\ 
+              tauRed (E_apply (E_apply (E_constant CONST_fork) (E_live_expr (q)))(E_live_expr ( p))) ((E_live_expr (LM_expr  (E_taggingright  (  (E_pair (E_live_expr (q')) p'  ) ) ) )))
+             )
+            \/
+            ((exists (q' : expr) (p': livemodes),is_value_of_expr q' /\ e= ((E_live_expr (LM_expr  (E_taggingright  (  (E_pair (E_live_expr (p')) q' ) ) ) ))) /\ 
+              tauRed (E_apply (E_apply (E_constant CONST_fork) (E_live_expr (q)))(E_live_expr ( p))) ((E_live_expr (LM_expr  (E_taggingleft  (  (E_pair q' (E_live_expr (p')) ) ) ) ))) 
+             )
+            )
+          )
+        ).
+Proof.
+ intros.
+ induction p; induction q.
+ apply fork_tau_swap_cc in H.
+ intuition.
+ substs.
+ left.
+ exists (LM_comp lab) (LM_comp lab0).
+ intuition.
+ apply fork_tau_swap_ce in H.
+ intuition.
+ destruct H.
+ intuition.
+ substs.
+ left.
+ exists (LM_comp lab) (LM_expr x).
+ intuition.
+ substs.
+ right.
+ right.
+ exists  x (LM_comp lab) .
+ intuition.
+ apply fork_tau_swap_ec in H.
+ intuition.
+ destruct H.
+ intuition.
+ substs.
+ left.
+ exists  (LM_expr x) (LM_comp lab).
+ intuition.
+ substs.
+ right.
+ left.
+ exists  x (LM_comp lab) .
+ intuition.
+ apply fork_tau_swap_ee in H.
+ intuition.
+ destruct H0.
+ destruct H.
+ intuition.
+ substs.
+ left.
+ exists (LM_expr x)(LM_expr x0).
+ intuition.
+ right.
+ right.
+ destruct H.
+ destruct H.
+ intuition.
+ substs.
+ exists x0 (LM_expr x).
+ intuition.
+ right.
+ left.
+ destruct H.
+ destruct H.
+ exists (x) (LM_expr x0).
+ intuition.
+Qed.
+
+Lemma fork_tau_behave_total : forall (p q : livemodes) (e : expr) , tauRed (E_apply (E_apply (E_constant CONST_fork) (E_live_expr (p))) (E_live_expr ( q))) e ->
+        (
+         ((exists (p' q' : livemodes), e = (E_apply (E_apply (E_constant CONST_fork) (E_live_expr (p'))) (E_live_expr ( q')))
+          )
+          )
+             
+          \/
+         (
+            (exists (p' : expr) (q': livemodes),is_value_of_expr p' /\ e= ((E_live_expr (LM_expr  (E_taggingleft  (  (E_pair p' (E_live_expr (q'))  ) ) ) ))) 
+             )
+            \/
+            ((exists (q' : expr) (p': livemodes),is_value_of_expr q' /\ e= ((E_live_expr (LM_expr  (E_taggingright  (  (E_pair (E_live_expr (p')) q' ) ) ) ))) 
+             )
+            )
+          )
+        ).
+Proof.
+ intros.
+ apply fork_tau_swap_total in H.
+ intuition.
+ left.
+ destruct H0.
+ destruct H.
+ exists x x0.
+ intuition.
+ right.
+ left.
+ destruct H. destruct H.
+ exists x x0.
+ intuition.
+ right; right.
+ destruct H; destruct H.
+ exists x x0.
+ intuition.
+Qed.
+
+Lemma fork_label_swap_total : forall (p q : livemodes) (e : expr) (l : label), labRed l (E_apply (E_apply (E_constant CONST_fork) (E_live_expr (p))) (E_live_expr ( q))) e ->
+        (
+         ((exists (p' q' : livemodes), e = (E_apply (E_apply (E_constant CONST_fork) (E_live_expr (p'))) (E_live_expr ( q'))) /\
+              labRed l (E_apply (E_apply (E_constant CONST_fork) (E_live_expr (q)))(E_live_expr ( p))) (E_apply (E_apply (E_constant CONST_fork) (E_live_expr (q'))) (E_live_expr ( p')))
+          )
+          )
+             
+          \/
+         (
+            (exists (p' : expr) (q': livemodes),is_value_of_expr p' /\ e= ((E_live_expr (LM_expr  (E_taggingleft  (  (E_pair p' (E_live_expr (q'))  ) ) ) ))) /\ 
+              labRed l (E_apply (E_apply (E_constant CONST_fork) (E_live_expr (q)))(E_live_expr ( p))) ((E_live_expr (LM_expr  (E_taggingright  (  (E_pair (E_live_expr (q')) p'  ) ) ) )))
+             )
+            \/
+            ((exists (q' : expr) (p': livemodes),is_value_of_expr q' /\ e= ((E_live_expr (LM_expr  (E_taggingright  (  (E_pair (E_live_expr (p')) q' ) ) ) ))) /\ 
+              labRed l (E_apply (E_apply (E_constant CONST_fork) (E_live_expr (q)))(E_live_expr ( p))) ((E_live_expr (LM_expr  (E_taggingleft  (  (E_pair q' (E_live_expr (p')) ) ) ) ))) 
+             )
+            )
+          )
+        ).
+Proof.
+ intros.
+ induction p; induction q.
+ apply fork_label_swap_cc in H.
+ intuition.
+ substs.
+ right.
+ left.
+ exists (E_constant CONST_unit) (LM_comp lab0).
+ intuition.
+ simpl; auto.
+ substs.
+ right.
+ right.
+ exists (E_constant CONST_unit) (LM_comp lab).
+ intuition.
+ simpl; auto.
+ apply fork_label_swap_ec_ce in H.
+ intuition.
+ destruct H1.
+ substs.
+ intuition.
+ substs.
+ right.
+ left.
+ exists (E_constant CONST_unit) (LM_expr x).
+ intuition.
+ simpl; auto.
+ left.
+ destruct H.
+ intuition. substs.
+ exists (LM_comp lab) (LM_expr x).
+ intuition.
+ right.
+ right.
+ destruct H.
+ intuition.
+ substs.
+ exists x (LM_comp lab).
+ intuition.
+ apply fork_label_swap_ce_ec in H.
+ intuition.
+ destruct H1.
+ substs.
+ intuition.
+ substs.
+ right.
+ right.
+ exists (E_constant CONST_unit) (LM_expr x).
+ intuition.
+ simpl; auto.
+ left.
+ destruct H.
+ intuition. substs.
+ exists  (LM_expr x) (LM_comp lab).
+ intuition.
+ right.
+ left.
+ destruct H.
+ intuition.
+ substs.
+ exists x (LM_comp lab).
+ intuition.
+ apply fork_label_swap_ee in H.
+ intuition.
+ destruct H0.
+ intuition.
+ destruct H.
+ intuition.
+ substs.
+ left.
+ exists (LM_expr x)(LM_expr x0).
+ intuition.
+ right.
+ right.
+ destruct H1.
+ intuition.
+ substs.
+ exists x0 (LM_expr x).
+ intuition.
+ right.
+ left.
+ destruct H1.
+ exists (x) (LM_expr x0).
+ intuition.
+ destruct H0.
+ intuition.
+ destruct H.
+ intuition.
+ substs.
+ left.
+ exists (LM_expr x0)(LM_expr x).
+ intuition.
+ right.
+ right.
+ destruct H1.
+ intuition.
+ substs.
+ exists x (LM_expr x0).
+ intuition.
+ right.
+ left.
+ destruct H1.
+ exists (x0) (LM_expr x).
+ intuition.
+Qed.
+ 
+Lemma fork_lab_behave : forall (p q : livemodes) (e : expr) (l : label), labRed l (E_apply (E_apply (E_constant CONST_fork) (E_live_expr (p))) (E_live_expr ( q))) e ->
+        (
+         ((exists (p' q' : livemodes), e = (E_apply (E_apply (E_constant CONST_fork) (E_live_expr (p'))) (E_live_expr ( q'))) 
+          )
+          )
+             
+          \/
+         (
+            (exists (p' : expr) (q': livemodes),is_value_of_expr p' /\ e= ((E_live_expr (LM_expr  (E_taggingleft  (  (E_pair p' (E_live_expr (q'))  ) ) ) ))) 
+             )
+            \/
+            ((exists (q' : expr) (p': livemodes),is_value_of_expr q' /\ e= ((E_live_expr (LM_expr  (E_taggingright  (  (E_pair (E_live_expr (p')) q' ) ) ) )))  
+             )
+            )
+          )
+        ).
+Proof.
+ intros.
+ apply fork_label_swap_total in H.
+ intuition.
+ left.
+ destruct H0.
+ destruct H.
+ exists x x0.
+ intuition.
+ right.
+ left.
+ destruct H. destruct H.
+ exists x x0.
+ intuition.
+ right; right.
+ destruct H; destruct H.
+ exists x x0.
+ intuition.
 Qed.
 
 
+Lemma bind_tau_behave_back_h : forall (x y : expr), tauRed x y -> ((fun x y => (exists (e e' : expr), x = (e >>= e') ) -> (exists (e e' : expr), x = (e >>= e') /\ ((exists (f : expr), tauRed e f /\ y = (f >>= e')) \/ (exists (f : expr), tauRed e (E_live_expr (LM_expr f)) /\ ((exists (f' : expr ), (tauRed f f' /\ y=(((E_live_expr (LM_expr f')))>>=e') ) \/ (tauRed f f' /\ is_value_of_expr f' /\ tauRed (E_apply e' f') y))))) )   ) x y). 
+Proof.
+ apply star_ind.
+ intros.
+ destruct H; destruct H.
+ substs.
+ exists x0 x1.
+ splits.
+ reflexivity.
+ left.
+ exists x0.
+ splits.
+ apply star_refl.
+ reflexivity.
+ intros.
+ destruct H2; destruct H2; substs.
+ exists x0 x1.
+ splits.
+ reflexivity.
+ inversion H.
+ substs.
+ inversion H2.
+ substs.
+ assert (  exists e e'0,
+     e' >>= x1 = e >>= e'0 /\
+     ((exists f, tauRed e f /\ z = f >>= e'0) \/
+      (exists f,
+       tauRed e (E_live_expr (LM_expr f)) /\
+       (exists f',
+        tauRed f f' /\ z = E_live_expr (LM_expr f') >>= e'0 \/
+        tauRed f f' /\ is_value_of_expr f' /\ tauRed (E_apply e'0 f') z)))).
+ apply H1.
+ exists e' x1.
+ reflexivity.
+ destruct H3; destruct H3.
+ intuition.
+ simplify_eq H4; clear H4; intros; substs.
+ destruct H3.
+ intuition.
+ substs.
+ left.
+ exists x1.
+ splits.
+ apply S_star with (y:=x).
+ apply tStep with (s:=s).
+ assumption.
+ assumption.
+ reflexivity.
+ simplify_eq H4; clear H4; intros; substs.
+ right.
+ destruct H3.
+ exists x1.
+ splits.
+ apply S_star with (y:=x).
+ apply tStep with (s:=s).
+ assumption.
+ intuition.
+ intuition.
+ substs.
+ assert ( exists e e'0,
+     E_live_expr (LM_expr e') >>= x1 = e >>= e'0 /\
+     ((exists f, tauRed e f /\ z = f >>= e'0) \/
+      (exists f,
+       tauRed e (E_live_expr (LM_expr f)) /\
+       (exists f',
+        tauRed f f' /\ z = E_live_expr (LM_expr f') >>= e'0 \/
+        tauRed f f' /\ is_value_of_expr f' /\ tauRed (E_apply e'0 f') z)))).
+ apply H1.
+ exists (E_live_expr (LM_expr e')) (x1).
+ reflexivity.
+ destruct H3; destruct H3.
+ intuition.
+ substs.
+ simplify_eq H4; clear H4; intros; substs.
+ destruct H3; elim H3; intros.
+ simplify_eq H5; clear H5; intros; substs.
+ apply taured_val_id in H4.
+ substs.
+ right.
+ exists e.
+ splits.
+ apply star_refl.
+ 
+ exists e'.
+ left.
+ splits.
+ apply S_star with (y:=e').
+ apply tStep with (s:=s).
+ assumption.
+ apply star_refl.
+ apply reflexivity.
+ simpl; auto.
+ simplify_eq H4; clear H4; intros; substs.
+ destruct H3.
+ elim H3.
+ intros.
+ apply taured_val_id in H4.
+ simplify_eq H4; clear H4; intros; substs.
+ destruct H5.
+ destruct H4.
+ clear H3.
+ intuition.
+ substs.
+ right.
+ exists e.
+ splits.
+ apply star_refl.
+ exists x1.
+ left.
+ splits.
+ apply S_star with (y:=x).
+ apply tStep with (s:=s).
+ assumption.
+ assumption.
+ apply reflexivity.
+ clear H3.
+ intuition.
+ right.
+ exists e.
+ splits.
+ apply star_refl.
+ exists x1.
+ right.
+ splits.
+ apply S_star with (y:=x).
+ apply tStep with (s:=s).
+ assumption.
+ assumption.
+ assumption.
+ assumption.
+ simpl; auto.
+ substs.
+ right.
+ exists v.
+ splits.
+ apply star_refl.
+ exists v.
+ right.
+ splits.
+ apply star_refl.
+ assumption.
+ assumption.
+Qed.
 
+Lemma bind_lab_behave_back_h : forall (e e' y : expr) (l : label), labRed l (e >>= e') y -> 
+   (( ( (
+            (exists (f : expr), labRed l e f /\ tauRed (f >>= e') y)
+            \/
+            (exists (f : expr), tauRed e (E_live_expr (LM_expr f)) /\ 
+               ((exists (f' : expr ), 
+                  (labRed l f f' /\ tauRed (((E_live_expr (LM_expr f')))>>=e') y ) 
+                   \/ 
+                  (tauRed f f' /\ is_value_of_expr f' /\ labRed l (E_apply e' f') y)
+                 )  
+                )
+            )
+            \/
+            (tauRed e (E_live_expr (LM_comp l)) /\ tauRed (E_apply e' (E_constant CONST_unit)) y
+            )
+          ) )   )). 
+Proof.
+ intros.
+ inversion H.
+ intuition.
+ apply bind_tau_behave_back_h in H4.
+ destruct H4.
+ destruct H4.
+ intuition.
+ substs.
+ destruct H4.
+ intuition.
+ substs.
+ simplify_eq H5; clear H5; intros; substs.
+ inversion H0.
+ substs.
+ apply bind_tau_behave_back_h in H6.
+ destruct H6.
+ destruct H1.
+ intuition.
+ simplify_eq H3; clear H3; intros; substs.
+ destruct H1.
+ intuition.
+ substs.
+ left.
+ exists x0.
+ intuition.
+ apply lab_r with (e1:=x1)(e2:=x2)(s:=s).
+ intuition.
+ apply star_refl.
+ simplify_eq H3; clear H3; intros; substs.
+ destruct H1.
+ intuition.
+ substs.
+ destruct H4.
+ intuition.
+ substs.
+ left.
+ exists (E_live_expr (LM_expr x0)).
+ intuition.
+ apply lab_r with (e1:=x1)(e2:=x2)(s:=s).
+ intuition.
+ apply bind_tau_behave_front_boxed with (e':=x3) in H1.
+ assumption.
+ left.
+ exists (E_live_expr (LM_expr x0)).
+ intuition.
+ apply lab_r with (e1:=x1)(e2:=x2)(s:=s).
+ intuition.
+ apply star_trans with (y:=(E_live_expr (LM_expr x4) >>= x3)).
+ apply bind_tau_behave_front_boxed with (e':=x3) in H1.
+ assumption.
+ apply S_star with (y:=(E_apply x3 x4)).
+ apply tStep with (s:=S_First).
+ apply JO_red_dobind.
+ assumption.
+ assumption.
+ exists e' x0.
+ reflexivity.
+ substs.
+ right.
+ left.
+ exists e.
+ splits.
+ assumption.
+ exists e'.
+ left.
+ intuition.
+ apply lab_r with (e1:=e)(e2:=e')(s:=s).
+ intuition.
+ apply star_refl.
+ apply star_refl.
+ substs.
+ right.
+ right.
+ intuition.
+ simplify_eq H5; clear H5; intros; substs.
+ destruct H4.
+ intuition.
+ destruct H3.
+ intuition.
+ substs.
+ right.
+ left.
+ exists x1.
+ intuition.
+ inversion H0.
+ apply red_not_value in H9; simpl in H9; intuition.
+ substs.
+ exists e'.
+ left.
+ intuition.
+ apply lab_r with (e1:=x2)(e2:=e')(s:=s).
+ intuition.
+ apply star_refl.
+ right.
+  left.
+ exists x1.
+ intuition.
+ exists x2.
+ right.
+ intuition.
+ apply lab_r with (e1:=e1)(e2:=e2)(s:=s).
+ intuition.
+ substs.
+ exists e e'.
+ reflexivity.
+Qed.
+
+
+Lemma ttr_val_not_labred : forall (e v e' : expr)(l:label), totalTauRed e v /\ is_value_of_expr v -> (~ (labRed l e e')).
+Proof.
+ intros.
+ intuition.
+ inversion H0.
+ intuition.
+ assert (totalTauRed e v /\ tauRed e e1).
+ auto.
+ apply ttau_prefix in H7.
+ intuition.
+ inversion H10.
+ substs.
+ apply red_not_value in H; contradiction.
+ substs.
+ inversion H9.
+ intuition.
+ apply H3 in H.
+ auto.
+ substs.
+ inversion H9.
+ substs.
+ apply red_not_value in H; contradiction.
+ substs.
+ inversion H3.
+ apply red_not_value in H5; contradiction.
+Qed.
+
+Lemma fork_swap_bind_lab_behave : forall (p q : livemodes) (e : expr) (l : label), labRed l ((E_apply (E_apply (E_constant CONST_fork) (E_live_expr ( p)))
+          (E_live_expr ( q))) >>= swapf) e ->
+           (
+            (exists (p' q' : livemodes), tauRed ((E_apply (E_apply (E_constant CONST_fork) (E_live_expr ( p')))
+          (E_live_expr ( q'))) >>= swapf) e /\  labRed l ((E_apply (E_apply (E_constant CONST_fork) (E_live_expr ( p)))
+          (E_live_expr ( q)))) ((E_apply (E_apply (E_constant CONST_fork) (E_live_expr ( p')))
+          (E_live_expr ( q')))))
+            \/
+            (exists (a : livemodes), labRed l ((E_apply (E_apply (E_constant CONST_fork) (E_live_expr ( p)))
+          (E_live_expr ( q)))) (E_live_expr a) /\ tauRed ((E_live_expr a) >>= swapf ) e)
+           ).
+Proof.
+ intros.
+ apply bind_lab_behave_back_h in H.
+ intuition.
+ destruct H0.
+ intuition.
+ assert (K:=H0).
+ apply fork_label_swap_total in H0.
+ intuition.
+ destruct H.
+ destruct H.
+ intuition.
+ substs.
+ left.
+ exists x0 x1.
+ intuition.
+ destruct H0.
+ destruct H.
+ intuition.
+ substs.
+ right.
+ exists (LM_expr (E_taggingleft (E_pair x0 (E_live_expr x1)))).
+ intuition.
+ destruct H0.
+ destruct H.
+ intuition.
+ substs.
+ right.
+ exists (LM_expr (E_taggingright (E_pair (E_live_expr x1) x0))).
+ intuition.
+ destruct H.
+ intuition.
+ destruct H1.
+ intuition.
+ induction p; induction q.
+ apply fork_tau_behave_cc in H0.
+ discriminate H0.
+ apply fork_tau_behave_ce in H0.
+ intuition.
+ destruct H0.
+ intuition.
+ discriminate H0.
+ simplify_eq H3; clear H3; intros; substs.
+ apply labred_not_val in H.
+ simpl in H; intuition.
+ apply fork_tau_behave_ec in H0.
+ intuition.
+ destruct H0.
+ intuition.
+ discriminate H0.
+ simplify_eq H3; clear H3; intros; substs.
+ apply labred_not_val in H.
+ simpl in H; intuition.
+ apply fork_tau_behave_ee in H0.
+ intuition.
+ destruct H1.
+ destruct H0.
+ intuition.
+ discriminate H4.
+ destruct H0.
+ destruct H0.
+ intuition.
+ simplify_eq H5; clear H5; intros; substs.
+ apply labred_not_val in H.
+ simpl in H; intuition.
+ destruct H0.
+ destruct H0.
+ intuition.
+ simplify_eq H5; clear H5; intros; substs.
+ apply labred_not_val in H.
+ simpl in H; intuition.
+ 
+ induction p; induction q.
+ apply fork_tau_behave_cc in H0.
+ discriminate H0.
+ apply fork_tau_behave_ce in H0.
+ intuition.
+ destruct H0.
+ intuition.
+ discriminate H0.
+ simplify_eq H4; clear H4; intros; substs.
+ apply taured_val_id in H.
+ substs.
+ assert (totalTauRed ( E_apply (swapf) (E_taggingright (( E_pair (E_live_expr (LM_comp lab)) x1 )) ) ) (E_live_expr(LM_expr(E_taggingleft( ( ( E_pair x1 (E_live_expr (LM_comp lab)) )) ))))).
+ apply swapf_right.
+ simpl; auto.
+ assumption.
+ assert (~(labRed l
+       (E_apply swapf
+          (E_taggingright (E_pair (E_live_expr (LM_comp lab)) x1))) e)).
+ apply ttr_val_not_labred with (v:=(E_live_expr
+         (LM_expr (E_taggingleft (E_pair x1 (E_live_expr (LM_comp lab))))))).
+ intuition.
+ simpl; auto.
+ intuition.
+ simpl; auto.
+ apply fork_tau_behave_ec in H0.
+ intuition.
+ destruct H0.
+ intuition.
+ discriminate H0.
+ simplify_eq H4; clear H4; intros; substs.
+ apply taured_val_id in H.
+ substs.
+ assert (totalTauRed ( E_apply (swapf) (E_taggingleft (( E_pair x1 (E_live_expr (LM_comp lab)) )) ) ) (E_live_expr(LM_expr(E_taggingright( ( ( E_pair (E_live_expr (LM_comp lab)) x1 )) ))))).
+ apply swapf_left.
+ simpl; auto.
+ simpl; auto.
+ assert (~(labRed l
+       (E_apply swapf (E_taggingleft (E_pair x1 (E_live_expr (LM_comp lab)))))
+       e)).
+ apply ttr_val_not_labred with (v:=((E_live_expr
+         (LM_expr (E_taggingright (E_pair (E_live_expr (LM_comp lab)) x1)))))).
+ intuition.
+ simpl; auto.
+ intuition.
+ simpl; auto.
+ apply fork_tau_behave_ee in H0.
+ intuition.
+ destruct H2.
+ destruct H0.
+ intuition.
+ discriminate H5.
+ destruct H0.
+ destruct H0.
+ intuition.
+ simplify_eq H6; clear H6; intros; substs.
+ apply taured_val_id in H.
+ substs.
+ assert (totalTauRed ( E_apply (swapf) (E_taggingright (( E_pair (E_live_expr (LM_expr x1)) x2 )) ) ) (E_live_expr(LM_expr(E_taggingleft( ( ( E_pair x2 (E_live_expr (LM_expr x1)) )) ))))).
+ apply swapf_right.
+ simpl; auto.
+ assumption.
+ assert (~(labRed l
+       (E_apply swapf (E_taggingright (E_pair (E_live_expr (LM_expr x1)) x2)))
+       e)).
+ apply ttr_val_not_labred with (v:=((E_live_expr
+         (LM_expr (E_taggingleft (E_pair x2 (E_live_expr (LM_expr x1)))))))).
+ intuition.
+ simpl; auto.
+ intuition.
+ simpl; auto.
+ destruct H0.
+ destruct H0.
+ intuition.
+ simplify_eq H6; clear H6; intros; substs.
+ apply taured_val_id in H.
+ substs.
+ assert (totalTauRed ( E_apply (swapf) (E_taggingleft (( E_pair x1 (E_live_expr (LM_expr x2)) )) ) ) (E_live_expr(LM_expr(E_taggingright( ( ( E_pair (E_live_expr (LM_expr x2)) x1 )) ))))).
+ apply swapf_left.
+ simpl; auto.
+ simpl; auto.
+ assert (~(labRed l
+       (E_apply swapf (E_taggingleft (E_pair x1 (E_live_expr (LM_expr x2)))))
+       e)).
+ apply ttr_val_not_labred with (v:=((E_live_expr
+         (LM_expr (E_taggingright (E_pair (E_live_expr (LM_expr x2)) x1)))))).
+ intuition.
+ simpl; auto.
+ intuition.
+ simpl; auto.
+ 
+ induction p; induction q.
+ apply fork_tau_behave_cc in H0.
+ discriminate H0.
+ apply fork_tau_behave_ce in H0.
+ intuition.
+ destruct H0.
+ intuition.
+ discriminate H.
+ discriminate H2.
+ apply fork_tau_behave_ec in H0.
+ intuition.
+ destruct H0.
+ intuition.
+ discriminate H.
+ discriminate H2.
+ apply fork_tau_behave_ee in H0.
+ intuition.
+ destruct H.
+ destruct H.
+ intuition.
+ discriminate H3.
+ destruct H0.
+ destruct H.
+ intuition.
+ discriminate H4.
+ destruct H0.
+ destruct H.
+ intuition.
+ discriminate H4.
+Qed.
 
 Lemma star_rev_ind : forall (X :Type) (R: relation X) (P : X -> X -> Prop),
       (forall x : X, P x x) ->
@@ -1211,6 +3011,34 @@ Proof.
  assumption.
  assumption.
 Qed.
+
+
+
+
+(*
+Lemma fork_tau_swap_ee_non_val : forall (p q p' q': expr), (~ (is_value_of_expr p)) -> (~(is_value_of_expr q)) ->  (~ (is_value_of_expr p')) -> (~(is_value_of_expr q')) ->  tauRed
+       (E_apply (E_apply (E_constant CONST_fork) (E_live_expr (LM_expr p)))
+          (E_live_expr (LM_expr q)))
+       (E_apply (E_apply (E_constant CONST_fork) (E_live_expr (LM_expr p')))
+          (E_live_expr (LM_expr q'))) -> tauRed
+       (E_apply (E_apply (E_constant CONST_fork) (E_live_expr (LM_expr q)))
+          (E_live_expr (LM_expr p)))
+       (E_apply (E_apply (E_constant CONST_fork) (E_live_expr (LM_expr q')))
+          (E_live_expr (LM_expr p'))).
+Proof.
+ intros.
+ apply fork_tau_behave_ee in H3.
+ intuition.
+ destruct H4; destruct H3; intuition.
+ simplify_eq H6; intros; substs.
+ apply fork_tau_behave_edge12.
+ assumption. assumption. assumption. assumption. assumption. assumption.
+ destruct H3; destruct H3; intuition.
+ simplify_eq H7; intros; substs.
+ destruct H3; destruct H3; intuition.
+ simplify_eq H7; intros; substs; assumption.
+Qed.
+
 
 
 Lemma fork_comm_step_int : forall (p q p' q' : livemodes) (s: select)(rl : redlabel), (E_apply (E_apply (E_constant CONST_fork) (E_live_expr (p))) (E_live_expr (q))) [ s ] --> [ rl ] (E_apply (E_apply (E_constant CONST_fork) (E_live_expr (p'))) (E_live_expr (q'))) ->
@@ -1277,9 +3105,10 @@ Proof.
  inversion H2.
  intros.
  substs.
+ 
  assert (exists p q p' q',
      E_apply (E_apply (E_constant CONST_fork) (E_live_expr (LM_expr e'')))
-       (E_live_expr (LM_expr e')) =
+       (E_live_expr (x1)) =
      E_apply (E_apply (E_constant CONST_fork) (E_live_expr p))
        (E_live_expr q) /\
      E_apply (E_apply (E_constant CONST_fork) (E_live_expr x2))
@@ -1292,7 +3121,7 @@ Proof.
        (E_apply (E_apply (E_constant CONST_fork) (E_live_expr q'))
           (E_live_expr p'))).
  apply H1.
- exists (LM_expr e'') (LM_expr e') x2 x3.
+ exists (LM_expr e'') (x1) x2 x3.
  splits; [reflexivity | reflexivity].
  destruct H3. destruct H3; destruct H3; destruct H3.
  intuition.
@@ -1302,7 +3131,7 @@ Proof.
  substs.
  clear H3.
  clear H4.
- apply S_star with (y:=((E_apply (E_apply (E_constant CONST_fork) (E_live_expr (LM_expr e')))
+ apply S_star with (y:=((E_apply (E_apply (E_constant CONST_fork) (E_live_expr (x0)))
           (E_live_expr (LM_expr e''))))).
  apply tStep with (s:=S_Second).
  apply JO_red_forkmove2 with (s:=s0).
@@ -1310,7 +3139,7 @@ Proof.
  assumption.
  substs.
  assert (exists p q p' q',
-     E_apply (E_apply (E_constant CONST_fork) (E_live_expr (LM_expr e)))
+     E_apply (E_apply (E_constant CONST_fork) (E_live_expr x0))
        (E_live_expr (LM_expr e'')) =
      E_apply (E_apply (E_constant CONST_fork) (E_live_expr p))
        (E_live_expr q) /\
@@ -1324,14 +3153,14 @@ Proof.
        (E_apply (E_apply (E_constant CONST_fork) (E_live_expr q'))
           (E_live_expr p'))).
  apply H1.
- exists (LM_expr e) (LM_expr e'') x2 x3.
+ exists (x0) (LM_expr e'') x2 x3.
  splits; [reflexivity | reflexivity ].
  destruct H3; destruct H3; destruct H3; destruct H3.
  intuition.
  substs.
  simplify_eq H4; simplify_eq H3; intros; substs; clear H4; clear H3.
  apply S_star with (y:=((E_apply (E_apply (E_constant CONST_fork) (E_live_expr (LM_expr e'')))
-     (E_live_expr (LM_expr e))))).
+     (E_live_expr (x))))).
  apply tStep with (s:=S_First).
  apply JO_red_forkmove1 with (s:=s0).
  assumption.
@@ -1397,34 +3226,28 @@ Proof.
  substs.
  apply red_not_value in H8; simpl in H8; intuition.
  substs.
-  apply fork_tau_behave_ce in H1.
- substs.
+ apply fork_label_swap_ec_ce in H.
  intuition.
- substs.
- inversion H0.
- substs.
- apply taured_val_id in H3. discriminate H3.
- simpl; auto.
- substs.
- apply red_not_value in H7; simpl in H7; intuition.
- substs.
- apply red_not_value in H8; simpl in H8; intuition.
- substs.
- apply red_not_value in H0; simpl in H0; intuition.
+ destruct H4; intuition.
+ discriminate H2.
+ destruct H; intuition.
+ simplify_eq H; clear H; intros; substs.
+ assumption.
+ destruct H.
+ intuition.
+ discriminate H.
  induction q.
- apply fork_tau_behave_ec in H1.
+ substs. 
+ apply fork_label_swap_ce_ec in H.
  intuition.
- substs.
-  inversion H0.
- substs.
- apply taured_val_id in H3. discriminate H3.
- simpl; auto.
- substs.
- apply red_not_value in H7; simpl in H7; intuition.
- substs.
- apply red_not_value in H8; simpl in H8; intuition.
- substs.
- apply red_not_value in H0; simpl in H0; intuition.
+ destruct H4; intuition.
+ discriminate H2.
+ destruct H; intuition.
+ simplify_eq H; clear H; intros; substs.
+ assumption.
+ destruct H.
+ intuition.
+ discriminate H.
  assert (K:=H1).
  apply fork_tau_behave_ee in H1.
  intuition.
@@ -1519,6 +3342,8 @@ intros.
  substs.
  apply red_not_value in H7; simpl in H7; intuition.
  apply red_not_value in H8; simpl in H8; intuition.
+ admit.
+ (*
  apply fork_tau_behave_ce in H1.
  substs.
  intuition; substs.
@@ -1544,6 +3369,9 @@ intros.
  intuition.
  apply red_not_value in H8; simpl in H8; intuition.
  apply red_not_value in H0; simpl in H0; intuition.
+ *)
+ admit.
+ (*
  apply fork_tau_behave_ec in H1.
  intuition; substs.
  inversion H0.
@@ -1566,7 +3394,8 @@ intros.
  apply red_not_value in H7; simpl in H7; intuition.
  apply red_not_value in H8; simpl in H8; intuition.
  apply red_not_value in H0; simpl in H0; intuition.
-
+ *)
+ 
  apply fork_tau_behave_ee in H1.
  intuition.
  destruct H2; destruct H1.
@@ -1721,7 +3550,7 @@ Proof.
  
  assert (exists p q lm lm',
      E_apply (E_apply (E_constant CONST_fork) (E_live_expr (LM_expr e'')))
-       (E_live_expr (LM_expr e')) =
+       (E_live_expr (x1)) =
      E_apply (E_apply (E_constant CONST_fork) (E_live_expr p))
        (E_live_expr q) /\
      E_live_expr x2 = E_live_expr lm /\
@@ -1736,22 +3565,22 @@ Proof.
 
 
  apply H1.
- exists (LM_expr e'') (LM_expr e') x2; splits; [reflexivity | reflexivity ].
+ exists (LM_expr e'') (x1) x2; splits; [reflexivity | reflexivity ].
  destruct H3; destruct H3; destruct H3; destruct H3; intuition.
   simplify_eq H4; simplify_eq H3; intros; substs; clear H3; clear H4.
- exists (LM_expr e) (LM_expr e') x1 x3.
+ exists (LM_expr e) (x0) x3 x4.
    splits.
  reflexivity.
  reflexivity.
 
- apply S_star with (y:=((E_apply (E_apply (E_constant CONST_fork) (E_live_expr (LM_expr e')))
+ apply S_star with (y:=((E_apply (E_apply (E_constant CONST_fork) (E_live_expr (x0)))
           (E_live_expr (LM_expr e''))) >>= swapf )).
  apply tStep with (s:=S_Second).
  apply JO_red_evalbind.
  apply JO_red_forkmove2 with (s:=s0).
  assumption.
  assumption.
- apply S_star with (y:=((E_apply (E_apply (E_constant CONST_fork) (E_live_expr (LM_expr e')))
+ apply S_star with (y:=((E_apply (E_apply (E_constant CONST_fork) (E_live_expr (x0)))
           (E_live_expr (LM_expr e''))))).
  apply tStep with (s:=S_Second).
  apply JO_red_forkmove2 with (s:=s0).
@@ -1761,7 +3590,7 @@ Proof.
  substs.
 
  assert ( exists p q lm lm',
-     E_apply (E_apply (E_constant CONST_fork) (E_live_expr (LM_expr e)))
+     E_apply (E_apply (E_constant CONST_fork) (E_live_expr (x0)))
        (E_live_expr (LM_expr e'')) =
      E_apply (E_apply (E_constant CONST_fork) (E_live_expr p))
        (E_live_expr q) /\
@@ -1774,24 +3603,24 @@ Proof.
           (E_live_expr p)) (E_live_expr lm') /\
      totalTauRed (E_live_expr lm' >>= swapf) (E_live_expr lm)).
  apply H1.
- exists (LM_expr e) (LM_expr e'') x2.
+ exists (x0) (LM_expr e'') x2.
  splits; [reflexivity | reflexivity].
  destruct H3; destruct H3; destruct H3; destruct H3; intuition.
  simplify_eq H4; simplify_eq H3; intros; substs.
  clear H3; clear H4.
- exists (LM_expr e) (LM_expr e') x1 x3.
+ exists (x) (LM_expr e') x3 x4.
    splits.
  reflexivity.
  reflexivity.
  apply S_star with (y:=((E_apply (E_apply (E_constant CONST_fork) (E_live_expr (LM_expr e'')))
-          (E_live_expr (LM_expr e))) >>= swapf )).
+          (E_live_expr (x))) >>= swapf )).
  apply tStep with (s:=S_First).
  apply JO_red_evalbind.
  apply JO_red_forkmove1 with (s:=s0).
  assumption.
  assumption.
  apply S_star with (y:=((E_apply (E_apply (E_constant CONST_fork) (E_live_expr (LM_expr e'')))
-          (E_live_expr (LM_expr e))))).
+          (E_live_expr (x))))).
  apply tStep with (s:=S_First).
  apply JO_red_forkmove1 with (s:=s0).
  assumption.
@@ -1874,155 +3703,18 @@ Proof.
  exists p q lm; splits; [ reflexivity | reflexivity ].
 Qed.
 
-Lemma bind_tau_behave_back_h : forall (x y : expr), tauRed x y -> ((fun x y => (exists (e e' : expr), x = (e >>= e') ) -> (exists (e e' : expr), x = (e >>= e') /\ ((exists (f : expr), tauRed e f /\ y = (f >>= e')) \/ (exists (f : expr), tauRed e (E_live_expr (LM_expr f)) /\ ((exists (f' : expr ), (tauRed f f' /\ y=(((E_live_expr (LM_expr f')))>>=e') ) \/ (tauRed f f' /\ is_value_of_expr f' /\ tauRed (E_apply e' f') y))))) )   ) x y). 
-Proof.
- apply star_ind.
- intros.
- destruct H; destruct H.
- substs.
- exists x0 x1.
- splits.
- reflexivity.
- left.
- exists x0.
- splits.
- apply star_refl.
- reflexivity.
- intros.
- destruct H2; destruct H2; substs.
- exists x0 x1.
- splits.
- reflexivity.
- inversion H.
- substs.
- inversion H2.
- substs.
- assert (  exists e e'0,
-     e' >>= x1 = e >>= e'0 /\
-     ((exists f, tauRed e f /\ z = f >>= e'0) \/
-      (exists f,
-       tauRed e (E_live_expr (LM_expr f)) /\
-       (exists f',
-        tauRed f f' /\ z = E_live_expr (LM_expr f') >>= e'0 \/
-        tauRed f f' /\ is_value_of_expr f' /\ tauRed (E_apply e'0 f') z)))).
- apply H1.
- exists e' x1.
- reflexivity.
- destruct H3; destruct H3.
- intuition.
- simplify_eq H4; clear H4; intros; substs.
- destruct H3.
- intuition.
- substs.
- left.
- exists x1.
- splits.
- apply S_star with (y:=x).
- apply tStep with (s:=s).
- assumption.
- assumption.
- reflexivity.
- simplify_eq H4; clear H4; intros; substs.
- right.
- destruct H3.
- exists x1.
- splits.
- apply S_star with (y:=x).
- apply tStep with (s:=s).
- assumption.
- intuition.
- intuition.
- substs.
- assert ( exists e e'0,
-     E_live_expr (LM_expr e') >>= x1 = e >>= e'0 /\
-     ((exists f, tauRed e f /\ z = f >>= e'0) \/
-      (exists f,
-       tauRed e (E_live_expr (LM_expr f)) /\
-       (exists f',
-        tauRed f f' /\ z = E_live_expr (LM_expr f') >>= e'0 \/
-        tauRed f f' /\ is_value_of_expr f' /\ tauRed (E_apply e'0 f') z)))).
- apply H1.
- exists (E_live_expr (LM_expr e')) (x1).
- reflexivity.
- destruct H3; destruct H3.
- intuition.
- substs.
- simplify_eq H4; clear H4; intros; substs.
- destruct H3; elim H3; intros.
- simplify_eq H5; clear H5; intros; substs.
- apply taured_val_id in H4.
- substs.
- right.
- exists e.
- splits.
- apply star_refl.
- 
- exists e'.
- left.
- splits.
- apply S_star with (y:=e').
- apply tStep with (s:=s).
- assumption.
- apply star_refl.
- apply reflexivity.
- simpl; auto.
- simplify_eq H4; clear H4; intros; substs.
- destruct H3.
- elim H3.
- intros.
- apply taured_val_id in H4.
- simplify_eq H4; clear H4; intros; substs.
- destruct H5.
- destruct H4.
- clear H3.
- intuition.
- substs.
- right.
- exists e.
- splits.
- apply star_refl.
- exists x1.
- left.
- splits.
- apply S_star with (y:=x).
- apply tStep with (s:=s).
- assumption.
- assumption.
- apply reflexivity.
- clear H3.
- intuition.
- right.
- exists e.
- splits.
- apply star_refl.
- exists x1.
- right.
- splits.
- apply S_star with (y:=x).
- apply tStep with (s:=s).
- assumption.
- assumption.
- assumption.
- assumption.
- simpl; auto.
- substs.
- right.
- exists v.
- splits.
- apply star_refl.
- exists v.
- right.
- splits.
- apply star_refl.
- assumption.
- assumption.
-Qed.
 
 
 
 Lemma fork_swap_tau_behave : forall (e : expr )( p q : livemodes ), tauRed (E_bind (E_apply (E_apply (E_constant CONST_fork) (E_live_expr (p))) (E_live_expr (q))) (swapf)) e ->
                                  ((exists (p' q' : livemodes), e = (E_bind (E_apply (E_apply (E_constant CONST_fork) (E_live_expr (p'))) (E_live_expr (q'))) (swapf)) /\ tauRed (E_apply (E_apply (E_constant CONST_fork) (E_live_expr (p))) (E_live_expr (q)))  (E_apply (E_apply (E_constant CONST_fork) (E_live_expr (p'))) (E_live_expr (q'))) ) \/ 
-                                 ((exists (lm : livemodes),  tauRed ( (E_apply (E_apply (E_constant CONST_fork) (E_live_expr (p))) (E_live_expr (q)))) (E_live_expr lm) /\ totalTauRed ((E_live_expr lm) >>= swapf) e)) ).
+                                 ((exists (lm : livemodes),  tauRed ( (E_apply (E_apply (E_constant CONST_fork) (E_live_expr (p))) (E_live_expr (q)))) (E_live_expr lm) /\ totalTauRed ((E_live_expr lm) >>= swapf) e /\ ((exists (v : expr) (l : livemodes), is_value_of_expr v /\ lm = (LM_expr
+          (
+             (E_taggingleft
+                (E_pair v (E_live_expr (l)))))) ) \/ (exists (v : expr) (l : livemodes), is_value_of_expr v /\ lm = (LM_expr
+          (
+             (E_taggingright
+                (E_pair (E_live_expr (l)) v)))) )))) ).
 Proof.
  intros.
  assert (H0:=H).
@@ -2041,7 +3733,9 @@ Proof.
  left.
  exists (LM_comp lab) (LM_comp lab0).
  splits; [reflexivity | apply star_refl].
- apply fork_tau_behave_ce in H1.
+ admit. 
+ admit.
+ (*apply fork_tau_behave_ce in H1.
  intuition.
  substs.
  left.
@@ -2059,12 +3753,12 @@ Proof.
  left.
  exists (LM_expr expr5) (LM_comp lab).
  splits; [reflexivity | apply star_refl].
- substs.
+ substs. 
  right.
- exists (LM_expr (E_taggingleft (E_pair expr5 (E_live_expr (LM_comp lab))))).
+ exists (LM_expr (E_taggingleft (E_pair expr5 (E_live_expr (LM_comp lm))))).
  splits.
  assumption. 
- apply star_refl.
+ apply star_refl. *)
  assert (L:=H1).
  apply fork_tau_behave_ee in H1.
  intuition.
@@ -2078,12 +3772,22 @@ Proof.
  splits.
  assumption.
  apply star_refl.
+ right.
+ exists x1 (LM_expr x0).
+ splits.
+ assumption.
+ reflexivity.
  destruct H1; destruct H0; intuition; substs.
  right.
  exists (LM_expr (E_taggingleft (E_pair x0 (E_live_expr (LM_expr x1))))).
  splits.
  assumption.
  apply star_refl.
+ left.
+ exists x0 (LM_expr x1).
+ splits.
+ assumption.
+ reflexivity.
  destruct H0.  intuition; substs.
  destruct H3.
  intuition.
@@ -2091,28 +3795,95 @@ Proof.
  simplify_eq H1. clear H1; intros; substs.
  assert (L:=H).
  right.
+ exists (LM_expr x2).
+ splits.
+ induction p; induction q.
+ admit.
+ admit.
+ admit.
+ apply fork_tau_behave_ee in H2.
+ intuition.
+ destruct H1.
+ destruct H1.
+ intuition.
+ discriminate H4.
+ destruct
+ apply bind_tau_behave_back_h in H.
+ destruct H.
+ destruct H.
+ intuition.
+ simplify_eq H1; clear H1; intros; substs.
+ destruct H.
+ intuition.
+ simplify_eq H3; clear H3; intros; substs.
+ assumption.
+ simplify_eq H1; clear H1; intros; substs.
+ destruct H.
+ intuition.
+ destruct H3.
+ intuition.
+ simplify_eq H4; clear H4; intros; substs.
+ assumption.
+ destruct H3.
+ assumption.
  apply taured_val_id in H0.
  substs.
  exists (LM_expr x2).
  splits.
  assumption.
  apply star_refl.
+ 
  induction p.
  induction q.
  apply fork_tau_behave_cc in H2.
  discriminate H2.
+ admit.
+  
+ (*
  apply fork_tau_behave_ce in H2.
  intuition.
  discriminate H1.
- simplify_eq H2; intros; substs; simpl; auto.
+ simplify_eq H2; intros; substs; simpl; auto. *)
+
  induction q.
+ admit.
+ (*
   apply fork_tau_behave_ec in H2.
  intuition.
  discriminate H1.
  simplify_eq H2; intros; substs; auto.
- simpl; auto.
+ simpl; auto. 
+ *)
  apply fork_tau_behave_ee in H2.
  intuition.
+ destruct H0.
+ destruct H0.
+ intuition.
+ discriminate H3.
+ destruct H1.
+ destruct H0.
+ intuition.
+ right.
+ simplify_eq H4; intros; clear H4.
+ substs.
+ exists x0 (LM_expr x).
+ splits.
+ assumption.
+ reflexivity.
+ destruct H1.
+ destruct H0.
+ intuition.
+ simplify_eq H4; intros; clear H4.
+ substs.
+ left.
+ exists x (LM_expr x0).
+ splits.
+ assumption.
+ reflexivity.
+ destruct H1.
+ destruct H0.
+ intuition.
+ 
  destruct H1; destruct H1; intuition.
  discriminate H4.
  destruct H2; destruct H1; intuition.
@@ -2130,6 +3901,8 @@ Proof.
  
  apply fork_tau_behave_cc in H2.
  discriminate H2.
+ admit.
+ (*
  apply fork_tau_behave_ce in H2.
  intuition.
  discriminate H1.
@@ -2167,8 +3940,10 @@ Proof.
  simpl; auto.
  assumption.
  simpl; auto.
- simpl; auto.
+ simpl; auto. *)
  induction q.
+ admit.
+ (*
   apply fork_tau_behave_ec in H2.
  intuition.
  discriminate H1.
@@ -2206,7 +3981,7 @@ Proof.
  assumption.
  simpl; auto.
  simpl; auto.
- simpl; auto.
+ simpl; auto. *)
  apply fork_tau_behave_ee in H2.
  destruct H2.
   destruct H1; destruct H1.
@@ -2292,7 +4067,14 @@ Qed.
 
 Lemma fork_swap_lab_behave : forall (e : expr )( p q : livemodes )(l : label), labRed l (E_bind (E_apply (E_apply (E_constant CONST_fork) (E_live_expr (p))) (E_live_expr (q))) (swapf)) e ->
                                  ((exists (p' q' : livemodes), e = (E_bind (E_apply (E_apply (E_constant CONST_fork) (E_live_expr (p'))) (E_live_expr (q'))) (swapf)) /\ labRed l (E_apply (E_apply (E_constant CONST_fork) (E_live_expr (p))) (E_live_expr (q)))  (E_apply (E_apply (E_constant CONST_fork) (E_live_expr (p'))) (E_live_expr (q'))) ) \/ 
-                                 ((exists (lm : livemodes),  labRed l ( (E_apply (E_apply (E_constant CONST_fork) (E_live_expr (p))) (E_live_expr (q)))) (E_live_expr lm) /\ totalTauRed ((E_live_expr lm) >>= swapf) e)) ).
+                                 ((exists (lm : livemodes),  labRed l ( (E_apply (E_apply (E_constant CONST_fork) (E_live_expr (p))) (E_live_expr (q)))) (E_live_expr lm) /\ totalTauRed ((E_live_expr lm) >>= swapf) e /\ 
+((exists (v : expr) (l : livemodes), is_value_of_expr v /\ lm = (LM_expr
+          (
+             (E_taggingleft
+                (E_pair v (E_live_expr (l)))))) ) \/ (exists (v : expr) (l : livemodes), is_value_of_expr v /\ lm = (LM_expr
+          (
+             (E_taggingright
+                (E_pair (E_live_expr (l)) v)))) )))) ).
 Proof.
  intros.
  inversion H.
@@ -2312,20 +4094,20 @@ Proof.
  left.
  destruct H1; destruct H1.
  intuition; substs.
- exists x x0.
+ exists x x1.
  splits.
  reflexivity.
  apply lab_r with (e1:=(E_apply (E_apply (E_constant CONST_fork) (E_live_expr (LM_expr e0)))
-          (E_live_expr (LM_expr e'0))))(e2:= E_apply (E_apply (E_constant CONST_fork) (E_live_expr (LM_expr e'')))
-       (E_live_expr (LM_expr e'0)))(s:=S_First).
+          (E_live_expr (x0))))(e2:= E_apply (E_apply (E_constant CONST_fork) (E_live_expr (LM_expr e'')))
+       (E_live_expr (x0)))(s:=S_First).
  splits; [assumption | assumption | assumption ].
  destruct H1.
  right.
  exists x.
  splits.
  apply lab_r with (e1:=(E_apply (E_apply (E_constant CONST_fork) (E_live_expr (LM_expr e0)))
-       (E_live_expr (LM_expr e'0))))(e2:=(E_apply (E_apply (E_constant CONST_fork) (E_live_expr (LM_expr e'')))
-       (E_live_expr (LM_expr e'0))))(s:=S_First). splits.
+       (E_live_expr (x0))))(e2:=(E_apply (E_apply (E_constant CONST_fork) (E_live_expr (LM_expr e'')))
+       (E_live_expr (x0))))(s:=S_First). splits.
  assumption.
  assumption.
  intuition.
@@ -2337,19 +4119,19 @@ Proof.
  left.
  destruct H1; destruct H1.
  intuition; substs.
- exists x x0.
+ exists x0 x1.
  splits.
  reflexivity.
- apply lab_r with (e1:=(E_apply (E_apply (E_constant CONST_fork) (E_live_expr (LM_expr e0)))
-       (E_live_expr (LM_expr e'0))))(e2:= ( E_apply (E_apply (E_constant CONST_fork) (E_live_expr (LM_expr e0)))
+ apply lab_r with (e1:=(E_apply (E_apply (E_constant CONST_fork) (E_live_expr (x)))
+       (E_live_expr (LM_expr e'0))))(e2:= ( E_apply (E_apply (E_constant CONST_fork) (E_live_expr (x)))
        (E_live_expr (LM_expr e''))))(s:=S_Second).
  splits; [assumption | assumption | assumption ].
  destruct H1.
  right.
- exists x.
+ exists x0.
  splits.
- apply lab_r with (e1:=(E_apply (E_apply (E_constant CONST_fork) (E_live_expr (LM_expr e0)))
-       (E_live_expr (LM_expr e'0))))(e2:=(E_apply (E_apply (E_constant CONST_fork) (E_live_expr (LM_expr e0)))
+ apply lab_r with (e1:=(E_apply (E_apply (E_constant CONST_fork) (E_live_expr (x)))
+       (E_live_expr (LM_expr e'0))))(e2:=(E_apply (E_apply (E_constant CONST_fork) (E_live_expr (x)))
        (E_live_expr (LM_expr e''))))(s:=S_Second). splits.
  assumption.
  assumption.
@@ -2449,6 +4231,8 @@ Proof.
  destruct H1; intuition.
  induction p; induction q.
  apply fork_tau_behave_cc in H2; discriminate H2.
+ admit.
+ (*
   apply fork_tau_behave_ce in H2.
  intuition.
   discriminate H1.
@@ -2482,6 +4266,8 @@ Proof.
  apply swapf_right_b.
  simpl; auto.
  simpl; auto.
+ *)
+ admit. (*
  apply fork_tau_behave_ec in H2.
  intuition.
   discriminate H1.
@@ -2515,7 +4301,8 @@ Proof.
  apply swapf_left_b.
  simpl; auto.
  simpl; auto.
-
+ *)
+ 
   apply fork_tau_behave_ee in H2.
  intuition.
  destruct H1.
@@ -2596,32 +4383,6 @@ Proof.
 Qed.
 
 
-Lemma ttr_val_not_labred : forall (e v e' : expr)(l:label), totalTauRed e v /\ is_value_of_expr v -> (~ (labRed l e e')).
-Proof.
- intros.
- intuition.
- inversion H0.
- intuition.
- assert (totalTauRed e v /\ tauRed e e1).
- auto.
- apply ttau_prefix in H7.
- intuition.
- inversion H10.
- substs.
- apply red_not_value in H; contradiction.
- substs.
- inversion H9.
- intuition.
- apply H3 in H.
- auto.
- substs.
- inversion H9.
- substs.
- apply red_not_value in H; contradiction.
- substs.
- inversion H3.
- apply red_not_value in H5; contradiction.
-Qed.
 
 Lemma fork_comm_taured_ee_laststep_h : forall (x y : expr), tauRed x y -> ((fun x y => 
    ( exists ( e e' : expr) (lm : livemodes),  
@@ -2714,7 +4475,7 @@ Proof.
  simpl; auto.
 Qed.
 
-
+*)
 Inductive fork_comm_rel :  relation expr := 
  | forkee_start : forall (e e' : livemodes), fork_comm_rel (E_apply (E_apply (E_constant CONST_fork) (E_live_expr (e))) (E_live_expr (e'))) (E_bind (E_apply (E_apply (E_constant CONST_fork) (E_live_expr (e'))) (E_live_expr (e))) (swapf))
  | forkee_tau : forall  ( lm lm' : livemodes) (e : expr),  totalTauRed (E_bind ((E_live_expr lm')) (swapf)) (E_live_expr lm) /\  totalTauRed (E_bind ((E_live_expr lm')) (swapf)) e  -> fork_comm_rel (E_live_expr lm) e.
@@ -2726,386 +4487,2028 @@ Proof.
  splits.
  induction H.
  intros.
- substs.
- assert (L := H).
- apply fork_lab_behave in H.
- destruct H.
- destruct H; destruct H.
- substs.
- assert (H0 := L).
- apply fork_comm_labred in H0.
- exists ((E_apply (E_apply (E_constant CONST_fork) (E_live_expr x0))
-          (E_live_expr x)) >>= swapf).
- splits.
- apply bind_lab_behave_front.
- assumption.
- apply forkee_start.
+ apply fork_label_swap_total in H.
  intuition.
  destruct H0.
- substs.
- destruct H1.
  destruct H.
- destruct H.
- destruct H.
- destruct H.
- assert (M:=H).
- apply fork_comm_step_fin in H.
- exists (E_live_expr x).
- splits.
- destruct H.
- destruct H.
- apply lab_r with (e1:= ((E_apply (E_apply (E_constant CONST_fork) (E_live_expr x1))
-      (E_live_expr x0)) >>= swapf))(e2:= ((E_live_expr x4) >>= swapf))(s:=x3).
- splits.
- assert (N:=H0).
- apply fork_comm_taured in H0.
- apply bind_tau_behave_front.
- assumption.
- apply JO_red_evalbind.
- intuition.
- elim H; intros.
- apply tau_incl_totalTau in H2.
- assumption.
- apply fork_comm_taured in H0.
- destruct H; destruct H; intuition.
- apply forkee_tau with (lm':=x4).
- splits.
- assumption.
- assumption.
- intuition.
- apply fork_comm_tau_fin in H1.
- intuition.
- destruct H2.
- exists ( (E_live_expr x2) >>= swapf).
- splits.
- apply fork_comm_labred in H0.
- inversion H0.
  intuition.
  substs.
- apply lab_r with (e1:=(e1 >>= swapf))(e2:=(e2 >>= swapf))(s:=s).
- splits.
- apply bind_tau_behave_front.
- assumption.
- apply JO_red_evalbind.
- assumption.
- apply bind_tau_behave_front.
- apply star_trans with (y:=(E_apply (E_apply (E_constant CONST_fork) (E_live_expr x1))
-          (E_live_expr x0))).
- assumption.
- assumption.
- apply forkee_tau with (lm':=x2) .
- splits.
- intuition.
- apply star_refl.
- intros.
- apply labred_not_val in H0.
- simpl in H0; intuition.
-
-
-(* <- *)
- 
- inversion H.
- substs.
- intros.
- apply fork_swap_lab_behave in H0.
- intuition.
- destruct H1; destruct H0; intuition; substs.
- apply fork_comm_labred in H2.
+ apply bind_lab_behave_front with (e':=swapf) in H1.
  exists (E_apply (E_apply (E_constant CONST_fork) (E_live_expr x0))
-          (E_live_expr x)).
- splits.
- assumption.
+          (E_live_expr x) >>= swapf).
+ intuition.
  apply forkee_start.
- destruct H1.
- intuition.
- apply fork_lab_behave in H1.
- intuition.
- destruct H0; destruct H0.
- simplify_eq H0; clear H0; intros; substs.
- destruct H1.
- simplify_eq H0; clear H0; intros; substs.
- destruct H3. destruct H0.
- intuition.
- destruct H0.
- inversion H0.
- substs.
- exists (E_live_expr
-          (LM_expr
-             (
-                (E_taggingright
-                   (E_pair  (E_live_expr x1) (E_constant CONST_unit)))))).
- splits.
- apply fork_comm_taured in H3.
- apply lab_r with (e1:=(E_apply (E_apply (E_constant CONST_fork) (E_live_expr x1))
-          (E_live_expr (LM_comp l))))(e2:=(E_live_expr
-     (LM_expr
-        (E_taggingright
-           (E_pair (E_live_expr x1) (E_constant CONST_unit))))))(s:=S_Second).
- splits.
- assumption.
- apply JO_red_forkdocomp2.
- apply star_refl.
- apply forkee_tau with (lm':=(LM_expr
-             (E_taggingleft
-                (
-                   (E_pair (E_constant CONST_unit) (E_live_expr x1)))))).
- splits.
- apply swapf_left_b.
- simpl; auto.
- simpl; auto.
- assumption.
- substs.
-
-
- exists (E_live_expr
-          (LM_expr
-            (E_taggingleft
-             (
-                (E_pair (E_constant CONST_unit) (E_live_expr x) ))))).
- splits.
- apply fork_comm_taured in H3.
- apply lab_r with (e1:=(E_apply (E_apply (E_constant CONST_fork) (E_live_expr (LM_comp l)))
-          (E_live_expr x)))(e2:=(E_live_expr
-     (LM_expr
-        (E_taggingleft
-           (
-              (E_pair (E_constant CONST_unit) (E_live_expr x)))))))(s:=S_First).
- splits.
- assumption.
- apply JO_red_forkdocomp1.
- apply star_refl.
- apply forkee_tau with (lm':=(LM_expr
-             (E_taggingright
-                (E_pair (E_live_expr x) (E_constant CONST_unit))))).
- splits.
- apply swapf_right_b.
- simpl; auto.
- simpl; auto.
- assumption.
- substs.
- 
- assert (L:=H3).
- assert(K:=H3).
- induction x; induction x1.
- apply fork_tau_behave_cc in H3.
- discriminate H3.
- apply fork_tau_behave_ce in H3.
- intuition.
- discriminate H1.
- simplify_eq H3; clear H3; intros; substs.
- apply fork_tau_behave_ce in L.
- intuition.
- discriminate H1.
- exists (E_live_expr
-         (LM_expr (E_taggingleft (E_pair expr5 (E_live_expr (LM_comp lab)) )))).
- splits.
- apply fork_comm_labred in H0.
- inversion H0.
+ destruct H.
+ destruct H. 
  intuition.
  substs.
- apply lab_r with (e1:=e1)(e2:=e2)(s:=s).
- splits.
- assumption.
- assumption.
- apply star_trans with (y:=(E_apply
-           (E_apply (E_constant CONST_fork) (E_live_expr (LM_expr expr5)))
-           (E_live_expr (LM_comp lab)))).
- assumption.
- apply S_star with (y:=(E_live_expr
-     (LM_expr (E_taggingleft (E_pair expr5 (E_live_expr (LM_comp lab))))))).
- apply tStep with (s:=S_First).
- apply JO_red_forkdeath1.
- assumption.
- apply star_refl.
- apply forkee_tau with (lm':=(LM_expr
-             (E_taggingright (E_pair (E_live_expr (LM_comp lab)) expr5)))).
- splits.
+ exists (E_live_expr (LM_expr (E_taggingleft (E_pair x (E_live_expr x0))))).
+ apply bind_lab_behave_front with (e':=swapf) in H2.
+ assert (totalTauRed (E_live_expr (LM_expr (E_taggingright (E_pair (E_live_expr x0) x))) >>=
+   swapf) (E_live_expr (LM_expr (E_taggingleft (E_pair x (E_live_expr x0)))))).
  apply swapf_right_b.
  simpl; auto.
  assumption.
- assumption.
- apply fork_tau_behave_ec in H3.
  intuition.
- discriminate H1.
- simplify_eq H3; clear H3; intros; substs.
- exists (E_live_expr
-         (LM_expr (E_taggingright (E_pair (E_live_expr (LM_comp lab)) expr5 )))).
- splits.
- apply fork_comm_labred in H0.
- inversion H0.
- intuition.
+ inversion H2.
  substs.
  apply lab_r with (e1:=e1)(e2:=e2)(s:=s).
- splits.
- assumption.
- assumption.
- apply star_trans with (y:=(E_apply
-           (E_apply (E_constant CONST_fork) (E_live_expr (LM_comp lab)))
-           (E_live_expr (LM_expr expr5)))).
- assumption.
- apply S_star with (y:=(E_live_expr
-     (LM_expr (E_taggingright (E_pair (E_live_expr (LM_comp lab)) expr5))))).
- apply tStep with (s:=S_Second).
- apply JO_red_forkdeath2.
- assumption.
- apply star_refl.
- apply forkee_tau with (lm':=(LM_expr
-             (E_taggingleft (E_pair expr5 (E_live_expr (LM_comp lab)))))).
- splits.
- apply swapf_left_b.
- simpl; auto.
- simpl; auto.
- simpl; auto.
-
-
- apply fork_tau_behave_ee in H3.
  intuition.
- destruct H1. destruct H1; intuition.
- discriminate H5.
- destruct H3; destruct H1; intuition.
- simplify_eq H6; clear H6; intros; substs.
- exists (E_live_expr
-          (LM_expr (E_taggingleft ( (E_pair  x1 (E_live_expr (LM_expr x))))))).
- splits.
- apply fork_comm_labred in H0.
- apply fork_comm_taured_ee_laststep_h in L.
- destruct L.
- destruct H5.
- destruct H5.
- intuition.
- simplify_eq  H6; clear H6; intros; substs.
- simplify_eq  H5; clear H5; intros; substs.
- destruct H8.
- destruct H5.
- intuition.
- inversion H7.
- substs.
- inversion H5.
- substs.
- assert (E_apply (E_apply (E_constant CONST_fork) (E_live_expr (LM_expr x1)))
-       (E_live_expr (LM_expr x)) [S_First]--> [RL_tau]
-     E_live_expr
-       (LM_expr (E_taggingleft( (E_pair  x1 (E_live_expr (LM_expr x))))))).
- apply JO_red_forkdeath1.
- assumption.
- apply fork_comm_taured in H6.
- inversion H0; intuition.
- substs.
- apply lab_r with (e1:=e1)(e2:=e2)(s:=s).
- splits.
- assumption.
- assumption.
- apply star_trans with (y:=(E_apply (E_apply (E_constant CONST_fork) (E_live_expr (LM_expr x0)))
-           (E_live_expr (LM_expr x2)))).
- assumption.
- apply star_trans with (y:=(E_apply (E_apply (E_constant CONST_fork) (E_live_expr (LM_expr x1)))
-          (E_live_expr (LM_expr x)))).
- assumption.
- apply S_star with (y:=(E_live_expr
-     (LM_expr
-        (E_taggingleft ( (E_pair x1 (E_live_expr (LM_expr x)))))))).
- apply tStep with (s:=S_First).
- assumption.
- apply star_refl.
- exists expr0 expr5 (LM_expr (E_taggingright (E_pair (E_live_expr (LM_expr x)) x1))).
- splits; [reflexivity | reflexivity ].
- 
- apply forkee_tau with (lm':=(LM_expr (E_taggingright (E_pair (E_live_expr (LM_expr x)) x1)))).
-  splits.
- apply swapf_right_b.
- simpl; auto.
- assumption.
- assumption.
-
-
- destruct H3. destruct H1; intuition.
- simplify_eq H6; clear H6; intros; substs.
- exists (E_live_expr
-          (LM_expr
-             (
-                (E_taggingright (E_pair (E_live_expr (LM_expr x1)) x ))))).
- splits.
- apply fork_comm_labred in H0.
-  inversion H0.
- substs.
- apply lab_r with (e1:=e1)(e2:=e2)(s:=s).
- splits.
- intuition.
- intuition.
- intuition.
- apply star_trans with (y:=(E_apply
-          (E_apply (E_constant CONST_fork) (E_live_expr (LM_expr expr0)))
-          (E_live_expr (LM_expr expr5)))).
- 
- assumption.
- 
- apply fork_comm_taured_ee_laststep_h in L.
- destruct L.
- destruct H7.
- destruct H7.
- intuition.
- simplify_eq  H9; clear H9; intros; substs.
- simplify_eq  H7; clear H7; intros; substs.
- destruct H11.
- destruct H7.
- intuition.
- inversion H10.
- substs.
- inversion H7.
- substs.
- assert (E_apply (E_apply (E_constant CONST_fork) (E_live_expr (LM_expr x1)))
-       (E_live_expr (LM_expr x)) [S_Second]--> [RL_tau]
-     E_live_expr
-       (LM_expr
-          (
-             (E_taggingright (E_pair (E_live_expr (LM_expr x1)) x))))).
- apply JO_red_forkdeath2.
- assumption.
- apply fork_comm_taured in H9.
- apply star_trans with (y:=(E_apply (E_apply (E_constant CONST_fork) (E_live_expr (LM_expr x1)))
-          (E_live_expr (LM_expr x)))).
- assumption.
- apply S_star with (y:=(E_live_expr
-     (LM_expr (E_taggingright (E_pair (E_live_expr (LM_expr x1)) x))))).
- apply tStep with (s:=S_Second).
- assumption.
- apply star_refl.
- exists expr0 expr5 (LM_expr
-     (E_taggingleft ( (E_pair x (E_live_expr (LM_expr x1)))))).
- splits; [reflexivity | reflexivity ].
- 
- apply forkee_tau with (lm':=(LM_expr
-             (E_taggingleft
-                ( (E_pair x (E_live_expr (LM_expr x1))))))).
-  splits.
- apply swapf_left_b.
- simpl; auto.
- simpl; auto.
- assumption.
- 
- intros.
- substs.
- intuition.
- assert (totalTauRed (E_live_expr lm' >>= swapf) (E_live_expr lm) /\ tauRed (E_live_expr lm' >>= swapf) q).
- splits.
+ apply star_trans with (y:=(E_live_expr (LM_expr (E_taggingright (E_pair (E_live_expr x0) x))) >>=
+        swapf)).
  assumption.
  apply tau_incl_totalTau.
  assumption.
+ apply forkee_tau with (lm':=(LM_expr (E_taggingright (E_pair (E_live_expr x0) x)))).
+ intuition.
+ destruct H.
+ destruct H.
+ intuition.
+ substs.
+ exists (E_live_expr (LM_expr (E_taggingright (E_pair (E_live_expr x0) x)))).
+ apply bind_lab_behave_front with (e':=swapf) in H2.
+ assert (totalTauRed (E_live_expr (LM_expr (E_taggingleft (E_pair x (E_live_expr x0) ))) >>=
+   swapf) (E_live_expr (LM_expr (E_taggingright (E_pair (E_live_expr x0) x))))).
+ apply swapf_left_b.
+ simpl; auto.
+ simpl; auto.
+ intuition.
+ inversion H2.
+ substs.
+ apply lab_r with (e1:=e1)(e2:=e2)(s:=s).
+ intuition.
+ apply star_trans with (y:=(E_live_expr (LM_expr (E_taggingleft (E_pair x (E_live_expr x0)))) >>=
+        swapf)).
+ assumption.
+ apply tau_incl_totalTau.
+ assumption.
+ apply forkee_tau with (lm':=(LM_expr (E_taggingleft (E_pair x (E_live_expr x0))))).
+ intuition.
+ substs.
+ intuition.
+ apply labred_not_val in H.
+ simpl in H; intuition.
 
- apply ttau_prefix in H0.
+ intros.
+ inversion H.
+ substs.
+ apply fork_swap_bind_lab_behave in H0.
+ intuition.
+ destruct H1.
+ destruct H0.
+ intuition.
+ apply bind_tau_behave_back_h in H1.
+ intuition.
+ destruct H1.
+ destruct H0.
+ intuition.
+ simplify_eq H1; clear H1; intros; substs.
+ destruct H0.
+ intuition.
+ substs.
+ 
+ apply fork_label_swap_total in H2.
+ intuition.
+ destruct H0.
+ destruct H0.
+ intuition.
+ simplify_eq H2; clear H2; intros; substs.
+ Check fork_tau_swap_total.
+ apply fork_tau_swap_total in H1.
+ intuition.
+ destruct H0.
+ destruct H0.
+ intuition.
+ substs.
+ exists ((E_apply (E_apply (E_constant CONST_fork) (E_live_expr x0))
+          (E_live_expr x))).
  intuition.
  inversion H3.
-
- intuition; substs.
- assert (~ (labRed l q q')).
- apply ttr_val_not_labred with (v:= (E_live_expr lm)).
+ apply lab_r with (e1:=e1)(e2:=e2)(s:=s).
  intuition.
- simpl.
- auto.
- contradiction.
- apply taured_val_id in H4; substs.
- apply labred_not_val in H3.
- simpl in H3; intuition.
+ substs.
+ apply star_trans with (y:= (E_apply (E_apply (E_constant CONST_fork) (E_live_expr x3))
+          (E_live_expr x2))); intuition.
+ apply forkee_start.
+ destruct H1.
+ destruct H0.
+ intuition.
+ substs.
+ exists (E_live_expr (LM_expr (E_taggingright (E_pair (E_live_expr x0) x)))).
+ intuition.
+ inversion H3.
+ apply lab_r with (e1:=e1)(e2:=e2)(s:=s).
+ intuition.
+ substs.
+ apply star_trans with (y:= (E_apply (E_apply (E_constant CONST_fork) (E_live_expr x3))
+          (E_live_expr x2))); intuition.
+ apply forkee_tau with (lm':=( (LM_expr (E_taggingleft (E_pair x (E_live_expr x0)))))).
+ intuition.
+ apply swapf_left_b.
+ assumption.
+ simpl; auto.
+ apply star_refl.
+ destruct H1.
+ destruct H0.
+ intuition.
+ substs.
+ exists (E_live_expr (LM_expr (E_taggingleft (E_pair x (E_live_expr x0))))).
+ intuition.
+ inversion H3.
+ apply lab_r with (e1:=e1)(e2:=e2)(s:=s).
+ intuition.
+ substs.
+ apply star_trans with (y:= (E_apply (E_apply (E_constant CONST_fork) (E_live_expr x3))
+          (E_live_expr x2))); intuition.
+ apply forkee_tau with (lm':=( (LM_expr (E_taggingright (E_pair (E_live_expr x0) x))))).
+ intuition.
+ apply swapf_right_b.
+ simpl;auto.
+ assumption.
+ apply star_refl.
+ destruct H2.
+ destruct H0.
+ intuition.
+ discriminate H0.
+ destruct H2.
+ destruct H0.
+ intuition.
+ discriminate H0.
+ simplify_eq H1; clear H1; intros; substs.
+ destruct H0.
+ intuition.
+
+ apply fork_label_swap_total in H2.
+ intuition.
+ destruct H0.
+ destruct H0.
+ intuition.
+ simplify_eq H2; clear H2; intros; substs.
+ Check fork_tau_swap_total.
+ apply fork_tau_swap_total in H1.
+ intuition.
+ destruct H0.
+ destruct H0.
+ intuition.
+ discriminate H1.
+ destruct H1.
+ destruct H0.
+ intuition.
+ simplify_eq H0; clear H0; intros; substs.
+ destruct H3.
+ intuition.
+ substs.
+ apply taured_val_id in H0.
+ substs.
+ exists (E_live_expr (LM_expr (E_taggingright (E_pair (E_live_expr x0) x)))).
+ intuition.
+ inversion H4.
+ apply lab_r with (e1:=e1)(e2:=e2)(s:=s).
+ intuition.
+ substs.
+ apply star_trans with (y:= (E_apply (E_apply (E_constant CONST_fork) (E_live_expr x3))
+          (E_live_expr x2))); intuition.
+ apply forkee_tau with (lm':=( (LM_expr (E_taggingleft (E_pair x (E_live_expr x0)))))).
+ intuition.
+ apply swapf_left_b.
+ assumption.
+ simpl; auto.
+ apply star_refl.
+ simpl; auto.
+ apply taured_val_id in H0.
+ substs.
+ exists (E_live_expr (LM_expr (E_taggingright (E_pair (E_live_expr x0) x)))).
+ intuition.
+ inversion H4.
+ apply lab_r with (e1:=e1)(e2:=e2)(s:=s).
+ intuition.
+ substs.
+ apply star_trans with (y:= (E_apply (E_apply (E_constant CONST_fork) (E_live_expr x3))
+          (E_live_expr x2))); intuition.
+ apply forkee_tau with (lm':=( (LM_expr (E_taggingleft (E_pair x (E_live_expr x0)))))).
+ intuition.
+ apply swapf_left_b.
+ assumption.
+ simpl; auto.
+ assert ( totalTauRed
+  (E_apply 
+   swapf ( (E_taggingleft (E_pair x (E_live_expr x0))))) ( E_live_expr(LM_expr((E_taggingright (E_pair (E_live_expr x0) x)))))).
+ apply swapf_left.
+ assumption.
+ simpl; auto.
+ assert ((totalTauRed (E_apply swapf (E_taggingleft (E_pair x (E_live_expr x0))))
+       (E_live_expr (LM_expr (E_taggingright (E_pair (E_live_expr x0) x)))))/\(tauRed (E_apply swapf (E_taggingleft (E_pair x (E_live_expr x0)))) q')).
+ intuition.
+ apply ttau_prefix in H3.
+ intuition.
+ apply S_star with (y:=(E_apply swapf (E_taggingleft (E_pair x (E_live_expr x0))))). 
+ apply JO_red_dobind_td.
+ apply S_First.
+ simpl; auto.
+ assumption.
+ apply taured_val_id in H7.
+ substs.
+ apply swapf_left_b.
+ assumption. 
+ simpl; auto.
+ simpl; auto.
  simpl; auto.
 
- Qed.
+ destruct H1.
+ destruct H0.
+ intuition.
+ simplify_eq H0; clear H0; intros; substs.
+ destruct H3.
+ intuition.
+ substs.
+ apply taured_val_id in H0.
+ substs.
+ exists (E_live_expr (LM_expr (E_taggingleft (E_pair x (E_live_expr x0))))).
+ intuition.
+ inversion H4.
+ apply lab_r with (e1:=e1)(e2:=e2)(s:=s).
+ intuition.
+ substs.
+ apply star_trans with (y:= (E_apply (E_apply (E_constant CONST_fork) (E_live_expr x3))
+          (E_live_expr x2))); intuition.
+ apply forkee_tau with (lm':=( (LM_expr (E_taggingright (E_pair (E_live_expr x0) x))))).
+ intuition.
+ apply swapf_right_b.
+ simpl;auto.
+ assumption.
+ apply star_refl.
+ simpl; auto.
+ apply taured_val_id in H0.
+ substs.
+ exists (E_live_expr (LM_expr (E_taggingleft (E_pair x (E_live_expr x0))))).
+ intuition.
+ inversion H4.
+ apply lab_r with (e1:=e1)(e2:=e2)(s:=s).
+ intuition.
+ substs.
+ apply star_trans with (y:= (E_apply (E_apply (E_constant CONST_fork) (E_live_expr x3))
+          (E_live_expr x2))); intuition.
+ apply forkee_tau with (lm':=( (LM_expr (E_taggingright (E_pair (E_live_expr x0) x))))).
+ intuition.
+ apply swapf_right_b.
+ simpl; auto.
+ assumption.
+ assert ( totalTauRed
+  (E_apply 
+   swapf ( (E_taggingright (E_pair (E_live_expr x0) x)))) ( E_live_expr(LM_expr((E_taggingleft (E_pair x (E_live_expr x0) )))))).
+ apply swapf_right.
+ simpl; auto.
+ assumption.
+ assert ((totalTauRed (E_apply swapf (E_taggingright (E_pair (E_live_expr x0) x)))
+       (E_live_expr (LM_expr (E_taggingleft (E_pair x (E_live_expr x0))))))/\(tauRed (E_apply swapf (E_taggingright (E_pair (E_live_expr x0) x))) q')).
+ intuition.
+ apply ttau_prefix in H3.
+ intuition.
+ apply S_star with (y:=(E_apply swapf (E_taggingright (E_pair  (E_live_expr x0) x)))). 
+ apply JO_red_dobind_td.
+ apply S_First.
+ simpl; auto.
+ assumption.
+ apply taured_val_id in H7.
+ substs.
+ apply swapf_right_b.
+ 
+  
+ simpl; auto.
+ simpl; auto.
+ simpl; auto.
+ simpl; auto.
+ destruct H2.
+ destruct H0.
+ intuition.
+ discriminate H0.
+ destruct H2.
+ destruct H0.
+ intuition.
+ discriminate H0.
+ exists (E_apply (E_apply (E_constant CONST_fork) (E_live_expr x)) (E_live_expr x0)) (swapf).
+ reflexivity.
+ 
+ destruct H1.
+ intuition.
+ apply fork_label_swap_total in H1.
+ intuition.
+ destruct H0.
+ destruct H0.
+ intuition. 
+ discriminate H1.
+ destruct H1.
+ destruct H0.
+ intuition.
+ simplify_eq H0; clear H0; intros; substs. 
+ assert (totalTauRed (E_live_expr (LM_expr (E_taggingleft (E_pair x0 (E_live_expr x1) ))) >>=
+   swapf) (E_live_expr (LM_expr (E_taggingright (E_pair (E_live_expr x1) x0))))).
+ apply swapf_left_b.
+ simpl; auto.
+ simpl; auto.
+ assert (totalTauRed (E_live_expr (LM_expr (E_taggingleft (E_pair x0 (E_live_expr x1) ))) >>=
+   swapf) (E_live_expr (LM_expr (E_taggingright (E_pair (E_live_expr x1) x0)))) /\ (tauRed
+       (E_live_expr (LM_expr (E_taggingleft (E_pair x0 (E_live_expr x1)))) >>=
+        swapf) q')).
+ intuition.
+ apply ttau_prefix in H3.
+ intuition.
+ exists (E_live_expr (LM_expr (E_taggingright (E_pair (E_live_expr x1) x0)))).
+ intuition.
+ apply forkee_tau with (lm':=( (LM_expr (E_taggingleft (E_pair x0 (E_live_expr x1)))))).
+ intuition.
+ apply taured_val_id in H5.
+ substs.
+ exists (E_live_expr (LM_expr (E_taggingright (E_pair (E_live_expr x1) x0)))).
+ intuition.
+ apply forkee_tau with (lm':=( (LM_expr (E_taggingleft (E_pair x0 (E_live_expr x1)))))).
+ intuition.
+ simpl; auto.
+ destruct H1.
+ destruct H0.
+ intuition.
+ simplify_eq H0; clear H0; intros; substs. 
+ assert (totalTauRed (E_live_expr (LM_expr (E_taggingright (E_pair (E_live_expr x1) x0 ))) >>=
+   swapf) (E_live_expr (LM_expr (E_taggingleft (E_pair x0 (E_live_expr x1) ))))).
+ apply swapf_right_b.
+ simpl; auto.
+ simpl; auto.
+ assert (totalTauRed (E_live_expr (LM_expr (E_taggingright (E_pair (E_live_expr x1) x0 ))) >>=
+   swapf) (E_live_expr (LM_expr (E_taggingleft (E_pair x0 (E_live_expr x1) )))) /\ (tauRed
+       (E_live_expr (LM_expr (E_taggingright (E_pair (E_live_expr x1) x0))) >>=
+        swapf) q')).
+ intuition.
+ apply ttau_prefix in H3.
+ intuition.
+ exists (E_live_expr (LM_expr (E_taggingleft (E_pair x0 (E_live_expr x1))))).
+ intuition.
+ apply forkee_tau with (lm':=( (LM_expr (E_taggingright (E_pair (E_live_expr x1) x0))))).
+ intuition.
+ apply taured_val_id in H5.
+ substs.
+ exists (E_live_expr (LM_expr (E_taggingleft (E_pair x0 (E_live_expr x1))))).
+ intuition.
+ apply forkee_tau with (lm':=( (LM_expr (E_taggingright (E_pair (E_live_expr x1) x0))))).
+ intuition.
+ simpl; auto.
+  
+ substs.
+ intuition.
+ assert (~(labRed l (E_live_expr lm' >>= swapf) q')).
+ apply ttr_val_not_labred with (v:=(E_live_expr lm)).
+ intuition.
+ simpl; auto.
+ assert (labRed l (E_live_expr lm' >>= swapf) q').
+ inversion H0.
+ intuition.
+ apply lab_r with (e1:=e1)(e2:=e2)(s:=s).
+ intuition.
+ apply star_trans with (y:=q).
+ apply tau_incl_totalTau.
+ intuition.
+ assumption.
+ intuition.
+Qed.
+ 
+Notation " A # B " := (E_apply (E_apply (E_constant CONST_fork) ( (E_live_expr A)) ) ( (E_live_expr B))) (at level 20).
+Notation " A <# B "  := (E_live_expr(LM_expr(E_taggingleft(E_pair A (E_live_expr B))))) (at level 20).
+Notation " A #> B "  := (E_live_expr(LM_expr(E_taggingright(E_pair (E_live_expr A) B)))) (at level 20).
+Notation " A <|# B "  := (((E_taggingleft(E_pair A (E_live_expr B))))) (at level 20).
+Notation " A #|> B "  := (((E_taggingright(E_pair (E_live_expr B) A)))) (at level 20).
+
+
+Lemma fork_assoc_tau_step_int : forall (a a' b b' c c' : livemodes), tauStep ((LM_expr (a # b)) # c) ((LM_expr (a' # b')) # c')   ->
+ tauStep (a # ( LM_expr ( b # c ) ) ) (a' # ( LM_expr ( b' # c' ) )).
+Proof.
+ intros.
+ inversion H.
+ substs.
+ inversion H0.
+ substs.
+ inversion H5.
+ substs.
+ apply tStep with (s:=S_First).
+ apply JO_red_forkmove1 with (s:=s).
+ assumption.
+ substs.
+ apply tStep with (s:=S_Second).
+ apply JO_red_forkmove2 with (s:=S_First).
+ apply JO_red_forkmove1 with (s:=s).
+ assumption.
+ apply red_not_value in H6.
+ simpl in H6.
+ intuition.
+ apply red_not_value in H9.
+ simpl in H9.
+ intuition.
+ substs.
+ apply tStep with (s:=S_Second).
+ apply JO_red_forkmove2 with (s:=S_Second).
+ substs.
+ apply JO_red_forkmove2 with (s:=s0).
+ assumption.
+ apply red_not_value in H5; simpl in H5; intuition.
+ apply red_not_value in H8; simpl in H8; intuition.
+Qed.
+
+
+Lemma fork_tau_assoc_total : forall (a b c : livemodes) (e : expr) , tauRed ((LM_expr (a # b)) # c) e ->
+        (
+          (exists (a' b' c' : livemodes), e = (LM_expr (a' # b')) # c' /\ tauRed (a # (LM_expr (b # c))) (a' # (LM_expr (b' # c'))))
+          \/
+          (exists (a' b' : livemodes) (c' : expr), e = (LM_expr (a' # b')) #> c' /\ is_value_of_expr c' /\ tauRed (a # (LM_expr (b # c))) (a' #> ( (b' #> c'))))
+          \/
+          (exists (a' c' : livemodes) (b' : expr), e = ( (a' #> b')) <# c' /\ is_value_of_expr b' /\   tauRed (a # (LM_expr (b # c))) (a' #> ( (b' <# c'))))
+          \/
+          (exists (a' c' : livemodes) (b' : expr), e = (LM_expr (a' #> b')) # c' /\ is_value_of_expr b'/\  tauRed (a # (LM_expr (b # c))) (a' # ( LM_expr (b' <# c'))) /\  tauRed (a # (LM_expr (b # c))) (a' # ( LM_expr ( (LM_expr b') # c'))) )
+          \/
+          (exists (b' c' : livemodes) (a' : expr), e = (LM_expr (a' <# b')) # c' /\ is_value_of_expr a' /\  tauRed (a # (LM_expr (b # c))) (  a' <# ( LM_expr (b' # c'))) /\ tauRed (a # (LM_expr (b # c))) (  (LM_expr a') # ( LM_expr (b' # c'))) )
+          \/
+          (exists (b' c' : livemodes) (a' : expr), e = ( (a' <# b')) <# c' /\ is_value_of_expr a' /\  tauRed (a # (LM_expr (b # c))) (a' <# ( LM_expr (b' # c'))))
+          \/
+          (exists (a' : livemodes) (b' c' : expr), e = (LM_expr (a' #> b')) #> c' /\ is_value_of_expr b' /\ is_value_of_expr c'  /\  tauRed (a # (LM_expr (b # c))) (a' #> ( ((LM_expr b') #> c'))) /\ tauRed (a # (LM_expr (b # c))) (a' # ( LM_expr ((LM_expr b') # (LM_expr c')))) )
+          \/
+          (exists ( b'  : livemodes) (a' c' : expr), e = (LM_expr (a' <# b')) #> c' /\ is_value_of_expr a' /\ is_value_of_expr c'  /\  tauRed (a # (LM_expr (b # c))) (a' <# ( LM_expr (b' #> c'))) /\  tauRed (a # (LM_expr (b # c))) ((LM_expr a') # (( LM_expr (b' # (LM_expr c'))))))
+        ).
+Proof.
+ intros.
+ assert (L:=H).
+ induction a; induction b; induction c.
+ apply fork_tau_behave_ec in H.
+ destruct H.
+ intuition.
+ substs.
+ left.
+ apply fork_tau_behave_cc in H0.
+ substs.
+ exists (LM_comp lab) (LM_comp lab0) (LM_comp lab1 ).
+ intuition.
+ apply star_refl.
+ apply fork_tau_behave_cc in H0.
+ substs.
+ simpl in H2; intuition.
+ (* E(CC) E *)
+ apply fork_tau_behave_ee in H.
+ intuition.
+ destruct H0.
+ destruct H.
+ intuition.
+ substs.
+ apply fork_tau_behave_cc in H0.
+ substs.
+ left.
+ exists (LM_comp lab) (LM_comp lab0) (LM_expr x0).
+ intuition.
+ apply fork_tau_ce_push_h.
+ apply fork_tau_ce_push_h.
+ assumption.
+
+ destruct H.
+ destruct H.
+ intuition.
+ substs.
+ apply fork_tau_behave_cc in H.
+ substs.
+ branch 2.
+ exists (LM_comp lab) (LM_comp lab0) ( x0).
+ intuition.
+ apply star_trans with (y:=(LM_comp lab # LM_expr (LM_comp lab0 #> x0))).
+ apply fork_tau_ce_push_h.
+ apply star_trans with (y:=(LM_comp lab0 # LM_expr x0)).
+ apply fork_tau_ce_push_h.
+ assumption.
+ apply S_star with (y:=(LM_comp lab0 #> x0)).
+ apply tStep with (s:=S_Second).
+ apply JO_red_forkdeath2.
+ assumption.
+ apply star_refl.
+ apply S_star with (y:=(LM_comp lab #> (LM_comp lab0 #> x0))).
+ apply tStep with (s:=S_Second).
+ apply JO_red_forkdeath2.
+ simpl; auto.
+ apply star_refl.
+
+ destruct H.
+ destruct H.
+ intuition.
+ substs.
+ apply fork_tau_behave_cc in H.
+ substs.
+ simpl in H0; intuition.
+ (* E(CE) C *)
+ apply fork_tau_behave_ec in H.
+ destruct H.
+ intuition.
+ substs.
+ apply fork_tau_behave_ce in H0.
+ destruct H0.
+ intuition.
+ substs.
+ intuition.
+ left.
+ exists (LM_comp lab) (LM_expr x0) ( LM_comp lab0).
+ intuition.
+ apply fork_tau_ce_push_h.
+ apply fork_tau_ec_push_h.
+ assumption.
+ substs.
+ branch 4.
+ exists (LM_comp lab) (LM_comp lab0) x0.
+ intuition.
+ apply fork_tau_ce_push_h.
+ apply star_S with (y:=(LM_expr x0 # LM_comp lab0)).
+ apply fork_tau_ec_push_h.
+ assumption.
+ apply tStep with (s:=S_First).
+ apply JO_red_forkdeath1.
+ assumption.
+ apply fork_tau_ce_push_h.
+ apply fork_tau_ec_push_h.
+ assumption.
+ substs.
+ apply fork_tau_behave_ce in H0.
+ destruct H0.
+ intuition.
+ substs.
+ simpl in H2.
+ intuition.
+ substs.
+ branch 3.
+ exists (LM_comp lab) (LM_comp lab0) x0.
+ intuition.
+ apply star_trans with (y:=(LM_comp lab # LM_expr ( x0 <# LM_comp lab0))).
+ apply fork_tau_ce_push_h.
+ apply star_trans with (y:=(LM_expr x0 # LM_comp lab0)).
+ apply fork_tau_ec_push_h.
+ assumption.
+ apply S_star with (y:=(x0 <# LM_comp lab0)).
+ apply tStep with (s:=S_First).
+ apply JO_red_forkdeath1.
+ assumption.
+ apply star_refl.
+ apply S_star with (y:= (LM_comp lab #> (x0 <# LM_comp lab0))).
+ apply tStep with (s:=S_Second).
+ apply JO_red_forkdeath2.
+ simpl; auto.
+ apply star_refl.
+ 
+
+ (* E(CE) E *)
+ apply fork_tau_behave_ee in H.
+ intuition.
+ destruct  H0.
+ destruct H.
+ intuition.
+ substs.
+ apply fork_tau_behave_ce in H0.
+ destruct H0.
+ intuition.
+ substs.
+ left.
+ exists (LM_comp lab) (LM_expr x1) (LM_expr x0).
+ intuition.
+ apply fork_tau_ce_push_h.
+ apply fork_tau_push_ee_12.
+ assumption.
+ assumption.
+ substs.
+ branch 4.
+ exists (LM_comp lab) (LM_expr x0) (x1).
+ intuition.
+ apply fork_tau_ce_push_h.
+ apply star_S with (y:=(LM_expr x1 # LM_expr x0)).
+ apply fork_tau_push_ee_12.
+ assumption.
+ assumption.
+ apply tStep with (s:=S_First).
+ apply JO_red_forkdeath1.
+ assumption.
+ apply fork_tau_ce_push_h.
+ apply fork_tau_push_ee_12.
+ assumption.
+ assumption.
+ destruct H.
+ destruct H.
+ intuition.
+ substs.
+ apply fork_tau_behave_ce in H.
+ destruct H.
+ intuition.
+ substs.
+ branch 2.
+ exists (LM_comp lab) (LM_expr x1) ( x0).
+ intuition.
+ apply star_trans with (y:=(LM_comp lab # LM_expr (LM_expr x1 #> x0))).
+ apply fork_tau_ce_push_h.
+ apply star_trans with (y:=(LM_expr x1 # LM_expr x0)).
+ apply fork_tau_push_ee_12.
+ assumption.
+ assumption.
+ apply S_star with (y:=(LM_expr x1 #> x0)).
+ apply tStep with (s:=S_Second).
+ apply JO_red_forkdeath2.
+ assumption.
+ apply star_refl.
+ apply S_star with (y:=(LM_comp lab #> (LM_expr x1 #> x0))).
+ apply tStep with (s:=S_Second).
+ apply JO_red_forkdeath2.
+ simpl; auto.
+ apply star_refl.
+ 
+ substs.
+ branch 7.
+ exists (LM_comp lab) (x1) (x0).
+ intuition.
+ apply star_S with (y:=(LM_comp lab # LM_expr (LM_expr x1 #> x0))).
+ apply fork_tau_ce_push_h.
+ apply star_S with (y:=(LM_expr x1 # LM_expr x0)).
+ apply fork_tau_push_ee_12.
+ assumption.
+ assumption.
+ apply tStep with (s:=S_Second).
+ apply JO_red_forkdeath2.
+ assumption.
+ apply tStep with (s:=S_Second).
+ apply JO_red_forkdeath2.
+ simpl; auto.
+ apply fork_tau_ce_push_h.
+ apply fork_tau_push_ee_12.
+ assumption.
+ assumption.
+ destruct H.
+ destruct H.
+ intuition.
+ substs.
+ apply fork_tau_behave_ce in H.
+ destruct H.
+ intuition.
+ substs.
+ simpl in H0; intuition.
+ substs.
+ branch 3.
+ exists (LM_comp lab) (LM_expr x0) (x1).
+ intuition.
+ apply star_S with (y:=(LM_comp lab # (LM_expr (x1 <# LM_expr x0)))).
+ apply fork_tau_ce_push_h.
+ apply star_S with (y:=(LM_expr x1 # LM_expr x0)).
+ apply fork_tau_push_ee_12.
+ assumption.
+ assumption.
+ apply tStep with (s:=S_First).
+ apply JO_red_forkdeath1.
+ assumption.
+ apply tStep with (s:=S_Second).
+ apply JO_red_forkdeath2.
+ simpl; auto.
+
+ (* E(EC) C *)
+ apply fork_tau_behave_ec in H.
+ destruct H.
+ intuition.
+ substs.
+ apply fork_tau_behave_ec in H0.
+ destruct H0.
+ intuition.
+ substs.
+ intuition.
+ left.
+ exists  (LM_expr x0) (LM_comp lab) ( LM_comp lab0).
+ intuition.
+ apply fork_tau_push_ee_1.
+ assumption.
+ substs.
+ branch 5.
+ exists (LM_comp lab) (LM_comp lab0) x0.
+ intuition.
+ apply star_S with (y:=(LM_expr x0 # LM_expr (LM_comp lab # LM_comp lab0))).
+ apply fork_tau_push_ee_12.
+ apply star_refl.
+ assumption.
+ apply tStep with (s:=S_First).
+ apply JO_red_forkdeath1.
+ assumption.
+ apply fork_tau_push_ee_12.
+ apply star_refl.
+ assumption.
+ 
+ substs.
+ apply fork_tau_behave_ec in H0.
+ destruct H0.
+ intuition.
+ substs.
+ simpl in H2.
+ intuition.
+ substs.
+ branch 6.
+ exists (LM_comp lab) (LM_comp lab0) x0.
+ intuition.
+ apply star_S with (y:=(LM_expr x0 # LM_expr (LM_comp lab # LM_comp lab0))).
+ apply fork_tau_push_ee_12.
+ apply star_refl.
+ assumption.
+ apply tStep with (s:=S_First).
+ apply JO_red_forkdeath1.
+ assumption.
+ (* E(EC) E *)
+ apply fork_tau_behave_ee in H.
+ intuition.
+ destruct  H0.
+ destruct H.
+ intuition.
+ substs.
+ apply fork_tau_behave_ec in H0.
+ destruct H0.
+ intuition.
+ substs.
+ left.
+ exists (LM_expr x1) (LM_comp lab) (LM_expr x0).
+ intuition.
+ apply fork_tau_push_ee_12.
+ apply fork_tau_ce_push_h.
+ assumption.
+ assumption.
+ substs.
+ branch 5.
+ exists (LM_comp lab) (LM_expr x0) (x1).
+ intuition.
+ apply star_S with (y:=(LM_expr x1 # LM_expr (LM_comp lab # LM_expr x0))).
+ apply fork_tau_push_ee_12.
+ apply fork_tau_ce_push_h.
+ assumption.
+ assumption.
+ apply tStep with (s:=S_First).
+ apply JO_red_forkdeath1.
+ assumption.
+ apply fork_tau_push_ee_12.
+ apply fork_tau_ce_push_h.
+ assumption.
+ assumption.
+ destruct H.
+ destruct H.
+ intuition.
+ substs.
+ apply fork_tau_behave_ec in H.
+ destruct H.
+ intuition.
+ substs.
+ branch 2.
+ exists (LM_expr x1) (LM_comp lab) ( x0).
+ intuition.
+ apply star_trans with (y:=(LM_expr x1 # LM_expr (LM_comp lab #> x0))).
+ apply fork_tau_push_ee_12.
+ apply star_trans with (y:=(LM_comp lab # LM_expr x0)).
+ apply fork_tau_ce_push_h.
+ assumption.
+ apply S_star with (y:=(LM_comp lab #> x0)).
+ apply tStep with (s:=S_Second).
+ apply JO_red_forkdeath2.
+ assumption.
+ apply star_refl.
+ assumption.
+ apply S_star with (y:=(LM_expr x1 #> (LM_comp lab #> x0))).
+ apply tStep with (s:=S_Second).
+ apply JO_red_forkdeath2.
+ simpl; auto.
+ apply star_refl.
+ substs.
+ branch 8.
+ exists (LM_comp lab) (x1) (x0).
+ intuition.
+ apply star_S with (y:=((LM_expr x1) # LM_expr (LM_comp lab #> x0))).
+ apply fork_tau_push_ee_12.
+ apply star_S with (y:=(LM_comp lab # LM_expr x0)).
+ apply fork_tau_ce_push_h.
+ assumption.
+ apply tStep with (s:=S_Second); apply JO_red_forkdeath2; assumption.
+ assumption.
+ apply tStep with (s:=S_First); apply JO_red_forkdeath1; assumption.
+ apply fork_tau_push_ee_12.
+ apply fork_tau_ce_push_h.
+ assumption.
+ assumption.
+ destruct H.
+ destruct H.
+ intuition.
+ substs.
+ apply fork_tau_behave_ec in H.
+ destruct H.
+ intuition.
+ substs.
+ simpl in H0; intuition.
+ substs.
+ branch 6.
+ exists (LM_comp lab) (LM_expr x0) (x1).
+ intuition.
+ apply star_S with (y:=(LM_expr x1 # LM_expr (LM_comp lab # LM_expr x0))).
+ apply fork_tau_push_ee_12.
+ apply fork_tau_ce_push_h; assumption.
+ assumption.
+ apply tStep with (s:=S_First); apply JO_red_forkdeath1;  assumption.
+ (* E(EE) C *)
+ apply fork_tau_behave_ec in H.
+ destruct H.
+ intuition.
+ substs.
+ apply fork_tau_behave_ee in H0.
+ intuition.
+ destruct H.
+ destruct H.
+ intuition.
+ substs.
+ left.
+ exists  (LM_expr x0) (LM_expr x1) ( LM_comp lab).
+ intuition.
+ apply fork_tau_push_ee_12.
+ apply fork_tau_ec_push_h.
+ assumption.
+ assumption.
+ destruct H0.
+ destruct H.
+ intuition.
+ substs.
+ branch 4.
+ exists (LM_expr x0) (LM_comp lab) x1.
+ intuition.
+ apply fork_tau_push_ee_12.
+ apply star_S with (y:=(LM_expr x1 # LM_comp lab)).
+ apply fork_tau_ec_push_h.
+ assumption.
+ apply tStep with (s:=S_First).
+ apply JO_red_forkdeath1.
+ assumption.
+ assumption.
+ apply fork_tau_push_ee_12.
+ apply fork_tau_ec_push_h.
+ assumption.
+ assumption.
+ destruct H0.
+ destruct H.
+ intuition.
+ substs.
+ branch 5.
+ exists (LM_expr x1) (LM_comp lab) x0.
+ intuition.
+ apply star_S with (y:=(LM_expr x0 # LM_expr (LM_expr x1 # LM_comp lab))).
+ apply fork_tau_push_ee_12.
+ apply fork_tau_ec_push_h; assumption.
+ assumption.
+ apply tStep with (s:=S_First).
+ apply JO_red_forkdeath1.
+ assumption.
+ apply fork_tau_push_ee_12.
+ apply fork_tau_ec_push_h.
+ assumption.
+ assumption.
+ substs.
+ apply fork_tau_behave_ee in H0.
+ intuition.
+ destruct H.
+ destruct H.
+ intuition.
+ substs.
+ simpl in H2; intuition.
+ destruct H0.
+ destruct H.
+ intuition.
+ substs.
+ branch 3.
+ exists (LM_expr x0) (LM_comp lab) x1.
+ intuition.
+ apply star_S with (y:=(LM_expr x0 # (LM_expr (x1 <# LM_comp lab)))).
+ apply fork_tau_push_ee_12.
+ apply star_S with (y:=(LM_expr x1 # LM_comp lab)).
+ apply fork_tau_ec_push_h.
+ assumption.
+ apply tStep with (s:=S_First).
+ apply JO_red_forkdeath1.
+ assumption.
+ assumption.
+ apply tStep with (s:=S_Second).
+ apply JO_red_forkdeath2.
+ simpl; auto.
+ 
+ destruct H0.
+ destruct H.
+ intuition.
+ substs.
+ branch 6.
+ exists (LM_expr x1) (LM_comp lab) x0.
+ intuition.
+ apply star_S with (y:=(LM_expr x0 # LM_expr (LM_expr x1 # LM_comp lab))).
+ apply fork_tau_push_ee_12.
+ apply fork_tau_ec_push_h; assumption.
+ assumption.
+ apply tStep with (s:=S_First).
+ apply JO_red_forkdeath1.
+ assumption.
+ (* E(EE) E *)
+ apply fork_tau_behave_ee in H.
+ intuition.
+ destruct  H0.
+ destruct H.
+ intuition.
+ substs.
+ apply fork_tau_behave_ee in H0.
+ intuition.
+ destruct H1.
+ destruct H0.
+ intuition.
+ substs.
+ left.
+ exists (LM_expr x1) (LM_expr x2) (LM_expr x0).
+ intuition.
+ apply fork_tau_push_ee_12.
+ apply fork_tau_push_ee_12.
+ assumption.
+ assumption.
+ assumption.
+ destruct H0.
+ destruct H0.
+ intuition.
+ substs.
+ branch 4.
+ exists (LM_expr x1) (LM_expr x0) (x2).
+ intuition.
+ apply fork_tau_push_ee_12.
+ apply star_S with (y:=(LM_expr x2 # LM_expr x0)).
+ apply fork_tau_push_ee_12.
+ assumption.
+ assumption.
+ apply tStep with (s:=S_First).
+ apply JO_red_forkdeath1.
+ assumption.
+ assumption.
+ apply fork_tau_push_ee_12.
+ apply fork_tau_push_ee_12.
+ assumption. 
+ assumption.
+ assumption.
+ destruct H0.
+ destruct H0.
+ intuition.
+ substs.
+ branch 5.
+ exists (LM_expr x2) (LM_expr x0) x1.
+ intuition.
+ apply star_S with (y:=(LM_expr x1 # LM_expr (LM_expr x2 # LM_expr x0))).
+ apply fork_tau_push_ee_12.
+ apply fork_tau_push_ee_12.
+ assumption.
+ assumption.
+ assumption.
+ apply tStep with (s:=S_First).
+ apply JO_red_forkdeath1.
+ assumption.
+ apply fork_tau_push_ee_12.
+ apply fork_tau_push_ee_12.
+ assumption. 
+ assumption.
+ assumption.
+ destruct H.
+ destruct H.
+ intuition.
+ substs.
+ apply fork_tau_behave_ee in H.
+ intuition.
+ destruct H2.
+ destruct H.
+ intuition.
+ substs.
+ branch 2.
+ exists (LM_expr x1) (LM_expr x2) ( x0).
+ intuition.
+ apply star_S with (y:=(LM_expr x1 # LM_expr (LM_expr x2 #> x0))).
+ apply fork_tau_push_ee_12.
+ apply star_S with (y:=(LM_expr x2 # LM_expr x0)).
+ apply fork_tau_push_ee_12.
+ assumption.
+ assumption.
+ apply tStep with (s:=S_Second).
+ apply JO_red_forkdeath2.
+ assumption.
+ assumption.
+ apply tStep with (s:=S_Second).
+ apply JO_red_forkdeath2.
+ simpl; auto.
+
+ destruct H.
+ destruct H.
+ intuition.
+ substs.
+ branch 7.
+ exists (LM_expr x1) (x2) (x0).
+ intuition.
+ apply star_S with (y:=(LM_expr x1 # LM_expr (LM_expr x2 #> x0))).
+ apply fork_tau_push_ee_12.
+ apply star_S with (y:=(LM_expr x2 # LM_expr x0)).
+ apply fork_tau_push_ee_12.
+ assumption.
+ assumption.
+ apply tStep with (s:=S_Second).
+ apply JO_red_forkdeath2.
+ assumption.
+ assumption.
+ apply tStep with (s:=S_Second).
+ apply JO_red_forkdeath2.
+ simpl; auto.
+ apply fork_tau_push_ee_12.
+ apply fork_tau_push_ee_12.
+ assumption.
+ assumption.
+ assumption.
+ destruct H.
+ destruct H.
+ intuition.
+ substs.
+ branch 8.
+ exists (LM_expr x2) x1 x0.
+ intuition.
+ apply star_S with (y:=((LM_expr x1) # LM_expr (LM_expr x2 #> x0))).
+ apply fork_tau_push_ee_12.
+ apply star_S with (y:=(LM_expr x2 # LM_expr x0)).
+ apply fork_tau_push_ee_12.
+ assumption.
+ assumption.
+ apply tStep with (s:=S_Second); apply JO_red_forkdeath2; assumption.
+ assumption.
+ apply tStep with (s:=S_First); apply JO_red_forkdeath1; assumption.
+ apply fork_tau_push_ee_12.
+ apply fork_tau_push_ee_12.
+ assumption.
+ assumption.
+ assumption.
+ destruct H.
+ destruct H.
+ intuition.
+ substs.
+ apply fork_tau_behave_ee in H.
+ intuition.
+ destruct H2.
+ destruct H.
+ intuition.
+ substs.
+ simpl in H0; intuition.
+ destruct H.
+ destruct H.
+ intuition.
+ substs.
+ branch 3.
+ exists (LM_expr x1) (LM_expr x0) (x2).
+ intuition.
+ apply star_trans with (y:= (LM_expr x1 # (LM_expr (x2 <# LM_expr x0)))).
+ apply fork_tau_push_ee_12.
+ apply star_trans with (y:=(LM_expr x2 # LM_expr x0)).
+ apply fork_tau_push_ee_12.
+ assumption.
+ assumption.
+ apply S_star with (y:=(x2 <# LM_expr x0)).
+ apply tStep with (s:=S_First).
+ apply JO_red_forkdeath1.
+ assumption.
+ apply star_refl.
+ assumption.
+ apply S_star with (y:= (LM_expr x1 #> (x2 <# LM_expr x0))).
+ apply tStep with (s:=S_Second).
+ apply JO_red_forkdeath2.
+ simpl; auto.
+ apply star_refl.
+ destruct H.
+ destruct H.
+ intuition.
+ substs.
+ branch 6.
+ exists (LM_expr x2) (LM_expr x0) x1.
+ intuition.
+ apply star_S with (y:=(LM_expr x1 # LM_expr (LM_expr x2 # LM_expr x0))).
+ apply fork_tau_push_ee_12.
+ apply fork_tau_push_ee_12.
+ assumption.
+ assumption.
+ assumption.
+ apply tStep with (s:=S_First).
+ apply JO_red_forkdeath1.
+ assumption.
+Qed.
+
+Lemma fork_lab_assoc_total : forall (a b c : livemodes) (e : expr) (l : label) , labRed l ((LM_expr (a # b)) # c) e ->
+        (
+          (exists (a' b' c' : livemodes), e = (LM_expr (a' # b')) # c' /\ labRed l (a # (LM_expr (b # c))) (a' # (LM_expr (b' # c'))))
+          \/
+          (exists (a' b' : livemodes) (c' : expr), e = (LM_expr (a' # b')) #> c' /\ is_value_of_expr c' /\ labRed l (a # (LM_expr (b # c))) (a' #> ( (b' #> c'))))
+          \/
+          (exists (a' c' : livemodes) (b' : expr), e = ( (a' #> b')) <# c' /\ is_value_of_expr b' /\   labRed l  (a # (LM_expr (b # c))) (a' #> ( (b' <# c'))))
+          \/
+          (exists (a' c' : livemodes) (b' : expr), e = (LM_expr (a' #> b')) # c' /\ is_value_of_expr b'/\  labRed l (a # (LM_expr (b # c))) (a' # ( LM_expr (b' <# c'))) )
+          \/
+          (exists (b' c' : livemodes) (a' : expr), e = (LM_expr (a' <# b')) # c' /\ is_value_of_expr a' /\  labRed l (a # (LM_expr (b # c))) (  a' <# ( LM_expr (b' # c'))) )
+          \/
+          (exists (b' c' : livemodes) (a' : expr), e = ( (a' <# b')) <# c' /\ is_value_of_expr a' /\  labRed l (a # (LM_expr (b # c))) (a' <# ( LM_expr (b' # c'))))
+          \/
+          (exists (a' : livemodes) (b' c' : expr), e = (LM_expr (a' #> b')) #> c' /\ is_value_of_expr b' /\ is_value_of_expr c'  /\  labRed l (a # (LM_expr (b # c))) (a' #> ( ((LM_expr b') #> c'))))
+          \/
+          (exists ( b'  : livemodes) (a' c' : expr), e = (LM_expr (a' <# b')) #> c' /\ is_value_of_expr a' /\ is_value_of_expr c'  /\  labRed l (a # (LM_expr (b # c))) (a' <# ( LM_expr (b' #> c'))))
+          \/
+          (exists (x : livemodes) (q' : expr), e = (LM_expr (x #> (E_constant CONST_unit))) #> q' /\ tauRed (a # LM_expr (b # c)) (x # LM_expr (LM_comp l # LM_expr q')) /\ is_value_of_expr q' /\ labRed l (a # LM_expr (b # c)) (x #> (E_constant CONST_unit <# (LM_expr q'))))
+        ).
+Proof.
+ intros.
+ inversion H.
+ substs.
+ intuition.
+ apply fork_tau_assoc_total in H1.
+ intuition.
+ (* B1 *)
+ destruct H2.
+ destruct H1.
+ destruct H1.
+ destruct H1.
+ substs.
+ inversion H0.
+ (* B1 - L1 *)
+ substs.
+ inversion H8.
+ (* B1 - L1 - L1 *)
+ substs.
+ apply fork_tau_assoc_total in H3.
+ intuition.
+ branch 1.
+ destruct H1 as [ a' H1 ]; destruct H1 as [ b' H1 ]; destruct H1 as [ c' H1 ]; exists a' b' c';
+ intuition;
+ apply lab_r with (e1:=(LM_expr e0 # LM_expr (x0 # x1)))  (e2:=(LM_expr e''0 # LM_expr (x0 # x1))) (s:=S_First);
+ intuition;
+ apply JO_red_forkmove1 with (s:=s);
+ auto.
+ branch 2;
+ destruct H3 as [ a' H1 ]; destruct H1 as [ b' H1 ]; destruct H1 as [ c' H1 ];
+ exists a' b' c';
+ intuition;
+ apply lab_r with (e1:=(LM_expr e0 # LM_expr (x0 # x1)))  (e2:=(LM_expr e''0 # LM_expr (x0 # x1))) (s:=S_First);
+ intuition;
+ apply JO_red_forkmove1 with (s:=s);
+ auto.
+ branch 3;
+ destruct H1 as [ a' H1 ]; destruct H1 as [ b' H1 ]; destruct H1 as [ c' H1 ];
+ exists a' b' c';
+ intuition;
+ apply lab_r with (e1:=(LM_expr e0 # LM_expr (x0 # x1)))  (e2:=(LM_expr e''0 # LM_expr (x0 # x1))) (s:=S_First);
+ intuition;
+ apply JO_red_forkmove1 with (s:=s);
+ auto.
+ branch 4;
+ destruct H3 as [ a' H1 ]; destruct H1 as [ b' H1 ]; destruct H1 as [ c' H1 ];
+ exists a' b' c';
+ intuition;
+ apply lab_r with (e1:=(LM_expr e0 # LM_expr (x0 # x1)))  (e2:=(LM_expr e''0 # LM_expr (x0 # x1))) (s:=S_First);
+ intuition;
+ apply JO_red_forkmove1 with (s:=s);
+ auto.
+ branch 5.
+ destruct H1 as [ a' H1 ]; destruct H1 as [ b' H1 ]; destruct H1 as [ c' H1 ].
+ exists a' b' c'.
+ intuition.
+ apply lab_r with (e1:=(LM_expr e0 # LM_expr (x0 # x1)))  (e2:=(LM_expr e''0 # LM_expr (x0 # x1))) (s:=S_First).
+ intuition.
+ apply JO_red_forkmove1 with (s:=s).
+ auto.
+ branch 6.
+ destruct H3 as [ a' H1 ]; destruct H1 as [ b' H1 ]; destruct H1 as [ c' H1 ].
+ exists a' b' c'.
+ intuition.
+ apply lab_r with (e1:=(LM_expr e0 # LM_expr (x0 # x1)))  (e2:=(LM_expr e''0 # LM_expr (x0 # x1))) (s:=S_First).
+ intuition.
+ apply JO_red_forkmove1 with (s:=s).
+ auto.
+ branch 7.
+ destruct H1 as [ a' H1 ]; destruct H1 as [ b' H1 ]; destruct H1 as [ c' H1 ].
+ exists a' b' c'.
+ intuition.
+ apply lab_r with (e1:=(LM_expr e0 # LM_expr (x0 # x1)))  (e2:=(LM_expr e''0 # LM_expr (x0 # x1))) (s:=S_First).
+ intuition.
+ apply JO_red_forkmove1 with (s:=s).
+ auto.
+ branch 8.
+ destruct H1 as [ a' H1 ]; destruct H1 as [ b' H1 ]; destruct H1 as [ c' H1 ].
+ left.
+ exists a' b' c'.
+ intuition.
+ apply lab_r with (e1:=(LM_expr e0 # LM_expr (x0 # x1)))  (e2:=(LM_expr e''0 # LM_expr (x0 # x1))) (s:=S_First).
+ intuition.
+ apply JO_red_forkmove1 with (s:=s).
+ auto.
+ (* B1 - L1 - L2 *)
+ substs.
+ apply fork_tau_assoc_total in H3.
+ intuition.
+ branch 1;
+ destruct H1 as [ a' H1 ]; destruct H1 as [ b' H1 ]; destruct H1 as [ c' H1 ]; exists a' b' c';
+ intuition;
+ apply lab_r with (e1:=(x # LM_expr (LM_expr e' # x1)))  (e2:=(x # LM_expr (LM_expr e''0 # x1))) (s:=S_Second);
+ intuition;
+ apply JO_red_forkmove2 with (s:=S_First);
+ apply JO_red_forkmove1 with (s:=s);
+ auto.
+ branch 2;
+ destruct H3 as [ a' H1 ]; destruct H1 as [ b' H1 ]; destruct H1 as [ c' H1 ]; exists a' b' c';
+ intuition;
+ apply lab_r with (e1:=(x # LM_expr (LM_expr e' # x1)))  (e2:=(x # LM_expr (LM_expr e''0 # x1))) (s:=S_Second);
+ intuition;
+ apply JO_red_forkmove2 with (s:=S_First);
+ apply JO_red_forkmove1 with (s:=s);
+ auto.
+  branch 3;
+ destruct H1 as [ a' H1 ]; destruct H1 as [ b' H1 ]; destruct H1 as [ c' H1 ]; exists a' b' c';
+ intuition;
+ apply lab_r with (e1:=(x # LM_expr (LM_expr e' # x1)))  (e2:=(x # LM_expr (LM_expr e''0 # x1))) (s:=S_Second);
+ intuition;
+ apply JO_red_forkmove2 with (s:=S_First);
+ apply JO_red_forkmove1 with (s:=s);
+ auto.
+  branch 4;
+ destruct H3 as [ a' H1 ]; destruct H1 as [ b' H1 ]; destruct H1 as [ c' H1 ]; exists a' b' c';
+ intuition;
+ apply lab_r with (e1:=(x # LM_expr (LM_expr e' # x1)))  (e2:=(x # LM_expr (LM_expr e''0 # x1))) (s:=S_Second);
+ intuition;
+ apply JO_red_forkmove2 with (s:=S_First);
+ apply JO_red_forkmove1 with (s:=s);
+ auto.
+  branch 5;
+ destruct H1 as [ a' H1 ]; destruct H1 as [ b' H1 ]; destruct H1 as [ c' H1 ]; exists a' b' c';
+ intuition;
+ apply lab_r with (e1:=(x # LM_expr (LM_expr e' # x1)))  (e2:=(x # LM_expr (LM_expr e''0 # x1))) (s:=S_Second);
+ intuition;
+ apply JO_red_forkmove2 with (s:=S_First);
+ apply JO_red_forkmove1 with (s:=s);
+ auto.
+  branch 6;
+ destruct H3 as [ a' H1 ]; destruct H1 as [ b' H1 ]; destruct H1 as [ c' H1 ]; exists a' b' c';
+ intuition;
+ apply lab_r with (e1:=(x # LM_expr (LM_expr e' # x1)))  (e2:=(x # LM_expr (LM_expr e''0 # x1))) (s:=S_Second);
+ intuition;
+ apply JO_red_forkmove2 with (s:=S_First);
+ apply JO_red_forkmove1 with (s:=s);
+ auto.
+  branch 7;
+ destruct H1 as [ a' H1 ]; destruct H1 as [ b' H1 ]; destruct H1 as [ c' H1 ]; exists a' b' c';
+ intuition;
+ apply lab_r with (e1:=(x # LM_expr (LM_expr e' # x1)))  (e2:=(x # LM_expr (LM_expr e''0 # x1))) (s:=S_Second);
+ intuition;
+ apply JO_red_forkmove2 with (s:=S_First);
+ apply JO_red_forkmove1 with (s:=s);
+ auto.
+  branch 8; left;
+ destruct H1 as [ a' H1 ]; destruct H1 as [ b' H1 ]; destruct H1 as [ c' H1 ]; exists a' b' c';
+ intuition;
+ apply lab_r with (e1:=(x # LM_expr (LM_expr e' # x1)))  (e2:=(x # LM_expr (LM_expr e''0 # x1))) (s:=S_Second);
+ intuition;
+ apply JO_red_forkmove2 with (s:=S_First);
+ apply JO_red_forkmove1 with (s:=s);
+ auto.
+ (* B1 - L1 - L3 *)
+ substs.
+ induction x1.
+ apply fork_tau_behave_ec in H3.
+ destruct H3.
+ intuition.
+ substs.
+ apply taured_val_id in H3.
+ substs.
+ branch 5.
+ exists x0 (LM_comp lab) (E_constant CONST_unit).
+ intuition.
+ simpl; auto.
+ apply lab_r with (e1:=(LM_comp l # LM_expr (x0 # LM_comp lab))) (e2:=(E_constant CONST_unit <# LM_expr (x0 # LM_comp lab))) (s:=S_First).
+ intuition.
+ apply JO_red_forkdocomp1.
+ apply star_refl.
+ simpl; auto.
+ apply taured_val_id in H3.
+ substs.
+ branch 6.
+ exists x0 (LM_comp lab) (E_constant CONST_unit).
+ intuition.
+ apply lab_r with (e1:=(LM_comp l # LM_expr (x0 # LM_comp lab))) (e2:=(E_constant CONST_unit <# LM_expr (x0 # LM_comp lab))) (s:=S_First).
+ intuition.
+ apply JO_red_forkdocomp1.
+ apply star_refl.
+ simpl; auto.
+ apply fork_tau_behave_ee in H3.
+ intuition.
+ substs.
+ destruct H1 as [p' H1]; destruct H1 as [q' H1]; destruct H1 as [ H1 H3 ]; destruct H3 as [ H3 H4 ]; substs.
+ apply taured_val_id in H1; substs.
+ branch 5.
+ exists x0 (LM_expr q') (E_constant CONST_unit).
+ intuition.
+ simpl; auto.
+ apply lab_r with (e1:=(LM_comp l # LM_expr (x0 # LM_expr q'))) (e2:=(E_constant CONST_unit <# LM_expr (x0 # LM_expr q')))(s:=S_First).
+ intuition.
+ apply star_trans with (y:=(LM_comp l # LM_expr (x0 # LM_expr expr5))).
+ assumption.
+ apply fork_tau_ce_push_h.
+ induction x0.
+ apply fork_tau_ce_push_h.
+ assumption.
+ apply fork_tau_push_ee_2.
+ assumption.
+ apply JO_red_forkdocomp1.
+ apply star_refl.
+ simpl; auto.
+ destruct H3 as [p' H1]; destruct H1 as [q' H1]; destruct H1 as [ H1 H3 ]; destruct H3 as [ H3 H4 ]; destruct H4 as [ H4 H5 ]; substs.
+ apply taured_val_id in H3; substs.
+ branch 8. left.
+ exists x0 (E_constant CONST_unit) q'.
+ intuition.
+ simpl; auto.
+ apply lab_r with (e1:=(LM_comp l # LM_expr (x0 #> q')))(e2:=(E_constant CONST_unit <# LM_expr (x0 #> q')))(s:=S_First).
+ intuition.
+ apply star_trans with (y:=(LM_comp l # LM_expr (x0 # LM_expr expr5))).
+ assumption.
+ apply star_S with (y:=(LM_comp l # LM_expr (x0 # LM_expr q'))).
+ apply fork_tau_ce_push_h.
+ induction x0.
+ apply fork_tau_ce_push_h.
+ assumption.
+ apply fork_tau_push_ee_2.
+ assumption.
+ apply tStep with (s:=S_Second).
+ apply JO_red_forkmove2 with (s:=S_Second).
+ apply JO_red_forkdeath2.
+ assumption.
+ apply JO_red_forkdocomp1.
+ apply star_refl.
+ simpl; auto.
+ destruct H3 as [p' H1]; destruct H1 as [q' H1]; destruct H1 as [ H1 H3 ]; destruct H3 as [ H3 H4 ]; destruct H4 as [ H4 H5 ]; substs.
+ apply taured_val_id in H3; substs.
+ branch 6.
+ exists x0 (LM_expr q') (E_constant CONST_unit).
+ intuition.
+ apply lab_r with (e1:=(LM_comp l # LM_expr (x0 # LM_expr q')))(e2:=(E_constant CONST_unit <# LM_expr (x0 # LM_expr q')))(s:=S_First).
+ intuition.
+ apply star_trans with (y:=(LM_comp l # LM_expr (x0 # LM_expr expr5))).
+ assumption.
+ apply fork_tau_ce_push_h.
+ induction x0.
+ apply fork_tau_ce_push_h.
+ assumption.
+ apply fork_tau_push_ee_2.
+ assumption.
+ apply JO_red_forkdocomp1.
+ apply star_refl.
+ simpl; auto.
+ (* B1 - L1 - L4 *)
+ substs.
+ induction x1.
+ apply fork_tau_behave_ec in H3.
+ destruct H3.
+ intuition.
+ substs.
+ apply taured_val_id in H3.
+ substs.
+ branch 4.
+ exists x (LM_comp lab) (E_constant CONST_unit).
+ intuition.
+ simpl; auto.
+ apply lab_r with (e1:=(x # LM_expr (LM_comp l # LM_comp lab)))(e2:=(x # LM_expr (E_constant CONST_unit <# LM_comp lab)))(s:=S_Second).
+ intuition.
+ apply JO_red_forkmove2 with (s:=S_First).
+ apply JO_red_forkdocomp1.
+ apply star_refl.
+ simpl; auto.
+ apply taured_val_id in H3.
+ substs.
+ branch 3.
+ exists x (LM_comp lab) (E_constant CONST_unit).
+ intuition.
+ simpl; auto.
+ apply lab_r with (e1:=(x # LM_expr (LM_comp l # LM_comp lab)))(e2:=(x # LM_expr (E_constant CONST_unit <# LM_comp lab)))(s:=S_Second).
+ intuition.
+ apply JO_red_forkmove2 with (s:=S_First).
+ apply JO_red_forkdocomp1.
+ apply S_star with (y:=(x #> (E_constant CONST_unit <# LM_comp lab))).
+ apply tStep with (s:=S_Second).
+ apply JO_red_forkdeath2.
+ simpl; auto.
+ apply star_refl.
+ simpl; auto.
+ apply fork_tau_behave_ee in H3.
+ intuition.
+ substs.
+ destruct H1 as [p' H1]; destruct H1 as [q' H1]; destruct H1 as [ H1 H3 ]; destruct H3 as [ H3 H4 ]; substs.
+ apply taured_val_id in H1; substs.
+ branch 4.
+ exists x (LM_expr q') (E_constant CONST_unit).
+ intuition.
+ simpl; auto.
+ apply lab_r with (e1:=(x # LM_expr (LM_comp l # LM_expr q'))) (e2:=(x # LM_expr (E_constant CONST_unit <# LM_expr q')))(s:=S_Second).
+ intuition.
+ apply star_trans with (y:=(x # LM_expr (LM_comp l # LM_expr expr5))).
+ assumption.
+ induction x.
+ apply fork_tau_ce_push_h.
+ apply fork_tau_ce_push_h.
+ assumption.
+ apply fork_tau_push_ee_2.
+ apply fork_tau_ce_push_h.
+ assumption.
+ apply JO_red_forkmove2 with (s:=S_First).
+ apply JO_red_forkdocomp1.
+ apply star_refl.
+ simpl; auto.
+ destruct H3 as [p' H1]; destruct H1 as [q' H1]; destruct H1 as [ H1 H3 ]; destruct H3 as [ H3 H4 ]; destruct H4 as [ H4 H5 ]; substs.
+ apply taured_val_id in H3; substs.
+ branch 8. right.
+ exists x q'.
+ intuition.
+ simpl; auto.
+ assert (tauRed (a # LM_expr (b # c)) (x # LM_expr (LM_comp l # LM_expr q'))).
+ apply star_trans with (y:=(x # LM_expr (LM_comp l # LM_expr expr5))).
+ assumption.
+ induction x.
+ apply fork_tau_ce_push_h.
+ apply fork_tau_ce_push_h.
+ assumption.
+ apply fork_tau_push_ee_2.
+ apply fork_tau_ce_push_h.
+ assumption.
+ assumption.
+ apply lab_r with (e1:=(x # (LM_expr ( (LM_comp l) # LM_expr q'))))(e2:=(x # LM_expr ( (E_constant CONST_unit) <# LM_expr q')))(s:=S_Second).
+ intuition.
+ apply star_trans with (y:=(x # LM_expr (LM_comp l # LM_expr expr5))).
+ assumption.
+ induction x.
+ apply fork_tau_ce_push_h.
+ apply fork_tau_ce_push_h.
+ assumption.
+ apply fork_tau_push_ee_2.
+ apply fork_tau_ce_push_h.
+ assumption.
+ apply JO_red_forkmove2 with (s:=S_First).
+ apply JO_red_forkdocomp1.
+ apply S_star with (y:=(x #> (E_constant CONST_unit <# LM_expr q'))).
+ apply tStep with (s:=S_Second).
+ apply JO_red_forkdeath2.
+ simpl; auto.
+ apply star_refl.
+ simpl; auto. 
+ destruct H3 as [p' H1]; destruct H1 as [q' H1]; destruct H1 as [ H1 H3 ]; destruct H3 as [ H3 H4 ]; destruct H4 as [ H4 H5 ]; substs.
+ apply taured_val_id in H3; substs.
+ branch 3.
+ exists x (LM_expr q') (E_constant CONST_unit).
+ intuition.
+ apply lab_r with (e1:=(x # LM_expr (LM_comp l # LM_expr q')))(e2:=(x # (LM_expr((E_constant CONST_unit) <# LM_expr q'))))(s:=S_Second).
+ intuition.
+ apply star_trans with (y:=(x # LM_expr (LM_comp l # LM_expr expr5))).
+ assumption.
+ induction x.
+ apply fork_tau_ce_push_h.
+ apply fork_tau_ce_push_h.
+ assumption.
+ apply fork_tau_push_ee_2.
+ apply fork_tau_ce_push_h.
+ assumption.
+ apply JO_red_forkmove2 with (s:=S_First).
+ apply JO_red_forkdocomp1.
+ apply  S_star with (y:=(x #> (E_constant CONST_unit <# LM_expr q'))).
+ apply tStep with (s:=S_Second).
+ apply JO_red_forkdeath2.
+ simpl;auto.
+ apply star_refl.
+ simpl; auto.
+ (* B1 - L1 - L5 *)
+ apply red_not_value in H9; simpl in H9; intuition.
+ (* B1 - L1 - L6 *)
+ apply red_not_value in H10; simpl in H10; intuition.
+ (* B1 - L2 *)
+ substs.
+ apply fork_tau_assoc_total in H3.
+ intuition.
+ branch 1.
+ destruct H1 as [ a' H1 ]; destruct H1 as [ b' H1 ]; destruct H1 as [ c' H1 ]; exists a' b' c';
+ intuition.
+ apply lab_r with (e1:=( x # LM_expr (x0 # LM_expr e')))  (e2:=(x # LM_expr (x0 # LM_expr e''))) (s:=S_Second);
+ intuition.
+ apply JO_red_forkmove2 with (s:=S_Second).
+ apply JO_red_forkmove2 with (s:=s0).
+ auto.
+ branch 2;
+ destruct H3 as [ a' H1 ]; destruct H1 as [ b' H1 ]; destruct H1 as [ c' H1 ]; exists a' b' c';
+ intuition.
+ apply lab_r with (e1:=( x # LM_expr (x0 # LM_expr e')))  (e2:=(x # LM_expr (x0 # LM_expr e''))) (s:=S_Second);
+ intuition.
+ apply JO_red_forkmove2 with (s:=S_Second).
+ apply JO_red_forkmove2 with (s:=s0).
+ auto.
+ branch 3;
+ destruct H1 as [ a' H1 ]; destruct H1 as [ b' H1 ]; destruct H1 as [ c' H1 ]; exists a' b' c';
+ intuition.
+ apply lab_r with (e1:=( x # LM_expr (x0 # LM_expr e')))  (e2:=(x # LM_expr (x0 # LM_expr e''))) (s:=S_Second);
+ intuition.
+ apply JO_red_forkmove2 with (s:=S_Second).
+ apply JO_red_forkmove2 with (s:=s0).
+ auto.
+ branch 4;
+ destruct H3 as [ a' H1 ]; destruct H1 as [ b' H1 ]; destruct H1 as [ c' H1 ]; exists a' b' c';
+ intuition.
+ apply lab_r with (e1:=( x # LM_expr (x0 # LM_expr e')))  (e2:=(x # LM_expr (x0 # LM_expr e''))) (s:=S_Second);
+ intuition.
+ apply JO_red_forkmove2 with (s:=S_Second).
+ apply JO_red_forkmove2 with (s:=s0).
+ auto.
+ branch 5.
+ destruct H1 as [ a' H1 ]; destruct H1 as [ b' H1 ]; destruct H1 as [ c' H1 ]; exists a' b' c';
+ intuition.
+ apply lab_r with (e1:=( x # LM_expr (x0 # LM_expr e')))  (e2:=(x # LM_expr (x0 # LM_expr e''))) (s:=S_Second);
+ intuition.
+ apply JO_red_forkmove2 with (s:=S_Second).
+ apply JO_red_forkmove2 with (s:=s0).
+ auto.
+ branch 6.
+ destruct H3 as [ a' H1 ]; destruct H1 as [ b' H1 ]; destruct H1 as [ c' H1 ]; exists a' b' c';
+ intuition.
+ apply lab_r with (e1:=( x # LM_expr (x0 # LM_expr e')))  (e2:=(x # LM_expr (x0 # LM_expr e''))) (s:=S_Second);
+ intuition.
+ apply JO_red_forkmove2 with (s:=S_Second).
+ apply JO_red_forkmove2 with (s:=s0).
+ auto.
+ branch 7.
+ destruct H1 as [ a' H1 ]; destruct H1 as [ b' H1 ]; destruct H1 as [ c' H1 ]; exists a' b' c';
+ intuition.
+ apply lab_r with (e1:=( x # LM_expr (x0 # LM_expr e')))  (e2:=(x # LM_expr (x0 # LM_expr e''))) (s:=S_Second);
+ intuition.
+ apply JO_red_forkmove2 with (s:=S_Second).
+ apply JO_red_forkmove2 with (s:=s0).
+ auto.
+ branch 8.
+ left.
+ destruct H1 as [ a' H1 ]; destruct H1 as [ b' H1 ]; destruct H1 as [ c' H1 ]; exists a' b' c';
+ intuition.
+ apply lab_r with (e1:=( x # LM_expr (x0 # LM_expr e')))  (e2:=(x # LM_expr (x0 # LM_expr e''))) (s:=S_Second);
+ intuition.
+ apply JO_red_forkmove2 with (s:=S_Second).
+ apply JO_red_forkmove2 with (s:=s0).
+ auto.
+ (* B1 - L3 *)
+ substs.
+ apply taured_val_id in H3.
+ substs.
+ branch 2.
+ exists x x0 (E_constant CONST_unit).
+ intuition.
+ simpl; auto.
+ apply lab_r with (e1:=(x # LM_expr (x0 # LM_comp l))) (e2:=(x # LM_expr (x0 #> E_constant CONST_unit))) (s:=S_Second).
+ intuition.
+ apply JO_red_forkmove2 with (s:=S_Second).
+ apply JO_red_forkdocomp2.
+ apply S_star with (y:=(x #> (x0 #> E_constant CONST_unit))).
+ apply tStep with (s:=S_Second).
+ apply JO_red_forkdeath2.
+ simpl; auto.
+ auto.
+ simpl; auto.
+ (* B1 - L4 *)
+ apply red_not_value in H8; simpl in H8; intuition.
+ (* B1 - L5 *)
+ apply red_not_value in H9; simpl in H9; intuition.
+ (* B2 *)
+ destruct H1.
+ destruct H1.
+ destruct H1.
+ destruct H1.
+ substs.
+ apply red_not_value in H0; simpl in H0; intuition.
+ (* B3 *)
+ destruct H2.
+ destruct H1.
+ destruct H1.
+ destruct H1.
+ substs.
+ apply red_not_value in H0; simpl in H0; intuition.
+ (* B4 LM_expr (a' #> b') # c' *)
+ destruct H1.
+ destruct H1.
+ destruct H1.
+ destruct H1.
+ substs.
+ inversion H0.
+ (* B4 - L1 *)
+ substs.
+ apply red_not_value in H8; simpl in H8; intuition.
+ (* B4 - L2 *)
+ substs.
+ apply fork_tau_behave_ee in H3.
+ intuition.
+  (* B4-L2-T1 *)
+  destruct H4.
+  destruct H3.
+  destruct H3.
+  destruct H4.
+  substs.
+  apply taured_val_id in H3.
+  substs.
+  branch 4.
+  exists x (LM_expr x2) x1.
+  intuition.
+  apply lab_r with (e1:=( x # LM_expr (LM_expr x1 # LM_expr e')))(e2:=( x # LM_expr (LM_expr x1 # LM_expr e'')))(s:=S_Second).
+ intuition.
+ apply JO_red_forkmove2 with (s:=S_Second).
+  apply JO_red_forkmove2 with (s:=s0).
+ assumption.
+ apply star_trans with (y:=( x # LM_expr (LM_expr x1 # LM_expr x2))).
+ induction x.
+ apply fork_tau_ce_push_h.
+ apply fork_tau_push_ee_2.
+ assumption.
+ 
+ apply fork_tau_push_ee_2.
+ apply fork_tau_push_ee_12.
+ assumption.
+ apply star_refl.
+ apply S_star with (y:=(x # LM_expr (x1 <# LM_expr x2))).
+ apply tStep with (s:=S_Second).
+ apply JO_red_forkmove2 with (s:=S_First).
+ apply JO_red_forkdeath1.
+ simpl; auto.
+ apply star_refl.
+ simpl; auto.
+  (* B4-L2-T2 *)
+  destruct H3.
+  destruct H3.
+  destruct H3.
+  destruct H4.
+  destruct H6.
+  substs.
+  apply taured_val_id in H4.
+  substs.
+  branch 7.
+  exists x x1 x2.
+  intuition.
+  apply lab_r with (e1:=(x # LM_expr (LM_expr x1 # LM_expr e')))(e2:=(x # LM_expr (LM_expr x1 # LM_expr e'')))(s:=S_Second).
+ intuition.
+ apply JO_red_forkmove2 with (s:=S_Second).
+  apply JO_red_forkmove2 with (s:=s0).
+ assumption.
+ apply star_trans with (y:=(x # LM_expr (LM_expr x1 # LM_expr x2))).
+ 
+ induction x.
+ apply fork_tau_ce_push_h.
+ apply fork_tau_push_ee_2.
+ 
+ assumption.
+ apply fork_tau_push_ee_2.
+ apply fork_tau_push_ee_2.
+ assumption.
+ apply S_star with (y:=( x # LM_expr (LM_expr x1 #> x2))).
+ apply tStep with (s:=S_Second).
+ apply JO_red_forkmove2 with (s:=S_Second).
+ apply JO_red_forkdeath2.
+ assumption.
+ apply S_star with (y:=(x #> (LM_expr x1 #> x2))).
+ apply tStep with (s:=S_Second).
+ apply JO_red_forkdeath2.
+ simpl; auto.
+ simpl; auto.
+ simpl; auto.
+  (* B4-L2-T3 *)
+  destruct H3.
+  destruct H3.
+  destruct H3.
+  destruct H4.
+  destruct H6.
+  substs.
+  apply taured_val_id in H4.
+  substs.
+  branch 3.
+  exists x (LM_expr x2) x1.
+  intuition.
+  apply lab_r with (e1:=(x # LM_expr (LM_expr x1 # LM_expr e')))(e2:=(x # LM_expr (LM_expr x1 # LM_expr e'')))(s:=S_Second).
+ intuition.
+ apply JO_red_forkmove2 with (s:=S_Second).
+  apply JO_red_forkmove2 with (s:=s0).
+ assumption.
+ apply star_trans with (y:=(x # LM_expr (LM_expr x1 # LM_expr x2))).
+
+ induction x.
+ apply fork_tau_ce_push_h.
+  apply fork_tau_push_ee_2.
+ assumption.
+ apply fork_tau_push_ee_2.
+  apply fork_tau_push_ee_2.
+ assumption.
+ apply S_star with (y:=(x # LM_expr (x1 <# LM_expr x2))).
+ apply tStep with (s:=S_Second).
+ apply JO_red_forkmove2 with (s:=S_First).
+ apply JO_red_forkdeath1.
+ assumption.
+ apply S_star with (y:=(x #> (x1 <# LM_expr x2))).
+ apply tStep with (s:=S_Second).
+ apply JO_red_forkdeath2.
+ assumption.
+ simpl; auto.
+ simpl; auto.
+ (* B4 - L3 *)
+ substs.
+ branch 7.
+ apply taured_val_id in H3.
+ substs.
+ exists x x1 (E_constant CONST_unit).
+ intuition.
+ simpl; auto.
+ apply lab_r with (e1:=(x # LM_expr (LM_expr x1 # LM_comp l)))(e2:=(x # LM_expr (LM_expr x1 #> (E_constant CONST_unit))))(s:=S_Second).
+ intuition.
+ apply JO_red_forkmove2 with (s:=S_Second).
+ apply JO_red_forkdocomp2.
+ apply S_star with (y:=(x #> (LM_expr x1 #> E_constant CONST_unit))).
+ apply tStep with (s:=S_Second).
+ apply JO_red_forkdeath2.
+ simpl; auto.
+ apply star_refl.
+ simpl; auto.
+ (* B4 - L4 *)
+ substs.
+ apply red_not_value in H8; simpl in H8; intuition.
+ (* B4 - L5 *)
+ apply red_not_value in H9; simpl in H9; intuition.
+ (* B5 *)
+ destruct H2.
+ destruct H1.
+ destruct H1.
+ destruct H1.
+ substs.
+ inversion H0.
+ (* B5 - L1 *)
+ substs.
+ apply red_not_value in H8; simpl in H8; intuition.
+ (* B5 - L2 *)
+ substs.
+ apply fork_tau_behave_ee in H3.
+ intuition.
+  (* B5-L2-T1 *)
+  destruct H4.
+  destruct H3.
+  destruct H3.
+  destruct H4.
+  substs.
+  apply taured_val_id in H3.
+  substs.
+  branch 5.
+  exists x (LM_expr x2) x1.
+  intuition.
+  apply lab_r with (e1:=(LM_expr x1 # LM_expr (x # LM_expr e')))(e2:=(LM_expr x1 # LM_expr (x # LM_expr e'')))(s:=S_Second).
+ intuition.
+ apply JO_red_forkmove2 with (s:=S_Second).
+  apply JO_red_forkmove2 with (s:=s0).
+ assumption.
+ apply star_trans with (y:=(LM_expr x1 # LM_expr (x # LM_expr x2))).
+ apply fork_tau_push_ee_12.
+ induction x.
+ apply fork_tau_ce_push_h.
+ assumption.
+ apply fork_tau_push_ee_2.
+ assumption.
+ apply star_refl.
+ apply S_star with (y:=(x1 <# LM_expr (x # LM_expr x2))).
+ apply tStep with (s:=S_First).
+ apply JO_red_forkdeath1.
+ simpl; auto.
+ apply star_refl.
+ simpl; auto.
+  (* B5-L2-T2 *)
+  destruct H3.
+  destruct H3.
+  destruct H3.
+  destruct H4.
+  destruct H6.
+  substs.
+  apply taured_val_id in H4.
+  substs.
+  branch 8.
+  left.
+  exists x x1 x2.
+  intuition.
+  apply lab_r with (e1:=(LM_expr x1 # LM_expr (x # LM_expr e')))(e2:=(LM_expr x1 # LM_expr (x # LM_expr e'')))(s:=S_Second).
+ intuition.
+ apply JO_red_forkmove2 with (s:=S_Second).
+  apply JO_red_forkmove2 with (s:=s0).
+ assumption.
+ apply star_trans with (y:=(LM_expr x1 # LM_expr (x # LM_expr x2))).
+ apply fork_tau_push_ee_12.
+ induction x.
+ apply fork_tau_ce_push_h.
+ assumption.
+ apply fork_tau_push_ee_2.
+ assumption.
+ apply star_refl.
+ apply S_star with (y:=( (LM_expr x1) # LM_expr (x #> x2))).
+ apply tStep with (s:=S_Second).
+ apply JO_red_forkmove2 with (s:=S_Second).
+ apply JO_red_forkdeath2.
+ assumption.
+ apply S_star with (y:=(  x1 <# LM_expr (x #> x2))).
+ apply tStep with (s:=S_First).
+ apply JO_red_forkdeath1.
+ assumption.
+ simpl; auto.
+ simpl; auto.
+  (* B5-L2-T3 *)
+  destruct H3.
+  destruct H3.
+  destruct H3.
+  destruct H4.
+  destruct H6.
+  substs.
+  apply taured_val_id in H4.
+  substs.
+  branch 6.
+  exists x (LM_expr x2) x1.
+  intuition.
+  apply lab_r with (e1:=(LM_expr x1 # LM_expr (x # LM_expr e')))(e2:=(LM_expr x1 # LM_expr (x # LM_expr e'')))(s:=S_Second).
+ intuition.
+ apply JO_red_forkmove2 with (s:=S_Second).
+  apply JO_red_forkmove2 with (s:=s0).
+ assumption.
+ apply star_trans with (y:=(LM_expr x1 # LM_expr (x # LM_expr x2))).
+ apply fork_tau_push_ee_12.
+ induction x.
+ apply fork_tau_ce_push_h.
+ assumption.
+ apply fork_tau_push_ee_2.
+ assumption.
+ apply star_refl.
+ apply S_star with (y:=( x1 <# LM_expr (x # LM_expr x2))).
+ apply tStep with (s:=S_First).
+ apply JO_red_forkdeath1.
+ assumption.
+ simpl; auto.
+ simpl; auto.
+ (* B5 - L3 *)
+ substs.
+ branch 8.
+ apply taured_val_id in H3.
+ substs.
+ left.
+ exists x x1 (E_constant CONST_unit).
+ intuition.
+ simpl; auto.
+ apply lab_r with (e1:=(LM_expr x1 # LM_expr (x # LM_comp l)))(e2:=((LM_expr x1) # LM_expr ( x #> (E_constant CONST_unit))))(s:=S_Second).
+ intuition.
+ apply JO_red_forkmove2 with (s:=S_Second).
+ apply JO_red_forkdocomp2.
+ apply S_star with (y:=(x1 <# LM_expr (x #> E_constant CONST_unit))).
+ apply tStep with (s:=S_First).
+ apply JO_red_forkdeath1.
+ simpl; auto.
+ apply star_refl.
+ simpl; auto.
+ (* B5 - L4 *)
+ substs.
+ apply red_not_value in H8; simpl in H8; intuition.
+ (* B4 - L5 *)
+ apply red_not_value in H9; simpl in H9; intuition.
+ (* B6 *)
+ destruct H1.
+ destruct H1.
+ destruct H1.
+ destruct H1.
+ substs.
+ apply red_not_value in H0; simpl in H0; intuition.
+ (* B7 *)
+ destruct H2.
+ destruct H1.
+ destruct H1.
+ destruct H1.
+ substs.
+ apply red_not_value in H0; simpl in H0; intuition.
+ (* B8 *)
+ destruct H2.
+ destruct H1.
+ destruct H1.
+ destruct H1.
+ substs.
+ apply red_not_value in H0; simpl in H0; intuition.
+Qed.
+
+(*
+ 
+Inductive fork_assoc_rel :  relation expr := 
+ | forka_start : forall (a b c : livemodes), fork_assoc_rel (E_apply (E_apply (E_constant CONST_fork) ( (E_live_expr (LM_expr (E_apply (E_apply (E_constant CONST_fork) ( (E_live_expr a)) ) ( (E_live_expr b)))))) ) ( (E_live_expr c))) (E_apply (E_apply (E_constant CONST_fork) ( (E_live_expr a)) ) ( (E_live_expr (LM_expr (E_apply (E_apply (E_constant CONST_fork) ( (E_live_expr b)) ) ( (E_live_expr c)))))))
+ | forka_tau : forall  (e e' : expr),  is_value_of_expr e /\ is_value_of_expr e' -> fork_assoc_rel e e'.
+
+Theorem fork_assoc_wbsm : forall (p q : expr), fork_assoc_rel p q -> ((forall (l : label) (p' : expr), labRed l p p' -> (exists (q' : expr), labRed l q q' /\ fork_assoc_rel p' q') ) /\ (forall (l : label) (q' : expr), labRed l q q' -> (exists (p' : expr), labRed l p p' /\ fork_assoc_rel p' q') )).
+Proof.
+ intros.
+ splits.
+ intros.
+ assert (L:=H0).
+ inversion H.
+ substs.
+ apply fork_lab_behave in H0.
+ intuition.
+ destruct H1.
+ destruct H0.
+ substs.
+ induction c.
+ assert (H0:=L).
+ apply fork_label_behave_ec in H0.
+ intuition.
+ destruct H2.
+ intuition.
+ discriminate H3.
+ destruct H0.
+ intuition.
+ simplify_eq H2; clear H2; intros; substs.
+ assert (K:=H1).
+ induction b.
+ induction a.
+ apply fork_label_origin_cc in H1.
+ intuition.
+ substs.
+ apply fork_label_behave in H1.
+ intuition.
+ destruct H0.
+ destruct H0.
+ substs.
+ 
+ exists ( x # LM_expr ( x0 # LM_comp lab)).
+ splits.
+ substs.
+ intuition.
+ substs.
+ admit.
+ assert (H0:=L).
+ apply fork_label_origin_ee in H0.
+ intuition.
+ destruct H1.
+ intuition.
+ destruct H0.
+ intuition.
+ simplify_eq H3.
+ intros.
+ substs.
+ clear H3.
+ substs.
+
+ admit.
+
+
+ substs.
+ destruct H2.
+ intuition.
+ discriminate H4.
+ destruct H2.
+ intuition.
+ discriminate H4.
+ destruct H1.
+ intuition.
+ destruct H0.
+ intuition.
+ simplify_eq H3; clear H3; intros; substs.
+ apply fork_tau_behave_total in H2.
+ intuition.
+ destruct H0.
+ destruct H0.
+ substs.
+ exists ((-< LM_expr (-< a b) LM_expr expr5)).
+ substs.
+ destruct H2.
+ destruct H0.
+ admit.
+ 
+ 
+
+ 
+ substs.
+ intuition. 
+ apply labred_not_val in H0.
+ intuition.
+ 
+
+ intros.
+ assert (L:=H0).
+ inversion H.
+ substs.
+ 
+ apply fork_lab_behave in H0.
+ intuition.
+ destruct H1.
+ destruct H0.
+ substs.
+ admit.
+ intuition.
+ destruct H0.
+ substs.
+ destruct H2.
+ destruct H0.
+ intuition.
+ admit.
+
+ admit.
+ 
+
+ substs.
+ intuition. 
+ apply labred_not_val in H0.
+ intuition.
+Qed.
+
+-< (-< a b) (c) = -< (a) (-< b c)
+*)
